<?xml version="1.0"?>
<rdf:RDF xmlns="http://purl.org/dc/elements/1.1/"
     xml:base="http://purl.org/dc/elements/1.1/"
     xmlns:dc="http://purl.org/dc/elements/1.1/"
     xmlns:mo="http://purl.org/ontology/mo/"
     xmlns:po="http://purl.org/ontology/po/"
     xmlns:tl="http://purl.org/NET/c4dm/timeline.owl#"
     xmlns:vs="http://www.w3.org/2003/06/sw-vocab-status/ns#"
     xmlns:geo="http://www.w3.org/2003/01/geo/wgs84_pos#"
     xmlns:owl="http://www.w3.org/2002/07/owl#"
     xmlns:rdf="http://www.w3.org/1999/02/22-rdf-syntax-ns#"
     xmlns:xml="http://www.w3.org/XML/1998/namespace"
     xmlns:xsd="http://www.w3.org/2001/XMLSchema#"
     xmlns:foaf="http://xmlns.com/foaf/0.1/"
     xmlns:frbr="http://purl.org/vocab/frbr/core#"
     xmlns:rdfs="http://www.w3.org/2000/01/rdf-schema#"
     xmlns:skos="http://www.w3.org/2004/02/skos/core#"
     xmlns:tags="http://www.holygoat.co.uk/owl/redwood/0.1/tags/"
     xmlns:event="http://purl.org/NET/c4dm/event.owl#"
     xmlns:dcterms="http://purl.org/dc/terms/"
     xmlns:provenance="http://www.bbc.co.uk/ontologies/provenance/">
    <owl:Ontology rdf:about="http://purl.org/dc/elements/1.1/">
        <owl:versionIRI rdf:resource="http://purl.org/ontology/po/1.1"/>
        <owl:imports rdf:resource="http://purl.org/NET/c4dm/event.owl"/>
        <owl:imports rdf:resource="http://purl.org/NET/c4dm/timeline.owl"/>
        <owl:imports rdf:resource="http://www.bbc.co.uk/ontologies/provenance"/>
        <creator rdf:resource="http://moustaki.org/foaf.rdf#moustaki"/>
        <provenance:canonicalLocation rdf:datatype="http://www.w3.org/2001/XMLSchema#string">https://repo.dev.bbc.co.uk/services/linked-data/ontologies/domain/programmes</provenance:canonicalLocation>
        <provenance:changeReason xml:lang="en-gb">Adding contributor</provenance:changeReason>
        <provenance:public rdf:datatype="http://www.w3.org/2001/XMLSchema#boolean">true</provenance:public>
        <provenance:slug rdf:datatype="http://www.w3.org/2001/XMLSchema#string">po</provenance:slug>
        <provenance:version rdf:datatype="http://www.w3.org/2001/XMLSchema#string">1.1</provenance:version>
        <rdfs:comment>
		A vocabulary for programme data.
		It defines concepts such as brands, series, episodes, broadcasts, etc.
	</rdfs:comment>
        <rdfs:isDefinedBy rdf:resource="http://purl.org/ontology/po/"/>
        <rdfs:label>Programmes ontology</rdfs:label>
        <owl:priorVersion rdf:resource="http://purl.org/ontology/po/1.0"/>
        <owl:versionInfo rdf:datatype="http://www.w3.org/2001/XMLSchema#string">1.1</owl:versionInfo>
    </owl:Ontology>
    


    <!-- 
    ///////////////////////////////////////////////////////////////////////////////////////
    //
    // Annotation properties
    //
    ///////////////////////////////////////////////////////////////////////////////////////
     -->

    


    <!-- http://purl.org/dc/elements/1.1/coverage -->

    <owl:AnnotationProperty rdf:about="http://purl.org/dc/elements/1.1/coverage">
        <dcterms:description xml:lang="en">Spatial topic and spatial applicability may be a named place or a location specified by its geographic coordinates. Temporal topic may be a named period, date, or date range. A jurisdiction may be a named administrative entity or a geographic place to which the resource applies. Recommended best practice is to use a controlled vocabulary such as the Thesaurus of Geographic Names [TGN]. Where appropriate, named places or time periods can be used in preference to numeric identifiers such as sets of coordinates or date ranges.</dcterms:description>
        <dcterms:hasVersion rdf:resource="http://dublincore.org/usage/terms/history/#coverage-006"/>
        <dcterms:issued rdf:datatype="http://www.w3.org/2001/XMLSchema#date">1999-07-02</dcterms:issued>
        <dcterms:modified rdf:datatype="http://www.w3.org/2001/XMLSchema#date">2008-01-14</dcterms:modified>
        <rdfs:comment xml:lang="en">The spatial or temporal topic of the resource, the spatial applicability of the resource, or the jurisdiction under which the resource is relevant.</rdfs:comment>
        <rdfs:isDefinedBy rdf:resource="http://purl.org/dc/elements/1.1/"/>
        <rdfs:label xml:lang="en">Coverage</rdfs:label>
        <skos:note xml:lang="en">A second property with the same name as this property has been declared in the dcterms: namespace (http://purl.org/dc/terms/).  See the Introduction to the document &quot;DCMI Metadata Terms&quot; (http://dublincore.org/documents/dcmi-terms/) for an explanation.</skos:note>
    </owl:AnnotationProperty>
    


    <!-- http://purl.org/dc/elements/1.1/creator -->

    <owl:AnnotationProperty rdf:about="http://purl.org/dc/elements/1.1/creator">
        <dcterms:description xml:lang="en">Examples of a Creator include a person, an organization, or a service. Typically, the name of a Creator should be used to indicate the entity.</dcterms:description>
        <dcterms:hasVersion rdf:resource="http://dublincore.org/usage/terms/history/#creator-006"/>
        <dcterms:issued rdf:datatype="http://www.w3.org/2001/XMLSchema#date">1999-07-02</dcterms:issued>
        <dcterms:modified rdf:datatype="http://www.w3.org/2001/XMLSchema#date">2008-01-14</dcterms:modified>
        <rdfs:comment xml:lang="en">An entity primarily responsible for making the resource.</rdfs:comment>
        <rdfs:isDefinedBy rdf:resource="http://purl.org/dc/elements/1.1/"/>
        <rdfs:label xml:lang="en">Creator</rdfs:label>
        <skos:note xml:lang="en">A second property with the same name as this property has been declared in the dcterms: namespace (http://purl.org/dc/terms/).  See the Introduction to the document &quot;DCMI Metadata Terms&quot; (http://dublincore.org/documents/dcmi-terms/) for an explanation.</skos:note>
    </owl:AnnotationProperty>
    


    <!-- http://purl.org/dc/elements/1.1/description -->

    <owl:AnnotationProperty rdf:about="http://purl.org/dc/elements/1.1/description">
        <dcterms:description xml:lang="en">Description may include but is not limited to: an abstract, a table of contents, a graphical representation, or a free-text account of the resource.</dcterms:description>
        <dcterms:hasVersion rdf:resource="http://dublincore.org/usage/terms/history/#description-006"/>
        <dcterms:issued rdf:datatype="http://www.w3.org/2001/XMLSchema#date">1999-07-02</dcterms:issued>
        <dcterms:modified rdf:datatype="http://www.w3.org/2001/XMLSchema#date">2008-01-14</dcterms:modified>
        <rdfs:comment xml:lang="en">An account of the resource.</rdfs:comment>
        <rdfs:isDefinedBy rdf:resource="http://purl.org/dc/elements/1.1/"/>
        <rdfs:label xml:lang="en">Description</rdfs:label>
        <skos:note xml:lang="en">A second property with the same name as this property has been declared in the dcterms: namespace (http://purl.org/dc/terms/).  See the Introduction to the document &quot;DCMI Metadata Terms&quot; (http://dublincore.org/documents/dcmi-terms/) for an explanation.</skos:note>
    </owl:AnnotationProperty>
    


    <!-- http://purl.org/dc/elements/1.1/format -->

    <owl:AnnotationProperty rdf:about="http://purl.org/dc/elements/1.1/format">
        <dcterms:description xml:lang="en">Examples of dimensions include size and duration. Recommended best practice is to use a controlled vocabulary such as the list of Internet Media Types [MIME].</dcterms:description>
        <dcterms:hasVersion rdf:resource="http://dublincore.org/usage/terms/history/#format-007"/>
        <dcterms:issued rdf:datatype="http://www.w3.org/2001/XMLSchema#date">1999-07-02</dcterms:issued>
        <dcterms:modified rdf:datatype="http://www.w3.org/2001/XMLSchema#date">2008-01-14</dcterms:modified>
        <rdfs:comment xml:lang="en">The file format, physical medium, or dimensions of the resource.</rdfs:comment>
        <rdfs:isDefinedBy rdf:resource="http://purl.org/dc/elements/1.1/"/>
        <rdfs:label xml:lang="en">Format</rdfs:label>
        <skos:note xml:lang="en">A second property with the same name as this property has been declared in the dcterms: namespace (http://purl.org/dc/terms/).  See the Introduction to the document &quot;DCMI Metadata Terms&quot; (http://dublincore.org/documents/dcmi-terms/) for an explanation.</skos:note>
    </owl:AnnotationProperty>
    


    <!-- http://purl.org/dc/elements/1.1/identifier -->

    <owl:AnnotationProperty rdf:about="http://purl.org/dc/elements/1.1/identifier">
        <dcterms:description xml:lang="en">Recommended best practice is to identify the resource by means of a string conforming to a formal identification system. </dcterms:description>
        <dcterms:hasVersion rdf:resource="http://dublincore.org/usage/terms/history/#identifier-006"/>
        <dcterms:issued rdf:datatype="http://www.w3.org/2001/XMLSchema#date">1999-07-02</dcterms:issued>
        <dcterms:modified rdf:datatype="http://www.w3.org/2001/XMLSchema#date">2008-01-14</dcterms:modified>
        <rdfs:comment xml:lang="en">An unambiguous reference to the resource within a given context.</rdfs:comment>
        <rdfs:isDefinedBy rdf:resource="http://purl.org/dc/elements/1.1/"/>
        <rdfs:label xml:lang="en">Identifier</rdfs:label>
        <skos:note xml:lang="en">A second property with the same name as this property has been declared in the dcterms: namespace (http://purl.org/dc/terms/).  See the Introduction to the document &quot;DCMI Metadata Terms&quot; (http://dublincore.org/documents/dcmi-terms/) for an explanation.</skos:note>
    </owl:AnnotationProperty>
    


    <!-- http://purl.org/dc/elements/1.1/language -->

    <owl:AnnotationProperty rdf:about="http://purl.org/dc/elements/1.1/language">
        <dcterms:description xml:lang="en">Recommended best practice is to use a controlled vocabulary such as RFC 4646 [RFC4646].</dcterms:description>
        <dcterms:hasVersion rdf:resource="http://dublincore.org/usage/terms/history/#language-007"/>
        <dcterms:issued rdf:datatype="http://www.w3.org/2001/XMLSchema#date">1999-07-02</dcterms:issued>
        <dcterms:modified rdf:datatype="http://www.w3.org/2001/XMLSchema#date">2008-01-14</dcterms:modified>
        <rdfs:comment xml:lang="en">A language of the resource.</rdfs:comment>
        <rdfs:isDefinedBy rdf:resource="http://purl.org/dc/elements/1.1/"/>
        <rdfs:label xml:lang="en">Language</rdfs:label>
        <rdfs:seeAlso rdf:resource="http://www.ietf.org/rfc/rfc4646.txt"/>
        <skos:note xml:lang="en">A second property with the same name as this property has been declared in the dcterms: namespace (http://purl.org/dc/terms/).  See the Introduction to the document &quot;DCMI Metadata Terms&quot; (http://dublincore.org/documents/dcmi-terms/) for an explanation.</skos:note>
    </owl:AnnotationProperty>
    


    <!-- http://purl.org/dc/elements/1.1/publisher -->

    <owl:AnnotationProperty rdf:about="http://purl.org/dc/elements/1.1/publisher">
        <dcterms:description xml:lang="en">Examples of a Publisher include a person, an organization, or a service. Typically, the name of a Publisher should be used to indicate the entity.</dcterms:description>
        <dcterms:hasVersion rdf:resource="http://dublincore.org/usage/terms/history/#publisher-006"/>
        <dcterms:issued rdf:datatype="http://www.w3.org/2001/XMLSchema#date">1999-07-02</dcterms:issued>
        <dcterms:modified rdf:datatype="http://www.w3.org/2001/XMLSchema#date">2008-01-14</dcterms:modified>
        <rdfs:comment xml:lang="en">An entity responsible for making the resource available.</rdfs:comment>
        <rdfs:isDefinedBy rdf:resource="http://purl.org/dc/elements/1.1/"/>
        <rdfs:label xml:lang="en">Publisher</rdfs:label>
        <skos:note xml:lang="en">A second property with the same name as this property has been declared in the dcterms: namespace (http://purl.org/dc/terms/).  See the Introduction to the document &quot;DCMI Metadata Terms&quot; (http://dublincore.org/documents/dcmi-terms/) for an explanation.</skos:note>
    </owl:AnnotationProperty>
    


    <!-- http://purl.org/dc/elements/1.1/relation -->

    <owl:AnnotationProperty rdf:about="http://purl.org/dc/elements/1.1/relation">
        <dcterms:description xml:lang="en">Recommended best practice is to identify the related resource by means of a string conforming to a formal identification system. </dcterms:description>
        <dcterms:hasVersion rdf:resource="http://dublincore.org/usage/terms/history/#relation-006"/>
        <dcterms:issued rdf:datatype="http://www.w3.org/2001/XMLSchema#date">1999-07-02</dcterms:issued>
        <dcterms:modified rdf:datatype="http://www.w3.org/2001/XMLSchema#date">2008-01-14</dcterms:modified>
        <rdfs:comment xml:lang="en">A related resource.</rdfs:comment>
        <rdfs:isDefinedBy rdf:resource="http://purl.org/dc/elements/1.1/"/>
        <rdfs:label xml:lang="en">Relation</rdfs:label>
        <skos:note xml:lang="en">A second property with the same name as this property has been declared in the dcterms: namespace (http://purl.org/dc/terms/).  See the Introduction to the document &quot;DCMI Metadata Terms&quot; (http://dublincore.org/documents/dcmi-terms/) for an explanation.</skos:note>
    </owl:AnnotationProperty>
    


    <!-- http://purl.org/dc/elements/1.1/rights -->

    <owl:AnnotationProperty rdf:about="http://purl.org/dc/elements/1.1/rights">
        <dcterms:description xml:lang="en">Typically, rights information includes a statement about various property rights associated with the resource, including intellectual property rights.</dcterms:description>
        <dcterms:hasVersion rdf:resource="http://dublincore.org/usage/terms/history/#rights-006"/>
        <dcterms:issued rdf:datatype="http://www.w3.org/2001/XMLSchema#date">1999-07-02</dcterms:issued>
        <dcterms:modified rdf:datatype="http://www.w3.org/2001/XMLSchema#date">2008-01-14</dcterms:modified>
        <rdfs:comment xml:lang="en">Information about rights held in and over the resource.</rdfs:comment>
        <rdfs:isDefinedBy rdf:resource="http://purl.org/dc/elements/1.1/"/>
        <rdfs:label xml:lang="en">Rights</rdfs:label>
        <skos:note xml:lang="en">A second property with the same name as this property has been declared in the dcterms: namespace (http://purl.org/dc/terms/).  See the Introduction to the document &quot;DCMI Metadata Terms&quot; (http://dublincore.org/documents/dcmi-terms/) for an explanation.</skos:note>
    </owl:AnnotationProperty>
    


    <!-- http://purl.org/dc/elements/1.1/source -->

    <owl:AnnotationProperty rdf:about="http://purl.org/dc/elements/1.1/source">
        <dcterms:description xml:lang="en">The described resource may be derived from the related resource in whole or in part. Recommended best practice is to identify the related resource by means of a string conforming to a formal identification system.</dcterms:description>
        <dcterms:hasVersion rdf:resource="http://dublincore.org/usage/terms/history/#source-006"/>
        <dcterms:issued rdf:datatype="http://www.w3.org/2001/XMLSchema#date">1999-07-02</dcterms:issued>
        <dcterms:modified rdf:datatype="http://www.w3.org/2001/XMLSchema#date">2008-01-14</dcterms:modified>
        <rdfs:comment xml:lang="en">A related resource from which the described resource is derived.</rdfs:comment>
        <rdfs:isDefinedBy rdf:resource="http://purl.org/dc/elements/1.1/"/>
        <rdfs:label xml:lang="en">Source</rdfs:label>
        <skos:note xml:lang="en">A second property with the same name as this property has been declared in the dcterms: namespace (http://purl.org/dc/terms/).  See the Introduction to the document &quot;DCMI Metadata Terms&quot; (http://dublincore.org/documents/dcmi-terms/) for an explanation.</skos:note>
    </owl:AnnotationProperty>
    


    <!-- http://purl.org/dc/elements/1.1/subject -->

    <owl:AnnotationProperty rdf:about="http://purl.org/dc/elements/1.1/subject">
        <dcterms:description xml:lang="en">Typically, the subject will be represented using keywords, key phrases, or classification codes. Recommended best practice is to use a controlled vocabulary.</dcterms:description>
        <dcterms:hasVersion rdf:resource="http://dublincore.org/usage/terms/history/#subject-007"/>
        <dcterms:issued rdf:datatype="http://www.w3.org/2001/XMLSchema#date">1999-07-02</dcterms:issued>
        <dcterms:modified rdf:datatype="http://www.w3.org/2001/XMLSchema#date">2012-06-14</dcterms:modified>
        <rdfs:comment xml:lang="en">The topic of the resource.</rdfs:comment>
        <rdfs:isDefinedBy rdf:resource="http://purl.org/dc/elements/1.1/"/>
        <rdfs:label xml:lang="en">Subject</rdfs:label>
        <skos:note xml:lang="en">A second property with the same name as this property has been declared in the dcterms: namespace (http://purl.org/dc/terms/).  See the Introduction to the document &quot;DCMI Metadata Terms&quot; (http://dublincore.org/documents/dcmi-terms/) for an explanation.</skos:note>
    </owl:AnnotationProperty>
    


    <!-- http://purl.org/dc/elements/1.1/title -->

    <owl:AnnotationProperty rdf:about="http://purl.org/dc/elements/1.1/title">
        <dcterms:hasVersion rdf:resource="http://dublincore.org/usage/terms/history/#title-006"/>
        <dcterms:issued rdf:datatype="http://www.w3.org/2001/XMLSchema#date">1999-07-02</dcterms:issued>
        <dcterms:modified rdf:datatype="http://www.w3.org/2001/XMLSchema#date">2008-01-14</dcterms:modified>
        <rdfs:comment xml:lang="en">A name given to the resource.</rdfs:comment>
        <rdfs:isDefinedBy rdf:resource="http://purl.org/dc/elements/1.1/"/>
        <rdfs:label xml:lang="en">Title</rdfs:label>
        <skos:note xml:lang="en">A second property with the same name as this property has been declared in the dcterms: namespace (http://purl.org/dc/terms/).  See the Introduction to the document &quot;DCMI Metadata Terms&quot; (http://dublincore.org/documents/dcmi-terms/) for an explanation.</skos:note>
    </owl:AnnotationProperty>
    


    <!-- http://purl.org/dc/elements/1.1/type -->

    <owl:AnnotationProperty rdf:about="http://purl.org/dc/elements/1.1/type">
        <dcterms:description xml:lang="en">Recommended best practice is to use a controlled vocabulary such as the DCMI Type Vocabulary [DCMITYPE]. To describe the file format, physical medium, or dimensions of the resource, use the Format element.</dcterms:description>
        <dcterms:hasVersion rdf:resource="http://dublincore.org/usage/terms/history/#type-006"/>
        <dcterms:issued rdf:datatype="http://www.w3.org/2001/XMLSchema#date">1999-07-02</dcterms:issued>
        <dcterms:modified rdf:datatype="http://www.w3.org/2001/XMLSchema#date">2008-01-14</dcterms:modified>
        <rdfs:comment xml:lang="en">The nature or genre of the resource.</rdfs:comment>
        <rdfs:isDefinedBy rdf:resource="http://purl.org/dc/elements/1.1/"/>
        <rdfs:label xml:lang="en">Type</rdfs:label>
        <skos:note xml:lang="en">A second property with the same name as this property has been declared in the dcterms: namespace (http://purl.org/dc/terms/).  See the Introduction to the document &quot;DCMI Metadata Terms&quot; (http://dublincore.org/documents/dcmi-terms/) for an explanation.</skos:note>
    </owl:AnnotationProperty>
    


    <!-- http://purl.org/dc/terms/abstract -->

    <owl:AnnotationProperty rdf:about="http://purl.org/dc/terms/abstract">
        <rdfs:subPropertyOf rdf:resource="http://purl.org/dc/elements/1.1/description"/>
        <rdfs:subPropertyOf rdf:resource="http://purl.org/dc/terms/description"/>
    </owl:AnnotationProperty>
    


    <!-- http://purl.org/dc/terms/accessRights -->

    <owl:AnnotationProperty rdf:about="http://purl.org/dc/terms/accessRights">
        <rdfs:subPropertyOf rdf:resource="http://purl.org/dc/elements/1.1/rights"/>
    </owl:AnnotationProperty>
    


    <!-- http://purl.org/dc/terms/alternative -->

    <owl:AnnotationProperty rdf:about="http://purl.org/dc/terms/alternative">
        <rdfs:subPropertyOf rdf:resource="http://purl.org/dc/elements/1.1/title"/>
    </owl:AnnotationProperty>
    


    <!-- http://purl.org/dc/terms/available -->

    <owl:AnnotationProperty rdf:about="http://purl.org/dc/terms/available">
        <rdfs:subPropertyOf rdf:resource="http://purl.org/dc/elements/1.1/date"/>
    </owl:AnnotationProperty>
    


    <!-- http://purl.org/dc/terms/bibliographicCitation -->

    <owl:AnnotationProperty rdf:about="http://purl.org/dc/terms/bibliographicCitation">
        <rdfs:subPropertyOf rdf:resource="http://purl.org/dc/elements/1.1/identifier"/>
    </owl:AnnotationProperty>
    


    <!-- http://purl.org/dc/terms/conformsTo -->

    <owl:AnnotationProperty rdf:about="http://purl.org/dc/terms/conformsTo">
        <rdfs:subPropertyOf rdf:resource="http://purl.org/dc/elements/1.1/relation"/>
        <rdfs:subPropertyOf rdf:resource="http://purl.org/dc/terms/relation"/>
    </owl:AnnotationProperty>
    


    <!-- http://purl.org/dc/terms/contributor -->

    <owl:AnnotationProperty rdf:about="http://purl.org/dc/terms/contributor">
        <rdfs:subPropertyOf rdf:resource="http://purl.org/dc/elements/1.1/contributor"/>
    </owl:AnnotationProperty>
    


    <!-- http://purl.org/dc/terms/coverage -->

    <owl:AnnotationProperty rdf:about="http://purl.org/dc/terms/coverage">
        <rdfs:subPropertyOf rdf:resource="http://purl.org/dc/elements/1.1/coverage"/>
    </owl:AnnotationProperty>
    


    <!-- http://purl.org/dc/terms/created -->

    <owl:AnnotationProperty rdf:about="http://purl.org/dc/terms/created">
        <rdfs:subPropertyOf rdf:resource="http://purl.org/dc/elements/1.1/date"/>
    </owl:AnnotationProperty>
    


    <!-- http://purl.org/dc/terms/creator -->

    <owl:AnnotationProperty rdf:about="http://purl.org/dc/terms/creator">
        <rdfs:subPropertyOf rdf:resource="http://purl.org/dc/elements/1.1/creator"/>
    </owl:AnnotationProperty>
    


    <!-- http://purl.org/dc/terms/date -->

    <owl:AnnotationProperty rdf:about="http://purl.org/dc/terms/date">
        <rdfs:subPropertyOf rdf:resource="http://purl.org/dc/elements/1.1/date"/>
    </owl:AnnotationProperty>
    


    <!-- http://purl.org/dc/terms/dateAccepted -->

    <owl:AnnotationProperty rdf:about="http://purl.org/dc/terms/dateAccepted">
        <rdfs:subPropertyOf rdf:resource="http://purl.org/dc/elements/1.1/date"/>
    </owl:AnnotationProperty>
    


    <!-- http://purl.org/dc/terms/dateCopyrighted -->

    <owl:AnnotationProperty rdf:about="http://purl.org/dc/terms/dateCopyrighted">
        <rdfs:subPropertyOf rdf:resource="http://purl.org/dc/elements/1.1/date"/>
    </owl:AnnotationProperty>
    


    <!-- http://purl.org/dc/terms/dateSubmitted -->

    <owl:AnnotationProperty rdf:about="http://purl.org/dc/terms/dateSubmitted">
        <rdfs:subPropertyOf rdf:resource="http://purl.org/dc/elements/1.1/date"/>
    </owl:AnnotationProperty>
    


    <!-- http://purl.org/dc/terms/description -->

    <owl:AnnotationProperty rdf:about="http://purl.org/dc/terms/description">
        <rdfs:subPropertyOf rdf:resource="http://purl.org/dc/elements/1.1/description"/>
    </owl:AnnotationProperty>
    


    <!-- http://purl.org/dc/terms/extent -->

    <owl:AnnotationProperty rdf:about="http://purl.org/dc/terms/extent">
        <rdfs:subPropertyOf rdf:resource="http://purl.org/dc/elements/1.1/format"/>
    </owl:AnnotationProperty>
    


    <!-- http://purl.org/dc/terms/format -->

    <owl:AnnotationProperty rdf:about="http://purl.org/dc/terms/format">
        <rdfs:subPropertyOf rdf:resource="http://purl.org/dc/elements/1.1/format"/>
    </owl:AnnotationProperty>
    


    <!-- http://purl.org/dc/terms/hasFormat -->

    <owl:AnnotationProperty rdf:about="http://purl.org/dc/terms/hasFormat">
        <rdfs:subPropertyOf rdf:resource="http://purl.org/dc/elements/1.1/relation"/>
        <rdfs:subPropertyOf rdf:resource="http://purl.org/dc/terms/relation"/>
    </owl:AnnotationProperty>
    


    <!-- http://purl.org/dc/terms/hasPart -->

    <owl:AnnotationProperty rdf:about="http://purl.org/dc/terms/hasPart">
        <rdfs:subPropertyOf rdf:resource="http://purl.org/dc/elements/1.1/relation"/>
        <rdfs:subPropertyOf rdf:resource="http://purl.org/dc/terms/relation"/>
    </owl:AnnotationProperty>
    


    <!-- http://purl.org/dc/terms/hasVersion -->

    <owl:AnnotationProperty rdf:about="http://purl.org/dc/terms/hasVersion">
        <rdfs:subPropertyOf rdf:resource="http://purl.org/dc/elements/1.1/relation"/>
        <rdfs:subPropertyOf rdf:resource="http://purl.org/dc/terms/relation"/>
    </owl:AnnotationProperty>
    


    <!-- http://purl.org/dc/terms/identifier -->

    <owl:AnnotationProperty rdf:about="http://purl.org/dc/terms/identifier">
        <rdfs:subPropertyOf rdf:resource="http://purl.org/dc/elements/1.1/identifier"/>
    </owl:AnnotationProperty>
    


    <!-- http://purl.org/dc/terms/isFormatOf -->

    <owl:AnnotationProperty rdf:about="http://purl.org/dc/terms/isFormatOf">
        <rdfs:subPropertyOf rdf:resource="http://purl.org/dc/elements/1.1/relation"/>
        <rdfs:subPropertyOf rdf:resource="http://purl.org/dc/terms/relation"/>
    </owl:AnnotationProperty>
    


    <!-- http://purl.org/dc/terms/isPartOf -->

    <owl:AnnotationProperty rdf:about="http://purl.org/dc/terms/isPartOf">
        <rdfs:subPropertyOf rdf:resource="http://purl.org/dc/elements/1.1/relation"/>
        <rdfs:subPropertyOf rdf:resource="http://purl.org/dc/terms/relation"/>
    </owl:AnnotationProperty>
    


    <!-- http://purl.org/dc/terms/isReferencedBy -->

    <owl:AnnotationProperty rdf:about="http://purl.org/dc/terms/isReferencedBy">
        <rdfs:subPropertyOf rdf:resource="http://purl.org/dc/elements/1.1/relation"/>
        <rdfs:subPropertyOf rdf:resource="http://purl.org/dc/terms/relation"/>
    </owl:AnnotationProperty>
    


    <!-- http://purl.org/dc/terms/isReplacedBy -->

    <owl:AnnotationProperty rdf:about="http://purl.org/dc/terms/isReplacedBy">
        <rdfs:subPropertyOf rdf:resource="http://purl.org/dc/elements/1.1/relation"/>
        <rdfs:subPropertyOf rdf:resource="http://purl.org/dc/terms/relation"/>
    </owl:AnnotationProperty>
    


    <!-- http://purl.org/dc/terms/isRequiredBy -->

    <owl:AnnotationProperty rdf:about="http://purl.org/dc/terms/isRequiredBy">
        <rdfs:subPropertyOf rdf:resource="http://purl.org/dc/elements/1.1/relation"/>
        <rdfs:subPropertyOf rdf:resource="http://purl.org/dc/terms/relation"/>
    </owl:AnnotationProperty>
    


    <!-- http://purl.org/dc/terms/isVersionOf -->

    <owl:AnnotationProperty rdf:about="http://purl.org/dc/terms/isVersionOf">
        <rdfs:subPropertyOf rdf:resource="http://purl.org/dc/elements/1.1/relation"/>
        <rdfs:subPropertyOf rdf:resource="http://purl.org/dc/terms/relation"/>
    </owl:AnnotationProperty>
    


    <!-- http://purl.org/dc/terms/issued -->

    <owl:AnnotationProperty rdf:about="http://purl.org/dc/terms/issued">
        <rdfs:subPropertyOf rdf:resource="http://purl.org/dc/elements/1.1/date"/>
    </owl:AnnotationProperty>
    


    <!-- http://purl.org/dc/terms/language -->

    <owl:AnnotationProperty rdf:about="http://purl.org/dc/terms/language">
        <rdfs:subPropertyOf rdf:resource="http://purl.org/dc/elements/1.1/language"/>
    </owl:AnnotationProperty>
    


    <!-- http://purl.org/dc/terms/license -->

    <owl:AnnotationProperty rdf:about="http://purl.org/dc/terms/license">
        <rdfs:subPropertyOf rdf:resource="http://purl.org/dc/elements/1.1/rights"/>
    </owl:AnnotationProperty>
    


    <!-- http://purl.org/dc/terms/medium -->

    <owl:AnnotationProperty rdf:about="http://purl.org/dc/terms/medium">
        <rdfs:subPropertyOf rdf:resource="http://purl.org/dc/elements/1.1/format"/>
    </owl:AnnotationProperty>
    


    <!-- http://purl.org/dc/terms/modified -->

    <owl:AnnotationProperty rdf:about="http://purl.org/dc/terms/modified">
        <rdfs:subPropertyOf rdf:resource="http://purl.org/dc/elements/1.1/date"/>
    </owl:AnnotationProperty>
    


    <!-- http://purl.org/dc/terms/publisher -->

    <owl:AnnotationProperty rdf:about="http://purl.org/dc/terms/publisher">
        <rdfs:subPropertyOf rdf:resource="http://purl.org/dc/elements/1.1/publisher"/>
    </owl:AnnotationProperty>
    


    <!-- http://purl.org/dc/terms/references -->

    <owl:AnnotationProperty rdf:about="http://purl.org/dc/terms/references">
        <rdfs:subPropertyOf rdf:resource="http://purl.org/dc/elements/1.1/relation"/>
        <rdfs:subPropertyOf rdf:resource="http://purl.org/dc/terms/relation"/>
    </owl:AnnotationProperty>
    


    <!-- http://purl.org/dc/terms/relation -->

    <owl:AnnotationProperty rdf:about="http://purl.org/dc/terms/relation">
        <rdfs:subPropertyOf rdf:resource="http://purl.org/dc/elements/1.1/relation"/>
    </owl:AnnotationProperty>
    


    <!-- http://purl.org/dc/terms/replaces -->

    <owl:AnnotationProperty rdf:about="http://purl.org/dc/terms/replaces">
        <rdfs:subPropertyOf rdf:resource="http://purl.org/dc/elements/1.1/relation"/>
        <rdfs:subPropertyOf rdf:resource="http://purl.org/dc/terms/relation"/>
    </owl:AnnotationProperty>
    


    <!-- http://purl.org/dc/terms/requires -->

    <owl:AnnotationProperty rdf:about="http://purl.org/dc/terms/requires">
        <rdfs:subPropertyOf rdf:resource="http://purl.org/dc/elements/1.1/relation"/>
        <rdfs:subPropertyOf rdf:resource="http://purl.org/dc/terms/relation"/>
    </owl:AnnotationProperty>
    


    <!-- http://purl.org/dc/terms/rights -->

    <owl:AnnotationProperty rdf:about="http://purl.org/dc/terms/rights">
        <rdfs:subPropertyOf rdf:resource="http://purl.org/dc/elements/1.1/rights"/>
    </owl:AnnotationProperty>
    


    <!-- http://purl.org/dc/terms/source -->

    <owl:AnnotationProperty rdf:about="http://purl.org/dc/terms/source">
        <rdfs:subPropertyOf rdf:resource="http://purl.org/dc/elements/1.1/source"/>
        <rdfs:subPropertyOf rdf:resource="http://purl.org/dc/terms/relation"/>
    </owl:AnnotationProperty>
    


    <!-- http://purl.org/dc/terms/spatial -->

    <owl:AnnotationProperty rdf:about="http://purl.org/dc/terms/spatial">
        <rdfs:subPropertyOf rdf:resource="http://purl.org/dc/elements/1.1/coverage"/>
    </owl:AnnotationProperty>
    


    <!-- http://purl.org/dc/terms/subject -->

    <owl:AnnotationProperty rdf:about="http://purl.org/dc/terms/subject">
        <rdfs:subPropertyOf rdf:resource="http://purl.org/dc/elements/1.1/subject"/>
    </owl:AnnotationProperty>
    


    <!-- http://purl.org/dc/terms/tableOfContents -->

    <owl:AnnotationProperty rdf:about="http://purl.org/dc/terms/tableOfContents">
        <rdfs:subPropertyOf rdf:resource="http://purl.org/dc/elements/1.1/description"/>
        <rdfs:subPropertyOf rdf:resource="http://purl.org/dc/terms/description"/>
    </owl:AnnotationProperty>
    


    <!-- http://purl.org/dc/terms/temporal -->

    <owl:AnnotationProperty rdf:about="http://purl.org/dc/terms/temporal">
        <rdfs:subPropertyOf rdf:resource="http://purl.org/dc/elements/1.1/coverage"/>
    </owl:AnnotationProperty>
    


    <!-- http://purl.org/dc/terms/title -->

    <owl:AnnotationProperty rdf:about="http://purl.org/dc/terms/title">
        <rdfs:subPropertyOf rdf:resource="http://purl.org/dc/elements/1.1/title"/>
    </owl:AnnotationProperty>
    


    <!-- http://purl.org/dc/terms/type -->

    <owl:AnnotationProperty rdf:about="http://purl.org/dc/terms/type">
        <rdfs:subPropertyOf rdf:resource="http://purl.org/dc/elements/1.1/type"/>
    </owl:AnnotationProperty>
    


    <!-- http://purl.org/dc/terms/valid -->

    <owl:AnnotationProperty rdf:about="http://purl.org/dc/terms/valid">
        <rdfs:subPropertyOf rdf:resource="http://purl.org/dc/elements/1.1/date"/>
    </owl:AnnotationProperty>
    


    <!-- 
    ///////////////////////////////////////////////////////////////////////////////////////
    //
    // Datatypes
    //
    ///////////////////////////////////////////////////////////////////////////////////////
     -->

    


    <!-- http://purl.org/dc/terms/Box -->

    <rdfs:Datatype rdf:about="http://purl.org/dc/terms/Box"/>
    


    <!-- http://purl.org/dc/terms/ISO3166 -->

    <rdfs:Datatype rdf:about="http://purl.org/dc/terms/ISO3166"/>
    


    <!-- http://purl.org/dc/terms/ISO639-2 -->

    <rdfs:Datatype rdf:about="http://purl.org/dc/terms/ISO639-2"/>
    


    <!-- http://purl.org/dc/terms/ISO639-3 -->

    <rdfs:Datatype rdf:about="http://purl.org/dc/terms/ISO639-3"/>
    


    <!-- http://purl.org/dc/terms/Period -->

    <rdfs:Datatype rdf:about="http://purl.org/dc/terms/Period"/>
    


    <!-- http://purl.org/dc/terms/Point -->

    <rdfs:Datatype rdf:about="http://purl.org/dc/terms/Point"/>
    


    <!-- http://purl.org/dc/terms/RFC1766 -->

    <rdfs:Datatype rdf:about="http://purl.org/dc/terms/RFC1766"/>
    


    <!-- http://purl.org/dc/terms/RFC3066 -->

    <rdfs:Datatype rdf:about="http://purl.org/dc/terms/RFC3066"/>
    


    <!-- http://purl.org/dc/terms/RFC4646 -->

    <rdfs:Datatype rdf:about="http://purl.org/dc/terms/RFC4646"/>
    


    <!-- http://purl.org/dc/terms/RFC5646 -->

    <rdfs:Datatype rdf:about="http://purl.org/dc/terms/RFC5646"/>
    


    <!-- http://purl.org/dc/terms/URI -->

    <rdfs:Datatype rdf:about="http://purl.org/dc/terms/URI"/>
    


    <!-- http://purl.org/dc/terms/W3CDTF -->

    <rdfs:Datatype rdf:about="http://purl.org/dc/terms/W3CDTF"/>
    


    <!-- 
    ///////////////////////////////////////////////////////////////////////////////////////
    //
    // Object Properties
    //
    ///////////////////////////////////////////////////////////////////////////////////////
     -->

    


    <!-- http://purl.org/dc/terms/accessRights -->

    <owl:ObjectProperty rdf:about="http://purl.org/dc/terms/accessRights">
        <rdfs:subPropertyOf rdf:resource="http://purl.org/dc/terms/rights"/>
        <rdfs:range rdf:resource="http://purl.org/dc/terms/RightsStatement"/>
    </owl:ObjectProperty>
    


    <!-- http://purl.org/dc/terms/accrualMethod -->

    <owl:ObjectProperty rdf:about="http://purl.org/dc/terms/accrualMethod">
        <rdfs:domain rdf:resource="http://purl.org/dc/dcmitype/Collection"/>
        <rdfs:range rdf:resource="http://purl.org/dc/terms/MethodOfAccrual"/>
    </owl:ObjectProperty>
    


    <!-- http://purl.org/dc/terms/accrualPeriodicity -->

    <owl:ObjectProperty rdf:about="http://purl.org/dc/terms/accrualPeriodicity">
        <rdfs:domain rdf:resource="http://purl.org/dc/dcmitype/Collection"/>
        <rdfs:range rdf:resource="http://purl.org/dc/terms/Frequency"/>
    </owl:ObjectProperty>
    


    <!-- http://purl.org/dc/terms/accrualPolicy -->

    <owl:ObjectProperty rdf:about="http://purl.org/dc/terms/accrualPolicy">
        <rdfs:domain rdf:resource="http://purl.org/dc/dcmitype/Collection"/>
        <rdfs:range rdf:resource="http://purl.org/dc/terms/Policy"/>
    </owl:ObjectProperty>
    


    <!-- http://purl.org/dc/terms/audience -->

    <owl:ObjectProperty rdf:about="http://purl.org/dc/terms/audience">
        <rdfs:range rdf:resource="http://purl.org/dc/terms/AgentClass"/>
    </owl:ObjectProperty>
    


    <!-- http://purl.org/dc/terms/conformsTo -->

    <owl:ObjectProperty rdf:about="http://purl.org/dc/terms/conformsTo">
        <rdfs:range rdf:resource="http://purl.org/dc/terms/Standard"/>
    </owl:ObjectProperty>
    


    <!-- http://purl.org/dc/terms/contributor -->

    <owl:ObjectProperty rdf:about="http://purl.org/dc/terms/contributor">
        <rdfs:range rdf:resource="http://purl.org/dc/terms/Agent"/>
    </owl:ObjectProperty>
    


    <!-- http://purl.org/dc/terms/coverage -->

    <owl:ObjectProperty rdf:about="http://purl.org/dc/terms/coverage">
        <rdfs:range rdf:resource="http://purl.org/dc/terms/LocationPeriodOrJurisdiction"/>
    </owl:ObjectProperty>
    


    <!-- http://purl.org/dc/terms/creator -->

    <owl:ObjectProperty rdf:about="http://purl.org/dc/terms/creator">
        <rdfs:subPropertyOf rdf:resource="http://purl.org/dc/terms/contributor"/>
        <rdfs:range rdf:resource="http://purl.org/dc/terms/Agent"/>
    </owl:ObjectProperty>
    


    <!-- http://purl.org/dc/terms/educationLevel -->

    <owl:ObjectProperty rdf:about="http://purl.org/dc/terms/educationLevel">
        <rdfs:subPropertyOf rdf:resource="http://purl.org/dc/terms/audience"/>
        <rdfs:range rdf:resource="http://purl.org/dc/terms/AgentClass"/>
    </owl:ObjectProperty>
    


    <!-- http://purl.org/dc/terms/extent -->

    <owl:ObjectProperty rdf:about="http://purl.org/dc/terms/extent">
        <rdfs:subPropertyOf rdf:resource="http://purl.org/dc/terms/format"/>
        <rdfs:range rdf:resource="http://purl.org/dc/terms/SizeOrDuration"/>
    </owl:ObjectProperty>
    


    <!-- http://purl.org/dc/terms/format -->

    <owl:ObjectProperty rdf:about="http://purl.org/dc/terms/format">
        <rdfs:range rdf:resource="http://purl.org/dc/terms/MediaTypeOrExtent"/>
    </owl:ObjectProperty>
    


    <!-- http://purl.org/dc/terms/instructionalMethod -->

    <owl:ObjectProperty rdf:about="http://purl.org/dc/terms/instructionalMethod">
        <rdfs:range rdf:resource="http://purl.org/dc/terms/MethodOfInstruction"/>
    </owl:ObjectProperty>
    


    <!-- http://purl.org/dc/terms/language -->

    <owl:ObjectProperty rdf:about="http://purl.org/dc/terms/language">
        <rdfs:range rdf:resource="http://purl.org/dc/terms/LinguisticSystem"/>
    </owl:ObjectProperty>
    


    <!-- http://purl.org/dc/terms/license -->

    <owl:ObjectProperty rdf:about="http://purl.org/dc/terms/license">
        <rdfs:subPropertyOf rdf:resource="http://purl.org/dc/terms/rights"/>
        <rdfs:range rdf:resource="http://purl.org/dc/terms/LicenseDocument"/>
    </owl:ObjectProperty>
    


    <!-- http://purl.org/dc/terms/mediator -->

    <owl:ObjectProperty rdf:about="http://purl.org/dc/terms/mediator">
        <rdfs:subPropertyOf rdf:resource="http://purl.org/dc/terms/audience"/>
        <rdfs:range rdf:resource="http://purl.org/dc/terms/AgentClass"/>
    </owl:ObjectProperty>
    


    <!-- http://purl.org/dc/terms/medium -->

    <owl:ObjectProperty rdf:about="http://purl.org/dc/terms/medium">
        <rdfs:subPropertyOf rdf:resource="http://purl.org/dc/terms/format"/>
        <rdfs:domain rdf:resource="http://purl.org/dc/terms/PhysicalResource"/>
        <rdfs:range rdf:resource="http://purl.org/dc/terms/PhysicalMedium"/>
    </owl:ObjectProperty>
    


    <!-- http://purl.org/dc/terms/provenance -->

    <owl:ObjectProperty rdf:about="http://purl.org/dc/terms/provenance">
        <rdfs:range rdf:resource="http://purl.org/dc/terms/ProvenanceStatement"/>
    </owl:ObjectProperty>
    


    <!-- http://purl.org/dc/terms/publisher -->

    <owl:ObjectProperty rdf:about="http://purl.org/dc/terms/publisher">
        <rdfs:range rdf:resource="http://purl.org/dc/terms/Agent"/>
    </owl:ObjectProperty>
    


    <!-- http://purl.org/dc/terms/rights -->

    <owl:ObjectProperty rdf:about="http://purl.org/dc/terms/rights">
        <rdfs:range rdf:resource="http://purl.org/dc/terms/RightsStatement"/>
    </owl:ObjectProperty>
    


    <!-- http://purl.org/dc/terms/rightsHolder -->

    <owl:ObjectProperty rdf:about="http://purl.org/dc/terms/rightsHolder">
        <rdfs:range rdf:resource="http://purl.org/dc/terms/Agent"/>
    </owl:ObjectProperty>
    


    <!-- http://purl.org/dc/terms/spatial -->

    <owl:ObjectProperty rdf:about="http://purl.org/dc/terms/spatial">
        <rdfs:subPropertyOf rdf:resource="http://purl.org/dc/terms/coverage"/>
        <rdfs:range rdf:resource="http://purl.org/dc/terms/Location"/>
    </owl:ObjectProperty>
    


    <!-- http://purl.org/dc/terms/temporal -->

    <owl:ObjectProperty rdf:about="http://purl.org/dc/terms/temporal">
        <rdfs:subPropertyOf rdf:resource="http://purl.org/dc/terms/coverage"/>
        <rdfs:range rdf:resource="http://purl.org/dc/terms/PeriodOfTime"/>
    </owl:ObjectProperty>
    


    <!-- http://purl.org/dc/terms/type -->

    <owl:ObjectProperty rdf:about="http://purl.org/dc/terms/type">
        <rdfs:range rdf:resource="http://www.w3.org/2000/01/rdf-schema#Class"/>
    </owl:ObjectProperty>
    


    <!-- http://purl.org/ontology/po/actor -->

    <owl:ObjectProperty rdf:about="http://purl.org/ontology/po/actor">
        <rdfs:subPropertyOf rdf:resource="http://purl.org/ontology/po/credit"/>
        <rdfs:domain rdf:resource="http://purl.org/ontology/po/Programme"/>
        <rdfs:range rdf:resource="http://xmlns.com/foaf/0.1/Agent"/>
        <rdfs:comment>Relates a programmes to one of its actors - a person who plays the role of a character</rdfs:comment>
        <rdfs:isDefinedBy rdf:resource="http://purl.org/ontology/po/"/>
        <rdfs:label>actor</rdfs:label>
        <vs:term_status>testing</vs:term_status>
    </owl:ObjectProperty>
    


    <!-- http://purl.org/ontology/po/anchor -->

    <owl:ObjectProperty rdf:about="http://purl.org/ontology/po/anchor">
        <rdfs:subPropertyOf rdf:resource="http://purl.org/ontology/po/credit"/>
        <rdfs:domain rdf:resource="http://purl.org/ontology/po/Programme"/>
        <rdfs:range rdf:resource="http://xmlns.com/foaf/0.1/Agent"/>
        <rdfs:comment>A television reporter who coordinates a programme</rdfs:comment>
        <rdfs:isDefinedBy rdf:resource="http://purl.org/ontology/po/"/>
        <rdfs:label>anchor</rdfs:label>
        <vs:term_status>testing</vs:term_status>
    </owl:ObjectProperty>
    


    <!-- http://purl.org/ontology/po/author -->

    <owl:ObjectProperty rdf:about="http://purl.org/ontology/po/author">
        <rdfs:subPropertyOf rdf:resource="http://purl.org/ontology/po/credit"/>
        <rdfs:domain rdf:resource="http://purl.org/ontology/po/Programme"/>
        <rdfs:range rdf:resource="http://xmlns.com/foaf/0.1/Agent"/>
        <rdfs:comment>Relates a programme to its author - the person who created the content</rdfs:comment>
        <rdfs:isDefinedBy rdf:resource="http://purl.org/ontology/po/"/>
        <rdfs:label>author</rdfs:label>
        <vs:term_status>testing</vs:term_status>
    </owl:ObjectProperty>
    


    <!-- http://purl.org/ontology/po/broadcast_of -->

    <owl:ObjectProperty rdf:about="http://purl.org/ontology/po/broadcast_of">
        <rdfs:subPropertyOf rdf:resource="http://purl.org/NET/c4dm/event.owl#factor"/>
        <rdfs:domain rdf:resource="http://purl.org/ontology/po/Broadcast"/>
        <rdfs:range rdf:resource="http://purl.org/ontology/po/Version"/>
        <rdfs:comment>
		Relates a particular broadcast to the version being broadcasted.
		Sub-property of the event:factor one.
	</rdfs:comment>
        <rdfs:isDefinedBy rdf:resource="http://purl.org/ontology/po/"/>
        <rdfs:label>broadcast of</rdfs:label>
        <vs:term_status>testing</vs:term_status>
    </owl:ObjectProperty>
    


    <!-- http://purl.org/ontology/po/broadcast_on -->

    <owl:ObjectProperty rdf:about="http://purl.org/ontology/po/broadcast_on">
        <owl:equivalentProperty rdf:resource="http://purl.org/ontology/po/broadcasted_on"/>
        <rdfs:subPropertyOf rdf:resource="http://purl.org/NET/c4dm/event.owl#factor"/>
        <rdfs:domain rdf:resource="http://purl.org/ontology/po/Broadcast"/>
        <rdfs:range rdf:resource="http://purl.org/ontology/po/Service"/>
        <rdfs:comment>
		Relates a particular broadcast to the service or outlet on which it was.
		Sub-property of the event:factor one.
	</rdfs:comment>
        <rdfs:isDefinedBy rdf:resource="http://purl.org/ontology/po/"/>
        <rdfs:label>broadcast on</rdfs:label>
        <vs:term_status>testing</vs:term_status>
    </owl:ObjectProperty>
    


    <!-- http://purl.org/ontology/po/broadcasted_on -->

    <owl:ObjectProperty rdf:about="http://purl.org/ontology/po/broadcasted_on">
        <rdfs:comment>Deprecated property, left here for historical reasons</rdfs:comment>
    </owl:ObjectProperty>
    


    <!-- http://purl.org/ontology/po/broadcaster -->

    <owl:ObjectProperty rdf:about="http://purl.org/ontology/po/broadcaster">
        <rdfs:domain rdf:resource="http://purl.org/ontology/po/Service"/>
        <rdfs:range rdf:resource="http://purl.org/ontology/po/Broadcaster"/>
        <rdfs:comment>
		Associates a service to a broadcaster
	</rdfs:comment>
        <rdfs:isDefinedBy rdf:resource="http://purl.org/ontology/po/"/>
        <rdfs:label>broadcaster</rdfs:label>
        <vs:term_status>testing</vs:term_status>
    </owl:ObjectProperty>
    


    <!-- http://purl.org/ontology/po/category -->

    <owl:ObjectProperty rdf:about="http://purl.org/ontology/po/category">
        <rdfs:domain rdf:resource="http://purl.org/ontology/po/Programme"/>
        <rdfs:range rdf:resource="http://purl.org/ontology/po/Genre"/>
        <rdfs:comment>
        Relates a programme to a particular category, e.g. genre, format, place...
    </rdfs:comment>
        <rdfs:isDefinedBy rdf:resource="http://purl.org/ontology/po/"/>
        <rdfs:label>category</rdfs:label>
        <vs:term_status>testing</vs:term_status>
    </owl:ObjectProperty>
    


    <!-- http://purl.org/ontology/po/channel -->

    <owl:ObjectProperty rdf:about="http://purl.org/ontology/po/channel">
        <rdfs:domain rdf:resource="http://purl.org/ontology/po/Service"/>
        <rdfs:range rdf:resource="http://purl.org/ontology/po/Channel"/>
        <rdfs:comment>
        Associates a service to a channel, e.g. Radio 4 LW to Radio 4 LW on Analogue Long Wave.
    </rdfs:comment>
        <rdfs:isDefinedBy rdf:resource="http://purl.org/ontology/po/"/>
        <rdfs:label>channel</rdfs:label>
        <vs:term_status>testing</vs:term_status>
    </owl:ObjectProperty>
    


    <!-- http://purl.org/ontology/po/clip -->

    <owl:ObjectProperty rdf:about="http://purl.org/ontology/po/clip">
        <rdfs:subPropertyOf rdf:resource="http://purl.org/dc/terms/hasPart"/>
        <rdfs:range rdf:resource="http://purl.org/ontology/po/Clip"/>
        <rdfs:comment>
        Associates a brand, a series or an episode to a clip.
    </rdfs:comment>
        <rdfs:isDefinedBy rdf:resource="http://purl.org/ontology/po/"/>
        <rdfs:label>clip</rdfs:label>
        <vs:term_status>testing</vs:term_status>
    </owl:ObjectProperty>
    


    <!-- http://purl.org/ontology/po/commentator -->

    <owl:ObjectProperty rdf:about="http://purl.org/ontology/po/commentator">
        <rdfs:subPropertyOf rdf:resource="http://purl.org/ontology/po/credit"/>
        <rdfs:domain rdf:resource="http://purl.org/ontology/po/Programme"/>
        <rdfs:range rdf:resource="http://xmlns.com/foaf/0.1/Agent"/>
        <rdfs:comment>Relates a programme to one of its commentators</rdfs:comment>
        <rdfs:isDefinedBy rdf:resource="http://purl.org/ontology/po/"/>
        <rdfs:label>commentator</rdfs:label>
        <vs:term_status>testing</vs:term_status>
    </owl:ObjectProperty>
    


    <!-- http://purl.org/ontology/po/credit -->

    <owl:ObjectProperty rdf:about="http://purl.org/ontology/po/credit">
        <rdfs:subPropertyOf rdf:resource="http://purl.org/dc/elements/1.1/contributor"/>
        <rdfs:domain rdf:resource="http://purl.org/ontology/po/Programme"/>
        <rdfs:range rdf:resource="http://xmlns.com/foaf/0.1/Agent"/>
        <rdfs:comment>Relates a programmes to a person who is credited in it</rdfs:comment>
        <rdfs:isDefinedBy rdf:resource="http://purl.org/ontology/po/"/>
        <rdfs:label>credit</rdfs:label>
        <vs:term_status>testing</vs:term_status>
    </owl:ObjectProperty>
    


    <!-- http://purl.org/ontology/po/director -->

    <owl:ObjectProperty rdf:about="http://purl.org/ontology/po/director">
        <rdfs:subPropertyOf rdf:resource="http://purl.org/ontology/po/credit"/>
        <rdfs:domain rdf:resource="http://purl.org/ontology/po/Programme"/>
        <rdfs:range rdf:resource="http://xmlns.com/foaf/0.1/Agent"/>
        <rdfs:comment>Relates a programme to its supervisor. Generally refers to the person responsible for all audience-visible components of a program, film, or show, whereas the producer is responsible for the financial and other behind-the-scenes aspects. A director&apos;s duties might also include casting, script editing, shot selection, shot composition, and editing</rdfs:comment>
        <rdfs:isDefinedBy rdf:resource="http://purl.org/ontology/po/"/>
        <rdfs:label>director</rdfs:label>
        <vs:term_status>testing</vs:term_status>
    </owl:ObjectProperty>
    


    <!-- http://purl.org/ontology/po/episode -->

    <owl:ObjectProperty rdf:about="http://purl.org/ontology/po/episode">
        <rdfs:subPropertyOf rdf:resource="http://purl.org/dc/terms/hasPart"/>
        <rdfs:range rdf:resource="http://purl.org/ontology/po/Episode"/>
        <rdfs:comment>
		Associates a brand or a series to an episode constituting it.
	</rdfs:comment>
        <rdfs:isDefinedBy rdf:resource="http://purl.org/ontology/po/"/>
        <rdfs:label>episode</rdfs:label>
        <vs:term_status>testing</vs:term_status>
    </owl:ObjectProperty>
    


    <!-- http://purl.org/ontology/po/executive_producer -->

    <owl:ObjectProperty rdf:about="http://purl.org/ontology/po/executive_producer">
        <rdfs:subPropertyOf rdf:resource="http://purl.org/ontology/po/credit"/>
        <rdfs:domain rdf:resource="http://purl.org/ontology/po/Programme"/>
        <rdfs:range rdf:resource="http://xmlns.com/foaf/0.1/Agent"/>
        <rdfs:comment>Relates a programme to its executive producer - a producer who is not involved in any technical aspects of the making process, but who is still responsible for the overall production. Typically an executive producer handles business and legal issues</rdfs:comment>
        <rdfs:isDefinedBy rdf:resource="http://purl.org/ontology/po/"/>
        <rdfs:label>executive producer</rdfs:label>
        <vs:term_status>testing</vs:term_status>
    </owl:ObjectProperty>
    


    <!-- http://purl.org/ontology/po/format -->

    <owl:ObjectProperty rdf:about="http://purl.org/ontology/po/format">
        <rdfs:subPropertyOf rdf:resource="http://purl.org/ontology/po/category"/>
        <rdfs:domain rdf:resource="http://purl.org/ontology/po/Programme"/>
        <rdfs:range rdf:resource="http://purl.org/ontology/po/Format"/>
        <rdfs:comment>
		Relates a programme to a particular format (eg. `Animation&apos;, `Documentary&apos;, etc.).
	</rdfs:comment>
        <rdfs:isDefinedBy rdf:resource="http://purl.org/ontology/po/"/>
        <rdfs:label>format</rdfs:label>
        <vs:term_status>testing</vs:term_status>
    </owl:ObjectProperty>
    


    <!-- http://purl.org/ontology/po/genre -->

    <owl:ObjectProperty rdf:about="http://purl.org/ontology/po/genre">
        <rdfs:subPropertyOf rdf:resource="http://purl.org/ontology/po/category"/>
        <rdfs:domain rdf:resource="http://purl.org/ontology/po/Programme"/>
        <rdfs:range rdf:resource="http://purl.org/ontology/po/Genre"/>
        <rdfs:comment>
		Relates a programme to a particular genre.
	</rdfs:comment>
        <rdfs:isDefinedBy rdf:resource="http://purl.org/ontology/po/"/>
        <rdfs:label>genre</rdfs:label>
        <vs:term_status>testing</vs:term_status>
    </owl:ObjectProperty>
    


    <!-- http://purl.org/ontology/po/location -->

    <owl:ObjectProperty rdf:about="http://purl.org/ontology/po/location">
        <rdfs:subPropertyOf rdf:resource="http://xmlns.com/foaf/0.1/based_near"/>
        <rdfs:domain rdf:resource="http://purl.org/ontology/po/Service"/>
        <rdfs:range rdf:resource="http://www.w3.org/2003/01/geo/wgs84_pos#SpatialThing"/>
        <rdfs:comment>
		Associates a service to a geographic location,
		aiming at capturing what this service aims at covering.
	</rdfs:comment>
        <rdfs:isDefinedBy rdf:resource="http://purl.org/ontology/po/"/>
        <rdfs:label>location</rdfs:label>
        <vs:term_status>testing</vs:term_status>
    </owl:ObjectProperty>
    


    <!-- http://purl.org/ontology/po/masterbrand -->

    <owl:ObjectProperty rdf:about="http://purl.org/ontology/po/masterbrand">
        <rdfs:domain rdf:resource="http://purl.org/ontology/po/Programme"/>
        <rdfs:range rdf:resource="http://purl.org/ontology/po/Service"/>
        <rdfs:comment>Associates a programme with its masterbrand (its commissioner)</rdfs:comment>
        <rdfs:isDefinedBy rdf:resource="http://purl.org/ontology/po/"/>
        <rdfs:label>masterbrand</rdfs:label>
        <vs:term_status>stable</vs:term_status>
    </owl:ObjectProperty>
    


    <!-- http://purl.org/ontology/po/microsite -->

    <owl:ObjectProperty rdf:about="http://purl.org/ontology/po/microsite">
        <rdfs:subPropertyOf rdf:resource="http://xmlns.com/foaf/0.1/page"/>
        <rdfs:domain rdf:resource="http://purl.org/ontology/po/Programme"/>
        <rdfs:range rdf:resource="http://xmlns.com/foaf/0.1/Document"/>
        <rdfs:comment>Associates a programme to its microsite. For example http://www.bbc.co.uk/programmes/b00fm04s and http://www.bbc.co.uk/eastenders/</rdfs:comment>
        <rdfs:isDefinedBy rdf:resource="http://purl.org/ontology/po/"/>
        <rdfs:label>microsite</rdfs:label>
        <vs:term_status>testing</vs:term_status>
    </owl:ObjectProperty>
    


    <!-- http://purl.org/ontology/po/news_reader -->

    <owl:ObjectProperty rdf:about="http://purl.org/ontology/po/news_reader">
        <rdfs:subPropertyOf rdf:resource="http://purl.org/ontology/po/credit"/>
        <rdfs:domain rdf:resource="http://purl.org/ontology/po/Programme"/>
        <rdfs:range rdf:resource="http://xmlns.com/foaf/0.1/Agent"/>
        <rdfs:comment>Relates a programme to its news reader</rdfs:comment>
        <rdfs:isDefinedBy rdf:resource="http://purl.org/ontology/po/"/>
        <rdfs:label>news reader</rdfs:label>
        <vs:term_status>testing</vs:term_status>
    </owl:ObjectProperty>
    


    <!-- http://purl.org/ontology/po/outlet -->

    <owl:ObjectProperty rdf:about="http://purl.org/ontology/po/outlet">
        <rdfs:domain rdf:resource="http://purl.org/ontology/po/Service"/>
        <rdfs:range rdf:resource="http://purl.org/ontology/po/Outlet"/>
        <rdfs:comment>
		Associates a service to an outlet, e.g. Radio 4 to Radio 4 LW.
	</rdfs:comment>
        <rdfs:isDefinedBy rdf:resource="http://purl.org/ontology/po/"/>
        <rdfs:label>outlet</rdfs:label>
        <vs:term_status>testing</vs:term_status>
    </owl:ObjectProperty>
    


    <!-- http://purl.org/ontology/po/parent_series -->

    <owl:ObjectProperty rdf:about="http://purl.org/ontology/po/parent_series">
        <rdfs:subPropertyOf rdf:resource="http://purl.org/dc/terms/isPartOf"/>
        <rdf:type rdf:resource="http://www.w3.org/2002/07/owl#TransitiveProperty"/>
        <rdfs:domain rdf:resource="http://purl.org/ontology/po/Series"/>
        <rdfs:range rdf:resource="http://purl.org/ontology/po/Series"/>
        <rdfs:comment>
		Relates a series to a series constituting it (eg. `Waking the dead&apos;).
	</rdfs:comment>
        <rdfs:isDefinedBy rdf:resource="http://purl.org/ontology/po/"/>
        <rdfs:label>parent series</rdfs:label>
        <vs:term_status>testing</vs:term_status>
    </owl:ObjectProperty>
    


    <!-- http://purl.org/ontology/po/parent_service -->

    <owl:ObjectProperty rdf:about="http://purl.org/ontology/po/parent_service">
        <rdfs:subPropertyOf rdf:resource="http://purl.org/dc/terms/isPartOf"/>
        <rdf:type rdf:resource="http://www.w3.org/2002/07/owl#TransitiveProperty"/>
        <rdfs:domain rdf:resource="http://purl.org/ontology/po/Service"/>
        <rdfs:range rdf:resource="http://purl.org/ontology/po/Service"/>
        <rdfs:comment>
		Relates a service to another service encapsulating it (eg. `BBC One&apos; and `BBC One South&apos;)
	</rdfs:comment>
        <rdfs:isDefinedBy rdf:resource="http://purl.org/ontology/po/"/>
        <rdfs:label>parent service</rdfs:label>
        <vs:term_status>testing</vs:term_status>
    </owl:ObjectProperty>
    


    <!-- http://purl.org/ontology/po/participant -->

    <owl:ObjectProperty rdf:about="http://purl.org/ontology/po/participant">
        <rdfs:subPropertyOf rdf:resource="http://purl.org/ontology/po/credit"/>
        <rdfs:domain rdf:resource="http://purl.org/ontology/po/Programme"/>
        <rdfs:range rdf:resource="http://xmlns.com/foaf/0.1/Agent"/>
        <rdfs:comment>Relates a programme to one of its participants</rdfs:comment>
        <rdfs:isDefinedBy rdf:resource="http://purl.org/ontology/po/"/>
        <rdfs:label>participant</rdfs:label>
        <vs:term_status>testing</vs:term_status>
    </owl:ObjectProperty>
    


    <!-- http://purl.org/ontology/po/performer -->

    <owl:ObjectProperty rdf:about="http://purl.org/ontology/po/performer">
        <rdfs:subPropertyOf rdf:resource="http://purl.org/ontology/po/credit"/>
        <rdfs:domain rdf:resource="http://purl.org/ontology/po/Programme"/>
        <rdfs:range rdf:resource="http://xmlns.com/foaf/0.1/Agent"/>
        <rdfs:comment>Relates a programme to an entertainer who performs a dramatic or musical work for audience</rdfs:comment>
        <rdfs:isDefinedBy rdf:resource="http://purl.org/ontology/po/"/>
        <rdfs:label>performer</rdfs:label>
        <vs:term_status>testing</vs:term_status>
    </owl:ObjectProperty>
    


    <!-- http://purl.org/ontology/po/person -->

    <owl:ObjectProperty rdf:about="http://purl.org/ontology/po/person">
        <rdfs:subPropertyOf rdf:resource="http://purl.org/ontology/po/category"/>
        <rdfs:domain rdf:resource="http://purl.org/ontology/po/Programme"/>
        <rdfs:range rdf:resource="http://purl.org/ontology/po/Person"/>
        <rdfs:comment>
        Relates a programme to a person
    </rdfs:comment>
        <rdfs:isDefinedBy rdf:resource="http://purl.org/ontology/po/"/>
        <rdfs:label>person</rdfs:label>
        <vs:term_status>testing</vs:term_status>
    </owl:ObjectProperty>
    


    <!-- http://purl.org/ontology/po/place -->

    <owl:ObjectProperty rdf:about="http://purl.org/ontology/po/place">
        <rdfs:subPropertyOf rdf:resource="http://purl.org/ontology/po/category"/>
        <rdfs:domain rdf:resource="http://purl.org/ontology/po/Programme"/>
        <rdfs:range rdf:resource="http://purl.org/ontology/po/Place"/>
        <rdfs:comment>
        Relates a programme to a place (e.g. `London&apos;)
    </rdfs:comment>
        <rdfs:isDefinedBy rdf:resource="http://purl.org/ontology/po/"/>
        <rdfs:label>place</rdfs:label>
        <vs:term_status>testing</vs:term_status>
    </owl:ObjectProperty>
    


    <!-- http://purl.org/ontology/po/producer -->

    <owl:ObjectProperty rdf:about="http://purl.org/ontology/po/producer">
        <rdfs:subPropertyOf rdf:resource="http://purl.org/ontology/po/credit"/>
        <rdfs:domain rdf:resource="http://purl.org/ontology/po/Programme"/>
        <rdfs:range rdf:resource="http://xmlns.com/foaf/0.1/Agent"/>
        <rdfs:comment>Relates a programme to its producer - the manager of an event, show, or other work, usually the individual in charge of finance, personnel, and other non-artistic aspects in the development of commercials, plays, movies, and other works</rdfs:comment>
        <rdfs:isDefinedBy rdf:resource="http://purl.org/ontology/po/"/>
        <rdfs:label>producer</rdfs:label>
        <vs:term_status>testing</vs:term_status>
    </owl:ObjectProperty>
    


    <!-- http://purl.org/ontology/po/season_broadcast -->

    <owl:ObjectProperty rdf:about="http://purl.org/ontology/po/season_broadcast">
        <rdfs:domain rdf:resource="http://purl.org/ontology/po/Season"/>
        <rdfs:range rdf:resource="http://purl.org/ontology/po/Broadcast"/>
        <rdfs:comment>Associates a season to its constituent broadcasts</rdfs:comment>
        <rdfs:isDefinedBy rdf:resource="http://purl.org/ontology/po/"/>
        <rdfs:label>broadcast</rdfs:label>
        <vs:term_status>testing</vs:term_status>
    </owl:ObjectProperty>
    


    <!-- http://purl.org/ontology/po/series -->

    <owl:ObjectProperty rdf:about="http://purl.org/ontology/po/series">
        <rdfs:subPropertyOf rdf:resource="http://purl.org/dc/terms/hasPart"/>
        <rdf:type rdf:resource="http://www.w3.org/2002/07/owl#TransitiveProperty"/>
        <rdfs:range rdf:resource="http://purl.org/ontology/po/Series"/>
        <rdfs:comment>
		Associates a brand or a series to a series constituting it.
	</rdfs:comment>
        <rdfs:isDefinedBy rdf:resource="http://purl.org/ontology/po/"/>
        <rdfs:label>series</rdfs:label>
        <vs:term_status>testing</vs:term_status>
    </owl:ObjectProperty>
    


    <!-- http://purl.org/ontology/po/service -->

    <owl:ObjectProperty rdf:about="http://purl.org/ontology/po/service">
        <rdf:type rdf:resource="http://www.w3.org/2002/07/owl#FunctionalProperty"/>
        <rdfs:domain rdf:resource="http://purl.org/ontology/po/Programme"/>
        <rdfs:range rdf:resource="http://purl.org/ontology/po/Service"/>
        <rdfs:comment>
		Associate a brand, series or episode to the master brand service.
	</rdfs:comment>
        <rdfs:isDefinedBy rdf:resource="http://purl.org/ontology/po/"/>
        <rdfs:label>service</rdfs:label>
        <vs:term_status>testing</vs:term_status>
    </owl:ObjectProperty>
    


    <!-- http://purl.org/ontology/po/subject -->

    <owl:ObjectProperty rdf:about="http://purl.org/ontology/po/subject">
        <rdfs:subPropertyOf rdf:resource="http://purl.org/ontology/po/category"/>
        <rdfs:domain rdf:resource="http://purl.org/ontology/po/Programme"/>
        <rdfs:range rdf:resource="http://purl.org/ontology/po/Subject"/>
        <rdfs:comment>
        Relates a programme to a subject (e.g. `Easter&apos;)
    </rdfs:comment>
        <rdfs:isDefinedBy rdf:resource="http://purl.org/ontology/po/"/>
        <rdfs:label>subject</rdfs:label>
        <vs:term_status>testing</vs:term_status>
    </owl:ObjectProperty>
    


    <!-- http://purl.org/ontology/po/time -->

    <owl:ObjectProperty rdf:about="http://purl.org/ontology/po/time">
        <rdfs:range rdf:resource="http://purl.org/NET/c4dm/timeline.owl#Interval"/>
        <rdfs:comment>Associates an episode&apos;s version or a version&apos;s segment with a temporal interval. This interval can be associated with a timeline, serving as an anchor for further temporal annotations, e.g. subtitles or played track</rdfs:comment>
        <rdfs:isDefinedBy rdf:resource="http://purl.org/ontology/po/"/>
        <rdfs:label>time</rdfs:label>
        <vs:term_status>stable</vs:term_status>
    </owl:ObjectProperty>
    


    <!-- http://purl.org/ontology/po/track -->

    <owl:ObjectProperty rdf:about="http://purl.org/ontology/po/track">
        <rdfs:subPropertyOf rdf:resource="http://purl.org/NET/c4dm/event.owl#factor"/>
        <rdfs:domain rdf:resource="http://purl.org/ontology/po/MusicSegment"/>
        <rdfs:range rdf:resource="http://purl.org/ontology/mo/Track"/>
        <rdfs:comment>Associates a music segment with a track, as defined in MO</rdfs:comment>
        <rdfs:isDefinedBy rdf:resource="http://purl.org/ontology/po/"/>
        <rdfs:label>track</rdfs:label>
        <vs:term_status>testing</vs:term_status>
    </owl:ObjectProperty>
    


    <!-- http://purl.org/ontology/po/version -->

    <owl:ObjectProperty rdf:about="http://purl.org/ontology/po/version">
        <rdf:type rdf:resource="http://www.w3.org/2002/07/owl#InverseFunctionalProperty"/>
        <rdfs:domain rdf:resource="http://purl.org/ontology/po/ProgrammeItem"/>
        <rdfs:range rdf:resource="http://purl.org/ontology/po/Version"/>
        <rdfs:comment>
		Associate an episode to a version of it.
		Different versions of a same episode can exist (shortened version, version
		designed for the hearing impaired, etc.).
	</rdfs:comment>
        <rdfs:isDefinedBy rdf:resource="http://purl.org/ontology/po/"/>
        <rdfs:label>version</rdfs:label>
        <vs:term_status>testing</vs:term_status>
    </owl:ObjectProperty>
    


    <!-- http://xmlns.com/foaf/0.1/based_near -->

    <owl:ObjectProperty rdf:about="http://xmlns.com/foaf/0.1/based_near"/>
    


    <!-- http://xmlns.com/foaf/0.1/page -->

    <owl:ObjectProperty rdf:about="http://xmlns.com/foaf/0.1/page"/>
    


    <!-- 
    ///////////////////////////////////////////////////////////////////////////////////////
    //
    // Data properties
    //
    ///////////////////////////////////////////////////////////////////////////////////////
     -->

    


    <!-- http://purl.org/dc/terms/alternative -->

    <owl:DatatypeProperty rdf:about="http://purl.org/dc/terms/alternative">
        <rdfs:subPropertyOf rdf:resource="http://purl.org/dc/terms/title"/>
        <rdfs:range rdf:resource="http://www.w3.org/2000/01/rdf-schema#Literal"/>
    </owl:DatatypeProperty>
    


    <!-- http://purl.org/dc/terms/available -->

    <owl:DatatypeProperty rdf:about="http://purl.org/dc/terms/available">
        <rdfs:subPropertyOf rdf:resource="http://purl.org/dc/terms/date"/>
        <rdfs:range rdf:resource="http://www.w3.org/2000/01/rdf-schema#Literal"/>
    </owl:DatatypeProperty>
    


    <!-- http://purl.org/dc/terms/bibliographicCitation -->

    <owl:DatatypeProperty rdf:about="http://purl.org/dc/terms/bibliographicCitation">
        <rdfs:subPropertyOf rdf:resource="http://purl.org/dc/terms/identifier"/>
        <rdfs:domain rdf:resource="http://purl.org/dc/terms/BibliographicResource"/>
        <rdfs:range rdf:resource="http://www.w3.org/2000/01/rdf-schema#Literal"/>
    </owl:DatatypeProperty>
    


    <!-- http://purl.org/dc/terms/created -->

    <owl:DatatypeProperty rdf:about="http://purl.org/dc/terms/created">
        <rdfs:subPropertyOf rdf:resource="http://purl.org/dc/terms/date"/>
        <rdfs:range rdf:resource="http://www.w3.org/2000/01/rdf-schema#Literal"/>
    </owl:DatatypeProperty>
    


    <!-- http://purl.org/dc/terms/date -->

    <owl:DatatypeProperty rdf:about="http://purl.org/dc/terms/date">
        <rdfs:range rdf:resource="http://www.w3.org/2000/01/rdf-schema#Literal"/>
    </owl:DatatypeProperty>
    


    <!-- http://purl.org/dc/terms/dateAccepted -->

    <owl:DatatypeProperty rdf:about="http://purl.org/dc/terms/dateAccepted">
        <rdfs:subPropertyOf rdf:resource="http://purl.org/dc/terms/date"/>
        <rdfs:range rdf:resource="http://www.w3.org/2000/01/rdf-schema#Literal"/>
    </owl:DatatypeProperty>
    


    <!-- http://purl.org/dc/terms/dateCopyrighted -->

    <owl:DatatypeProperty rdf:about="http://purl.org/dc/terms/dateCopyrighted">
        <rdfs:subPropertyOf rdf:resource="http://purl.org/dc/terms/date"/>
        <rdfs:range rdf:resource="http://www.w3.org/2000/01/rdf-schema#Literal"/>
    </owl:DatatypeProperty>
    


    <!-- http://purl.org/dc/terms/dateSubmitted -->

    <owl:DatatypeProperty rdf:about="http://purl.org/dc/terms/dateSubmitted">
        <rdfs:subPropertyOf rdf:resource="http://purl.org/dc/terms/date"/>
        <rdfs:range rdf:resource="http://www.w3.org/2000/01/rdf-schema#Literal"/>
    </owl:DatatypeProperty>
    


    <!-- http://purl.org/dc/terms/identifier -->

    <owl:DatatypeProperty rdf:about="http://purl.org/dc/terms/identifier">
        <rdfs:range rdf:resource="http://www.w3.org/2000/01/rdf-schema#Literal"/>
    </owl:DatatypeProperty>
    


    <!-- http://purl.org/dc/terms/issued -->

    <owl:DatatypeProperty rdf:about="http://purl.org/dc/terms/issued">
        <rdfs:subPropertyOf rdf:resource="http://purl.org/dc/terms/date"/>
        <rdfs:range rdf:resource="http://www.w3.org/2000/01/rdf-schema#Literal"/>
    </owl:DatatypeProperty>
    


    <!-- http://purl.org/dc/terms/modified -->

    <owl:DatatypeProperty rdf:about="http://purl.org/dc/terms/modified">
        <rdfs:subPropertyOf rdf:resource="http://purl.org/dc/terms/date"/>
        <rdfs:range rdf:resource="http://www.w3.org/2000/01/rdf-schema#Literal"/>
    </owl:DatatypeProperty>
    


    <!-- http://purl.org/dc/terms/title -->

    <owl:DatatypeProperty rdf:about="http://purl.org/dc/terms/title">
        <rdfs:range rdf:resource="http://www.w3.org/2000/01/rdf-schema#Literal"/>
    </owl:DatatypeProperty>
    


    <!-- http://purl.org/dc/terms/valid -->

    <owl:DatatypeProperty rdf:about="http://purl.org/dc/terms/valid">
        <rdfs:subPropertyOf rdf:resource="http://purl.org/dc/terms/date"/>
        <rdfs:range rdf:resource="http://www.w3.org/2000/01/rdf-schema#Literal"/>
    </owl:DatatypeProperty>
    


    <!-- http://purl.org/ontology/po/aspect_ratio -->

    <owl:DatatypeProperty rdf:about="http://purl.org/ontology/po/aspect_ratio">
        <rdfs:domain rdf:resource="http://purl.org/ontology/po/Version"/>
        <rdfs:range rdf:resource="http://www.w3.org/2001/XMLSchema#string"/>
        <rdfs:comment>
		The aspect ration of a particular version.
	</rdfs:comment>
        <rdfs:isDefinedBy rdf:resource="http://purl.org/ontology/po/"/>
        <rdfs:label>aspect ratio</rdfs:label>
        <vs:term_status>testing</vs:term_status>
    </owl:DatatypeProperty>
    


    <!-- http://purl.org/ontology/po/duration -->

    <owl:DatatypeProperty rdf:about="http://purl.org/ontology/po/duration">
        <rdfs:range rdf:resource="http://www.w3.org/2001/XMLSchema#int"/>
        <rdfs:comment>The duration of a version, in seconds.</rdfs:comment>
        <rdfs:isDefinedBy rdf:resource="http://purl.org/ontology/po/"/>
        <rdfs:label>duration</rdfs:label>
        <vs:term_status>testing</vs:term_status>
    </owl:DatatypeProperty>
    


    <!-- http://purl.org/ontology/po/frequency -->

    <owl:DatatypeProperty rdf:about="http://purl.org/ontology/po/frequency">
        <rdfs:domain rdf:resource="http://purl.org/ontology/po/Channel"/>
        <rdfs:range rdf:resource="http://www.w3.org/2001/XMLSchema#float"/>
        <rdfs:comment>Associates a channel to its frequency</rdfs:comment>
        <rdfs:isDefinedBy rdf:resource="http://purl.org/ontology/po/"/>
        <rdfs:label>frequency</rdfs:label>
        <vs:term_status>testing</vs:term_status>
    </owl:DatatypeProperty>
    


    <!-- http://purl.org/ontology/po/long_synopsis -->

    <owl:DatatypeProperty rdf:about="http://purl.org/ontology/po/long_synopsis">
        <rdfs:subPropertyOf rdf:resource="http://purl.org/ontology/po/synopsis"/>
        <rdfs:comment>
		A long synopsis of a series, brand or episode.
		Sub-property of po:synopsis.
	</rdfs:comment>
        <rdfs:isDefinedBy rdf:resource="http://purl.org/ontology/po/"/>
        <rdfs:label>long synopsis</rdfs:label>
        <vs:term_status>testing</vs:term_status>
    </owl:DatatypeProperty>
    


    <!-- http://purl.org/ontology/po/medium_synopsis -->

    <owl:DatatypeProperty rdf:about="http://purl.org/ontology/po/medium_synopsis">
        <rdfs:subPropertyOf rdf:resource="http://purl.org/ontology/po/synopsis"/>
        <rdfs:comment>
		A medium synopsis of a series, brand or episode.
		Sub-property of po:synopsis.
	</rdfs:comment>
        <rdfs:isDefinedBy rdf:resource="http://purl.org/ontology/po/"/>
        <rdfs:label>medium synopsis</rdfs:label>
        <vs:term_status>testing</vs:term_status>
    </owl:DatatypeProperty>
    


    <!-- http://purl.org/ontology/po/position -->

    <owl:DatatypeProperty rdf:about="http://purl.org/ontology/po/position">
        <rdfs:range rdf:resource="http://www.w3.org/2001/XMLSchema#int"/>
        <rdfs:comment>The position of a particular series or episode within its containing programme. This property can also be used to give the position of an interval within the containing timeline.</rdfs:comment>
        <rdfs:isDefinedBy rdf:resource="http://purl.org/ontology/po/"/>
        <rdfs:label>position</rdfs:label>
        <vs:term_status>testing</vs:term_status>
    </owl:DatatypeProperty>
    


    <!-- http://purl.org/ontology/po/schedule_date -->

    <owl:DatatypeProperty rdf:about="http://purl.org/ontology/po/schedule_date">
        <rdfs:domain rdf:resource="http://purl.org/ontology/po/Broadcast"/>
        <rdfs:range rdf:resource="http://www.w3.org/2001/XMLSchema#date"/>
        <rdfs:comment>
		The schedule date of a broadcast event.
	</rdfs:comment>
        <rdfs:isDefinedBy rdf:resource="http://purl.org/ontology/po/"/>
        <rdfs:label>schedule date</rdfs:label>
        <vs:term_status>testing</vs:term_status>
    </owl:DatatypeProperty>
    


    <!-- http://purl.org/ontology/po/short_synopsis -->

    <owl:DatatypeProperty rdf:about="http://purl.org/ontology/po/short_synopsis">
        <rdfs:subPropertyOf rdf:resource="http://purl.org/ontology/po/synopsis"/>
        <rdfs:comment>
		A short synopsis of a series, brand or episode.
		Sub-property of po:synopsis.
	</rdfs:comment>
        <rdfs:isDefinedBy rdf:resource="http://purl.org/ontology/po/"/>
        <rdfs:label>short synopsis</rdfs:label>
        <vs:term_status>testing</vs:term_status>
    </owl:DatatypeProperty>
    


    <!-- http://purl.org/ontology/po/sound_format -->

    <owl:DatatypeProperty rdf:about="http://purl.org/ontology/po/sound_format">
        <rdfs:domain rdf:resource="http://purl.org/ontology/po/Version"/>
        <rdfs:range rdf:resource="http://www.w3.org/2001/XMLSchema#string"/>
        <rdfs:comment>
		The sound format of a particular version.
	</rdfs:comment>
        <rdfs:isDefinedBy rdf:resource="http://purl.org/ontology/po/"/>
        <rdfs:label>sound format</rdfs:label>
        <vs:term_status>testing</vs:term_status>
    </owl:DatatypeProperty>
    


    <!-- http://purl.org/ontology/po/subtitle_language -->

    <owl:DatatypeProperty rdf:about="http://purl.org/ontology/po/subtitle_language">
        <rdfs:domain rdf:resource="http://purl.org/ontology/po/Version"/>
        <rdfs:range rdf:resource="http://www.w3.org/2001/XMLSchema#string"/>
        <rdfs:comment>Language of the subtitles embedded in a particular version</rdfs:comment>
        <rdfs:isDefinedBy rdf:resource="http://purl.org/ontology/po/"/>
        <rdfs:label>subtitle language</rdfs:label>
        <vs:term_status>testing</vs:term_status>
    </owl:DatatypeProperty>
    


    <!-- http://purl.org/ontology/po/synopsis -->

    <owl:DatatypeProperty rdf:about="http://purl.org/ontology/po/synopsis">
        <rdfs:domain rdf:resource="http://purl.org/ontology/po/Programme"/>
        <rdfs:range rdf:resource="http://www.w3.org/2001/XMLSchema#string"/>
        <rdfs:comment>
		The synopsis of a series, brand or episode.
	</rdfs:comment>
        <rdfs:isDefinedBy rdf:resource="http://purl.org/ontology/po/"/>
        <rdfs:label>synopsis</rdfs:label>
        <vs:term_status>testing</vs:term_status>
    </owl:DatatypeProperty>
    


    <!-- http://purl.org/ontology/po/text -->

    <owl:DatatypeProperty rdf:about="http://purl.org/ontology/po/text">
        <rdfs:domain rdf:resource="http://purl.org/ontology/po/Subtitle"/>
        <rdfs:range rdf:resource="http://www.w3.org/2001/XMLSchema#string"/>
        <rdfs:comment>Associates a subtitle event to the corresponding text</rdfs:comment>
        <rdfs:isDefinedBy rdf:resource="http://purl.org/ontology/po/"/>
        <rdfs:label>text</rdfs:label>
        <vs:term_status>testing</vs:term_status>
    </owl:DatatypeProperty>
    


    <!-- 
    ///////////////////////////////////////////////////////////////////////////////////////
    //
    // Classes
    //
    ///////////////////////////////////////////////////////////////////////////////////////
     -->

    


    <!-- http://purl.org/dc/dcam/VocabularyEncodingScheme -->

    <owl:Class rdf:about="http://purl.org/dc/dcam/VocabularyEncodingScheme"/>
    


    <!-- http://purl.org/dc/dcmitype/Collection -->

    <owl:Class rdf:about="http://purl.org/dc/dcmitype/Collection"/>
    


    <!-- http://purl.org/dc/terms/Agent -->

    <owl:Class rdf:about="http://purl.org/dc/terms/Agent"/>
    


    <!-- http://purl.org/dc/terms/AgentClass -->

    <owl:Class rdf:about="http://purl.org/dc/terms/AgentClass">
        <rdfs:subClassOf rdf:resource="http://www.w3.org/2000/01/rdf-schema#Class"/>
    </owl:Class>
    


    <!-- http://purl.org/dc/terms/BibliographicResource -->

    <owl:Class rdf:about="http://purl.org/dc/terms/BibliographicResource"/>
    


    <!-- http://purl.org/dc/terms/FileFormat -->

    <owl:Class rdf:about="http://purl.org/dc/terms/FileFormat">
        <rdfs:subClassOf rdf:resource="http://purl.org/dc/terms/MediaType"/>
    </owl:Class>
    


    <!-- http://purl.org/dc/terms/Frequency -->

    <owl:Class rdf:about="http://purl.org/dc/terms/Frequency"/>
    


    <!-- http://purl.org/dc/terms/Jurisdiction -->

    <owl:Class rdf:about="http://purl.org/dc/terms/Jurisdiction">
        <rdfs:subClassOf rdf:resource="http://purl.org/dc/terms/LocationPeriodOrJurisdiction"/>
    </owl:Class>
    


    <!-- http://purl.org/dc/terms/LicenseDocument -->

    <owl:Class rdf:about="http://purl.org/dc/terms/LicenseDocument">
        <rdfs:subClassOf rdf:resource="http://purl.org/dc/terms/RightsStatement"/>
    </owl:Class>
    


    <!-- http://purl.org/dc/terms/LinguisticSystem -->

    <owl:Class rdf:about="http://purl.org/dc/terms/LinguisticSystem"/>
    


    <!-- http://purl.org/dc/terms/Location -->

    <owl:Class rdf:about="http://purl.org/dc/terms/Location">
        <rdfs:subClassOf rdf:resource="http://purl.org/dc/terms/LocationPeriodOrJurisdiction"/>
    </owl:Class>
    


    <!-- http://purl.org/dc/terms/LocationPeriodOrJurisdiction -->

    <owl:Class rdf:about="http://purl.org/dc/terms/LocationPeriodOrJurisdiction"/>
    


    <!-- http://purl.org/dc/terms/MediaType -->

    <owl:Class rdf:about="http://purl.org/dc/terms/MediaType">
        <rdfs:subClassOf rdf:resource="http://purl.org/dc/terms/MediaTypeOrExtent"/>
    </owl:Class>
    


    <!-- http://purl.org/dc/terms/MediaTypeOrExtent -->

    <owl:Class rdf:about="http://purl.org/dc/terms/MediaTypeOrExtent"/>
    


    <!-- http://purl.org/dc/terms/MethodOfAccrual -->

    <owl:Class rdf:about="http://purl.org/dc/terms/MethodOfAccrual"/>
    


    <!-- http://purl.org/dc/terms/MethodOfInstruction -->

    <owl:Class rdf:about="http://purl.org/dc/terms/MethodOfInstruction"/>
    


    <!-- http://purl.org/dc/terms/PeriodOfTime -->

    <owl:Class rdf:about="http://purl.org/dc/terms/PeriodOfTime">
        <rdfs:subClassOf rdf:resource="http://purl.org/dc/terms/LocationPeriodOrJurisdiction"/>
    </owl:Class>
    


    <!-- http://purl.org/dc/terms/PhysicalMedium -->

    <owl:Class rdf:about="http://purl.org/dc/terms/PhysicalMedium">
        <rdfs:subClassOf rdf:resource="http://purl.org/dc/terms/MediaType"/>
    </owl:Class>
    


    <!-- http://purl.org/dc/terms/PhysicalResource -->

    <owl:Class rdf:about="http://purl.org/dc/terms/PhysicalResource"/>
    


    <!-- http://purl.org/dc/terms/Policy -->

    <owl:Class rdf:about="http://purl.org/dc/terms/Policy"/>
    


    <!-- http://purl.org/dc/terms/ProvenanceStatement -->

    <owl:Class rdf:about="http://purl.org/dc/terms/ProvenanceStatement"/>
    


    <!-- http://purl.org/dc/terms/RightsStatement -->

    <owl:Class rdf:about="http://purl.org/dc/terms/RightsStatement"/>
    


    <!-- http://purl.org/dc/terms/SizeOrDuration -->

    <owl:Class rdf:about="http://purl.org/dc/terms/SizeOrDuration">
        <rdfs:subClassOf rdf:resource="http://purl.org/dc/terms/MediaTypeOrExtent"/>
    </owl:Class>
    


    <!-- http://purl.org/dc/terms/Standard -->

    <owl:Class rdf:about="http://purl.org/dc/terms/Standard"/>
    


    <!-- http://purl.org/ontology/mo/Track -->

    <owl:Class rdf:about="http://purl.org/ontology/mo/Track"/>
    


    <!-- http://purl.org/ontology/po/AudioDescribedVersion -->

    <owl:Class rdf:about="http://purl.org/ontology/po/AudioDescribedVersion">
        <rdfs:subClassOf rdf:resource="http://purl.org/ontology/po/Version"/>
        <rdfs:comment>
		A version holding an audio description.
	</rdfs:comment>
        <rdfs:isDefinedBy rdf:resource="http://purl.org/ontology/po/"/>
        <rdfs:label>AudioDescribedVersion</rdfs:label>
        <vs:term_status>testing</vs:term_status>
    </owl:Class>
    


    <!-- http://purl.org/ontology/po/Brand -->

    <owl:Class rdf:about="http://purl.org/ontology/po/Brand">
        <rdfs:subClassOf rdf:resource="http://purl.org/ontology/po/Programme"/>
        <owl:disjointWith rdf:resource="http://purl.org/ontology/po/Clip"/>
        <owl:disjointWith rdf:resource="http://purl.org/ontology/po/Episode"/>
        <owl:disjointWith rdf:resource="http://purl.org/ontology/po/ProgrammeItem"/>
        <owl:disjointWith rdf:resource="http://purl.org/ontology/po/Series"/>
        <rdfs:comment>
		A brand, e.g. `Top Gear&apos;
	</rdfs:comment>
        <rdfs:isDefinedBy rdf:resource="http://purl.org/ontology/po/"/>
        <rdfs:label>Brand</rdfs:label>
        <vs:term_status>stable</vs:term_status>
    </owl:Class>
    


    <!-- http://purl.org/ontology/po/Broadcast -->

    <owl:Class rdf:about="http://purl.org/ontology/po/Broadcast">
        <rdfs:subClassOf rdf:resource="http://purl.org/NET/c4dm/event.owl#Event"/>
        <rdfs:comment>
		A broadcast event.
		Subsumes the event concept defined in
		the Event ontology.
		A broadcast is associated with a service, and with a
		particular version of an episode.
	</rdfs:comment>
        <rdfs:isDefinedBy rdf:resource="http://purl.org/ontology/po/"/>
        <rdfs:label>Broadcast</rdfs:label>
        <vs:term_status>stable</vs:term_status>
    </owl:Class>
    


    <!-- http://purl.org/ontology/po/Broadcaster -->

    <owl:Class rdf:about="http://purl.org/ontology/po/Broadcaster">
        <rdfs:subClassOf rdf:resource="http://xmlns.com/foaf/0.1/Organization"/>
        <rdfs:comment>
		An organization responsible of some broadcasting services.
        It can hold a set of services and outlets.
	</rdfs:comment>
        <rdfs:isDefinedBy rdf:resource="http://purl.org/ontology/po/"/>
        <rdfs:label>Broadcaster</rdfs:label>
        <vs:term_status>stable</vs:term_status>
    </owl:Class>
    


    <!-- http://purl.org/ontology/po/Category -->

    <owl:Class rdf:about="http://purl.org/ontology/po/Category">
        <rdfs:comment>
        A category provides a way of classifying a set of programmes. Such classifications
        can be performed according to multiple dimensions and taxonomies, e.g. genre, format, places, people, subjects...
    </rdfs:comment>
        <rdfs:isDefinedBy rdf:resource="http://purl.org/ontology/po/"/>
        <rdfs:label>Category</rdfs:label>
        <vs:term_status>testing</vs:term_status>
    </owl:Class>
    


    <!-- http://purl.org/ontology/po/Channel -->

    <owl:Class rdf:about="http://purl.org/ontology/po/Channel">
        <rdfs:comment>
        A physical channel on which a broadcast occurs.
        A single outlet or service can be associated with multiple channels.
        For example, Radio 4 LW broadcasts on Analogue Long Wave and on Digital
        Satellite.
    </rdfs:comment>
        <rdfs:isDefinedBy rdf:resource="http://purl.org/ontology/po/"/>
        <rdfs:label>Channel</rdfs:label>
        <vs:term_status>testing</vs:term_status>
    </owl:Class>
    


    <!-- http://purl.org/ontology/po/Clip -->

    <owl:Class rdf:about="http://purl.org/ontology/po/Clip">
        <rdfs:subClassOf rdf:resource="http://purl.org/ontology/po/Programme"/>
        <rdfs:subClassOf rdf:resource="http://purl.org/ontology/po/ProgrammeItem"/>
        <owl:disjointWith rdf:resource="http://purl.org/ontology/po/Series"/>
        <rdfs:comment>
        A particular clip, e.g. `Clip of Top Gear, first series&apos;
    </rdfs:comment>
        <rdfs:isDefinedBy rdf:resource="http://purl.org/ontology/po/"/>
        <rdfs:label>Clip</rdfs:label>
        <vs:term_status>testing</vs:term_status>
    </owl:Class>
    


    <!-- http://purl.org/ontology/po/DAB -->

    <owl:Class rdf:about="http://purl.org/ontology/po/DAB">
        <rdfs:subClassOf rdf:resource="http://purl.org/ontology/po/Channel"/>
        <rdfs:comment>
		Digital Audio Broadcasting
	</rdfs:comment>
        <rdfs:isDefinedBy rdf:resource="http://purl.org/ontology/po/"/>
        <rdfs:label>DAB</rdfs:label>
        <vs:term_status>testing</vs:term_status>
    </owl:Class>
    


    <!-- http://purl.org/ontology/po/DVB -->

    <owl:Class rdf:about="http://purl.org/ontology/po/DVB">
        <rdfs:subClassOf rdf:resource="http://purl.org/ontology/po/Channel"/>
        <rdfs:comment>
		Digital Video Broadcasting
	</rdfs:comment>
        <rdfs:isDefinedBy rdf:resource="http://purl.org/ontology/po/"/>
        <rdfs:label>DVB</rdfs:label>
        <vs:term_status>testing</vs:term_status>
    </owl:Class>
    


    <!-- http://purl.org/ontology/po/Episode -->

    <owl:Class rdf:about="http://purl.org/ontology/po/Episode">
        <rdfs:subClassOf rdf:resource="http://purl.org/ontology/po/Programme"/>
        <rdfs:subClassOf rdf:resource="http://purl.org/ontology/po/ProgrammeItem"/>
        <owl:disjointWith rdf:resource="http://purl.org/ontology/po/Series"/>
        <rdfs:comment>
		A particular episode, e.g. `Top Gear, first episode of the first series&apos; or the film &apos;A Walk in the Sun&apos; (http://www.bbc.co.uk/programmes/b00gfzdt)
	</rdfs:comment>
        <rdfs:isDefinedBy rdf:resource="http://purl.org/ontology/po/"/>
        <rdfs:label>Episode</rdfs:label>
        <vs:term_status>stable</vs:term_status>
    </owl:Class>
    


    <!-- http://purl.org/ontology/po/FM -->

    <owl:Class rdf:about="http://purl.org/ontology/po/FM">
        <rdfs:subClassOf rdf:resource="http://purl.org/ontology/po/Channel"/>
        <rdfs:comment>
		The FM broadcast band
	</rdfs:comment>
        <rdfs:isDefinedBy rdf:resource="http://purl.org/ontology/po/"/>
        <rdfs:label>FM</rdfs:label>
        <vs:term_status>testing</vs:term_status>
    </owl:Class>
    


    <!-- http://purl.org/ontology/po/FirstBroadcast -->

    <owl:Class rdf:about="http://purl.org/ontology/po/FirstBroadcast">
        <rdfs:subClassOf rdf:resource="http://purl.org/ontology/po/Broadcast"/>
        <owl:disjointWith rdf:resource="http://purl.org/ontology/po/RepeatBroadcast"/>
        <rdfs:comment>
		Specifies a broadcast as being the
		first one of a particular version.
	 </rdfs:comment>
        <rdfs:isDefinedBy rdf:resource="http://purl.org/ontology/po/"/>
        <rdfs:label>FirstBroadcast</rdfs:label>
        <vs:term_status>testing</vs:term_status>
    </owl:Class>
    


    <!-- http://purl.org/ontology/po/Format -->

    <owl:Class rdf:about="http://purl.org/ontology/po/Format">
        <rdfs:subClassOf rdf:resource="http://purl.org/ontology/po/Category"/>
        <rdfs:comment>
        Anchor point for format taxonomies, similar to po:Genre for genre taxonomies.
        Instances of this concept include documentaries, talk shows, animation, etc.
    </rdfs:comment>
        <rdfs:isDefinedBy rdf:resource="http://purl.org/ontology/po/"/>
        <rdfs:label>Format</rdfs:label>
        <vs:term_status>testing</vs:term_status>
    </owl:Class>
    


    <!-- http://purl.org/ontology/po/Genre -->

    <owl:Class rdf:about="http://purl.org/ontology/po/Genre">
        <rdfs:subClassOf rdf:resource="http://purl.org/ontology/po/Category"/>
        <rdfs:comment>
        An anchor point for a programmes&apos; genre taxonomy, e.g. &apos;Drama&apos;/&apos;Biographical&apos;.
	</rdfs:comment>
        <rdfs:isDefinedBy rdf:resource="http://purl.org/ontology/po/"/>
        <rdfs:label>Genre</rdfs:label>
        <vs:term_status>testing</vs:term_status>
    </owl:Class>
    


    <!-- http://purl.org/ontology/po/IPStream -->

    <owl:Class rdf:about="http://purl.org/ontology/po/IPStream">
        <rdfs:subClassOf rdf:resource="http://purl.org/ontology/po/Channel"/>
        <rdfs:comment>
		IP stream
	</rdfs:comment>
        <rdfs:isDefinedBy rdf:resource="http://purl.org/ontology/po/"/>
        <rdfs:label>IP stream</rdfs:label>
        <vs:term_status>testing</vs:term_status>
    </owl:Class>
    


    <!-- http://purl.org/ontology/po/LW -->

    <owl:Class rdf:about="http://purl.org/ontology/po/LW">
        <rdfs:subClassOf rdf:resource="http://purl.org/ontology/po/Channel"/>
        <rdfs:comment>
		The AM broadcast band
	</rdfs:comment>
        <rdfs:isDefinedBy rdf:resource="http://purl.org/ontology/po/"/>
        <rdfs:label>AM</rdfs:label>
        <vs:term_status>testing</vs:term_status>
    </owl:Class>
    


    <!-- http://purl.org/ontology/po/LocalRadio -->

    <owl:Class rdf:about="http://purl.org/ontology/po/LocalRadio">
        <rdfs:subClassOf rdf:resource="http://purl.org/ontology/po/Radio"/>
        <owl:disjointWith rdf:resource="http://purl.org/ontology/po/NationalRadio"/>
        <owl:disjointWith rdf:resource="http://purl.org/ontology/po/RegionalRadio"/>
        <rdfs:comment>
		Radio services aiming at a local coverage.
	</rdfs:comment>
        <rdfs:isDefinedBy rdf:resource="http://purl.org/ontology/po/"/>
        <rdfs:label>LocalRadio</rdfs:label>
        <vs:term_status>testing</vs:term_status>
    </owl:Class>
    


    <!-- http://purl.org/ontology/po/MusicSegment -->

    <owl:Class rdf:about="http://purl.org/ontology/po/MusicSegment">
        <rdfs:subClassOf rdf:resource="http://purl.org/ontology/po/Segment"/>
        <rdfs:comment>
		Classification of an episode version&apos;s region corresponding to a musical track being played.
	</rdfs:comment>
        <rdfs:label>MusicSegment</rdfs:label>
        <vs:term_status>testing</vs:term_status>
    </owl:Class>
    


    <!-- http://purl.org/ontology/po/NationalRadio -->

    <owl:Class rdf:about="http://purl.org/ontology/po/NationalRadio">
        <rdfs:subClassOf rdf:resource="http://purl.org/ontology/po/Radio"/>
        <owl:disjointWith rdf:resource="http://purl.org/ontology/po/RegionalRadio"/>
        <rdfs:comment>
		Radio services aiming at a national coverage.
	</rdfs:comment>
        <rdfs:isDefinedBy rdf:resource="http://purl.org/ontology/po/"/>
        <rdfs:label rdf:datatype="http://www.w3.org/2001/XMLSchema#string">NationalRadio</rdfs:label>
        <vs:term_status>testing</vs:term_status>
    </owl:Class>
    


    <!-- http://purl.org/ontology/po/OriginalVersion -->

    <owl:Class rdf:about="http://purl.org/ontology/po/OriginalVersion">
        <rdfs:subClassOf rdf:resource="http://purl.org/ontology/po/Version"/>
        <owl:disjointWith rdf:resource="http://purl.org/ontology/po/ShortenedVersion"/>
        <rdfs:comment>
		An `original&apos; version, the legacy version of
		a particular episode.
	</rdfs:comment>
        <rdfs:isDefinedBy rdf:resource="http://purl.org/ontology/po/"/>
        <rdfs:label rdf:datatype="http://www.w3.org/2001/XMLSchema#string">OriginalVersion</rdfs:label>
        <vs:term_status>testing</vs:term_status>
    </owl:Class>
    


    <!-- http://purl.org/ontology/po/Outlet -->

    <owl:Class rdf:about="http://purl.org/ontology/po/Outlet">
        <rdfs:subClassOf rdf:resource="http://purl.org/ontology/po/Service"/>
        <rdfs:comment>
        Outlet of a particular service, e.g. Radio 4 LW and FM for Radio 4.
        Outlets are services which do not have variations.
        The criterion for an outlet is its timeline.
        For example, Radio 4 LW broadcasts on Analogue Long Wave, but also on Digital Satellite.
        It corresponds to just one outlet, as they are simulcasts.
        The two physical channels for broadcasts correspond to po:Channel.
    </rdfs:comment>
        <rdfs:isDefinedBy rdf:resource="http://purl.org/ontology/po/"/>
        <rdfs:label rdf:datatype="http://www.w3.org/2001/XMLSchema#string">Outlet</rdfs:label>
        <vs:term_status>testing</vs:term_status>
    </owl:Class>
    


    <!-- http://purl.org/ontology/po/Person -->

    <owl:Class rdf:about="http://purl.org/ontology/po/Person">
        <owl:equivalentClass rdf:resource="http://xmlns.com/foaf/0.1/Person"/>
        <rdfs:subClassOf rdf:resource="http://purl.org/ontology/po/Category"/>
        <rdfs:comment>A person</rdfs:comment>
        <rdfs:isDefinedBy rdf:resource="http://purl.org/ontology/po/"/>
        <rdfs:label rdf:datatype="http://www.w3.org/2001/XMLSchema#string">Person</rdfs:label>
        <vs:term_status>testing</vs:term_status>
    </owl:Class>
    


    <!-- http://purl.org/ontology/po/Place -->

    <owl:Class rdf:about="http://purl.org/ontology/po/Place">
        <owl:equivalentClass rdf:resource="http://www.w3.org/2003/01/geo/wgs84_pos#Feature"/>
        <rdfs:subClassOf rdf:resource="http://purl.org/ontology/po/Category"/>
        <rdfs:comment>A physical place</rdfs:comment>
        <rdfs:isDefinedBy rdf:resource="http://purl.org/ontology/po/"/>
        <rdfs:label rdf:datatype="http://www.w3.org/2001/XMLSchema#string">Place</rdfs:label>
        <vs:term_status>testing</vs:term_status>
    </owl:Class>
    


    <!-- http://purl.org/ontology/po/Programme -->

    <owl:Class rdf:about="http://purl.org/ontology/po/Programme">
        <rdfs:comment>
		A programme, can either be a brand, a series or an episode
	</rdfs:comment>
        <rdfs:isDefinedBy rdf:resource="http://purl.org/ontology/po/"/>
        <rdfs:label rdf:datatype="http://www.w3.org/2001/XMLSchema#string">Programme</rdfs:label>
        <vs:term_status>stable</vs:term_status>
    </owl:Class>
    


    <!-- http://purl.org/ontology/po/ProgrammeItem -->

    <owl:Class rdf:about="http://purl.org/ontology/po/ProgrammeItem">
        <rdfs:subClassOf rdf:resource="http://purl.org/ontology/po/Programme"/>
        <owl:disjointWith rdf:resource="http://purl.org/ontology/po/Series"/>
        <rdfs:comment>
        A programme that can have versions, and as such can be broadcast or made available on-demand, e.g. a clip or an episode.
    </rdfs:comment>
        <rdfs:isDefinedBy rdf:resource="http://purl.org/ontology/po/"/>
        <rdfs:label rdf:datatype="http://www.w3.org/2001/XMLSchema#string">ProgrammeItem</rdfs:label>
        <vs:term_status>testing</vs:term_status>
    </owl:Class>
    


    <!-- http://purl.org/ontology/po/Radio -->

    <owl:Class rdf:about="http://purl.org/ontology/po/Radio">
        <rdfs:subClassOf rdf:resource="http://purl.org/ontology/po/Service"/>
        <owl:disjointWith rdf:resource="http://purl.org/ontology/po/TV"/>
        <owl:disjointWith rdf:resource="http://purl.org/ontology/po/Web"/>
        <rdfs:comment>
		Services that use a radio medium.
	</rdfs:comment>
        <rdfs:isDefinedBy rdf:resource="http://purl.org/ontology/po/"/>
        <rdfs:label rdf:datatype="http://www.w3.org/2001/XMLSchema#string">Radio</rdfs:label>
        <vs:term_status>testing</vs:term_status>
    </owl:Class>
    


    <!-- http://purl.org/ontology/po/RegionalRadio -->

    <owl:Class rdf:about="http://purl.org/ontology/po/RegionalRadio">
        <rdfs:subClassOf rdf:resource="http://purl.org/ontology/po/Radio"/>
        <rdfs:comment>
		Radio services aiming at a regional coverage.
	</rdfs:comment>
        <rdfs:isDefinedBy rdf:resource="http://purl.org/ontology/po/"/>
        <rdfs:label rdf:datatype="http://www.w3.org/2001/XMLSchema#string">RegionalRadio</rdfs:label>
        <vs:term_status>testing</vs:term_status>
    </owl:Class>
    


    <!-- http://purl.org/ontology/po/RepeatBroadcast -->

    <owl:Class rdf:about="http://purl.org/ontology/po/RepeatBroadcast">
        <rdfs:subClassOf rdf:resource="http://purl.org/ontology/po/Broadcast"/>
        <rdfs:comment>
		Specifies a broadcast as being a
		repeat.
	</rdfs:comment>
        <rdfs:isDefinedBy rdf:resource="http://purl.org/ontology/po/"/>
        <rdfs:label rdf:datatype="http://www.w3.org/2001/XMLSchema#string">Repeat</rdfs:label>
        <vs:term_status>testing</vs:term_status>
    </owl:Class>
    


    <!-- http://purl.org/ontology/po/Season -->

    <owl:Class rdf:about="http://purl.org/ontology/po/Season">
        <rdfs:comment>
		A season is a group of broadcasts.
	</rdfs:comment>
        <rdfs:isDefinedBy rdf:resource="http://purl.org/ontology/po/"/>
        <rdfs:label rdf:datatype="http://www.w3.org/2001/XMLSchema#string">Season</rdfs:label>
        <vs:term_status>testing</vs:term_status>
    </owl:Class>
    


    <!-- http://purl.org/ontology/po/Segment -->

    <owl:Class rdf:about="http://purl.org/ontology/po/Segment">
        <rdfs:subClassOf rdf:resource="http://purl.org/NET/c4dm/event.owl#Event"/>
        <rdfs:comment>
		Classification of an episode version&apos;s region, e.g. &apos;this track was played at that time&apos;.
	</rdfs:comment>
        <rdfs:isDefinedBy rdf:resource="http://purl.org/ontology/po/"/>
        <rdfs:label rdf:datatype="http://www.w3.org/2001/XMLSchema#string">Segment</rdfs:label>
        <vs:term_status>testing</vs:term_status>
    </owl:Class>
    


    <!-- http://purl.org/ontology/po/Series -->

    <owl:Class rdf:about="http://purl.org/ontology/po/Series">
        <rdfs:subClassOf rdf:resource="http://purl.org/ontology/po/Programme"/>
        <rdfs:comment>
		A series, e.g. `Top Gear, first season&apos;
	</rdfs:comment>
        <rdfs:isDefinedBy rdf:resource="http://purl.org/ontology/po/"/>
        <rdfs:label rdf:datatype="http://www.w3.org/2001/XMLSchema#string">Series</rdfs:label>
        <vs:term_status>stable</vs:term_status>
    </owl:Class>
    


    <!-- http://purl.org/ontology/po/Service -->

    <owl:Class rdf:about="http://purl.org/ontology/po/Service">
        <rdfs:comment>
        A broadcasting service.
		Instances of this concept include BBC Radio Wales, BBC Radio 4, BBC News, etc.
        A service is a collection of outlets which contain common material, but with some variations, e.g. by
        region.
        Hence, a service may have multiple outlets (po:Outlet), e.g. BBC Radio 4 has BBC Radio 4 LW and BBC Radio 4 FM.
        A hierarchy of services types is defined within this ontology, e.g. radio and TV.
        A service that is a master brand only (a service that only commissions programmes, e.g. BBC Switch) should
        be an instance of the top-level po:Service.
	</rdfs:comment>
        <rdfs:isDefinedBy rdf:resource="http://purl.org/ontology/po/"/>
        <rdfs:label rdf:datatype="http://www.w3.org/2001/XMLSchema#string">Service</rdfs:label>
        <vs:term_status>stable</vs:term_status>
    </owl:Class>
    


    <!-- http://purl.org/ontology/po/ShortenedVersion -->

    <owl:Class rdf:about="http://purl.org/ontology/po/ShortenedVersion">
        <rdfs:subClassOf rdf:resource="http://purl.org/ontology/po/Version"/>
        <rdfs:comment>
		A shortened version.
	</rdfs:comment>
        <rdfs:isDefinedBy rdf:resource="http://purl.org/ontology/po/"/>
        <rdfs:label rdf:datatype="http://www.w3.org/2001/XMLSchema#string">ShortenedVersion</rdfs:label>
        <vs:term_status>testing</vs:term_status>
    </owl:Class>
    


    <!-- http://purl.org/ontology/po/SignedVersion -->

    <owl:Class rdf:about="http://purl.org/ontology/po/SignedVersion">
        <rdfs:subClassOf rdf:resource="http://purl.org/ontology/po/Version"/>
        <rdfs:comment>
		A version holding sign language.
	</rdfs:comment>
        <rdfs:isDefinedBy rdf:resource="http://purl.org/ontology/po/"/>
        <rdfs:label rdf:datatype="http://www.w3.org/2001/XMLSchema#string">SignLanguage</rdfs:label>
        <vs:term_status>testing</vs:term_status>
    </owl:Class>
    


    <!-- http://purl.org/ontology/po/SpeechSegment -->

    <owl:Class rdf:about="http://purl.org/ontology/po/SpeechSegment">
        <rdfs:subClassOf rdf:resource="http://purl.org/ontology/po/Segment"/>
        <rdfs:comment>
        Classification of an episode version&apos;s region holding speech content.
    </rdfs:comment>
        <vs:term_status>testing</vs:term_status>
    </owl:Class>
    


    <!-- http://purl.org/ontology/po/Subject -->

    <owl:Class rdf:about="http://purl.org/ontology/po/Subject">
        <rdfs:subClassOf rdf:resource="http://purl.org/ontology/po/Category"/>
        <rdfs:comment>
        Anchor point for subject taxonomies.
    </rdfs:comment>
        <rdfs:isDefinedBy rdf:resource="http://purl.org/ontology/po/"/>
        <rdfs:label rdf:datatype="http://www.w3.org/2001/XMLSchema#string">Subject</rdfs:label>
        <vs:term_status>testing</vs:term_status>
    </owl:Class>
    


    <!-- http://purl.org/ontology/po/Subtitle -->

    <owl:Class rdf:about="http://purl.org/ontology/po/Subtitle">
        <rdfs:subClassOf rdf:resource="http://purl.org/NET/c4dm/event.owl#Event"/>
        <rdfs:comment>
        Classification of an episode version&apos;s region corresponding to a subtitle being shown.
    </rdfs:comment>
        <rdfs:isDefinedBy rdf:resource="http://purl.org/ontology/po/"/>
        <rdfs:label rdf:datatype="http://www.w3.org/2001/XMLSchema#string">Subtitle</rdfs:label>
        <vs:term_status>testing</vs:term_status>
    </owl:Class>
    


    <!-- http://purl.org/ontology/po/TV -->

    <owl:Class rdf:about="http://purl.org/ontology/po/TV">
        <rdfs:subClassOf rdf:resource="http://purl.org/ontology/po/Service"/>
        <owl:disjointWith rdf:resource="http://purl.org/ontology/po/Web"/>
        <rdfs:comment>
		Services that use a television medium.
	</rdfs:comment>
        <rdfs:isDefinedBy rdf:resource="http://purl.org/ontology/po/"/>
        <rdfs:label rdf:datatype="http://www.w3.org/2001/XMLSchema#string">TV</rdfs:label>
        <vs:term_status>testing</vs:term_status>
    </owl:Class>
    


    <!-- http://purl.org/ontology/po/Version -->

    <owl:Class rdf:about="http://purl.org/ontology/po/Version">
        <rdfs:comment>
		A particular version of an episode.
		Such versions include shortened ones, audio described ones
		or ones that holds sign language.
		The version is associated to a timeline.
	</rdfs:comment>
        <rdfs:isDefinedBy rdf:resource="http://purl.org/ontology/po/"/>
        <rdfs:label rdf:datatype="http://www.w3.org/2001/XMLSchema#string">Version</rdfs:label>
        <vs:term_status>stable</vs:term_status>
    </owl:Class>
    


    <!-- http://purl.org/ontology/po/Web -->

    <owl:Class rdf:about="http://purl.org/ontology/po/Web">
        <rdfs:subClassOf rdf:resource="http://purl.org/ontology/po/Service"/>
        <rdfs:comment>
		Services that use a Web medium.
	</rdfs:comment>
        <rdfs:isDefinedBy rdf:resource="http://purl.org/ontology/po/"/>
        <rdfs:label rdf:datatype="http://www.w3.org/2001/XMLSchema#string">Web</rdfs:label>
        <vs:term_status>testing</vs:term_status>
    </owl:Class>
    


    <!-- http://www.bbc.co.uk/ontologies/provenance/Ontology -->

    <owl:Class rdf:about="http://www.bbc.co.uk/ontologies/provenance/Ontology"/>
    


    <!-- http://www.w3.org/2000/01/rdf-schema#Class -->

    <owl:Class rdf:about="http://www.w3.org/2000/01/rdf-schema#Class"/>
    


    <!-- http://www.w3.org/2003/01/geo/wgs84_pos#Feature -->

    <owl:Class rdf:about="http://www.w3.org/2003/01/geo/wgs84_pos#Feature"/>
    


    <!-- http://xmlns.com/foaf/0.1/Document -->

    <owl:Class rdf:about="http://xmlns.com/foaf/0.1/Document"/>
    


    <!-- http://xmlns.com/foaf/0.1/Organization -->

    <owl:Class rdf:about="http://xmlns.com/foaf/0.1/Organization"/>
    


    <!-- http://xmlns.com/foaf/0.1/Person -->

    <rdf:Description rdf:about="http://xmlns.com/foaf/0.1/Person"/>
    


    <!-- 
    ///////////////////////////////////////////////////////////////////////////////////////
    //
    // Individuals
    //
    ///////////////////////////////////////////////////////////////////////////////////////
     -->

    


    <!-- http://creativecommons.org/licenses/by/4.0#id -->

    <owl:NamedIndividual rdf:about="http://creativecommons.org/licenses/by/4.0#id"/>
    


    <!-- http://metade.org/foaf.rdf#me -->

    <owl:NamedIndividual rdf:about="http://metade.org/foaf.rdf#me"/>
    


    <!-- http://purl.org/dc/aboutdcmi#DCMI -->

    <owl:NamedIndividual rdf:about="http://purl.org/dc/aboutdcmi#DCMI"/>
    


    <!-- http://purl.org/dc/terms/ -->

    <owl:NamedIndividual rdf:about="http://purl.org/dc/terms/">
        <dcterms:publisher rdf:resource="http://purl.org/dc/aboutdcmi#DCMI"/>
        <dcterms:modified rdf:datatype="http://www.w3.org/2001/XMLSchema#date">2012-06-14</dcterms:modified>
        <dcterms:title xml:lang="en">DCMI Metadata Terms - other</dcterms:title>
    </owl:NamedIndividual>
    


    <!-- http://purl.org/dc/terms/Agent -->

    <owl:NamedIndividual rdf:about="http://purl.org/dc/terms/Agent">
        <rdf:type rdf:resource="http://purl.org/dc/terms/AgentClass"/>
        <dcterms:issued rdf:datatype="http://www.w3.org/2001/XMLSchema#date">2008-01-14</dcterms:issued>
    </owl:NamedIndividual>
    


    <!-- http://purl.org/dc/terms/AgentClass -->

    <owl:NamedIndividual rdf:about="http://purl.org/dc/terms/AgentClass">
        <dcterms:issued rdf:datatype="http://www.w3.org/2001/XMLSchema#date">2008-01-14</dcterms:issued>
        <dcterms:modified rdf:datatype="http://www.w3.org/2001/XMLSchema#date">2012-06-14</dcterms:modified>
    </owl:NamedIndividual>
    


    <!-- http://purl.org/dc/terms/BibliographicResource -->

    <owl:NamedIndividual rdf:about="http://purl.org/dc/terms/BibliographicResource">
        <dcterms:issued rdf:datatype="http://www.w3.org/2001/XMLSchema#date">2008-01-14</dcterms:issued>
    </owl:NamedIndividual>
    


    <!-- http://purl.org/dc/terms/Box -->

    <owl:NamedIndividual rdf:about="http://purl.org/dc/terms/Box">
        <dcterms:issued rdf:datatype="http://www.w3.org/2001/XMLSchema#date">2000-07-11</dcterms:issued>
        <dcterms:modified rdf:datatype="http://www.w3.org/2001/XMLSchema#date">2008-01-14</dcterms:modified>
    </owl:NamedIndividual>
    


    <!-- http://purl.org/dc/terms/DCMIType -->

    <owl:NamedIndividual rdf:about="http://purl.org/dc/terms/DCMIType">
        <rdf:type rdf:resource="http://purl.org/dc/dcam/VocabularyEncodingScheme"/>
        <dcterms:issued rdf:datatype="http://www.w3.org/2001/XMLSchema#date">2000-07-11</dcterms:issued>
        <dcterms:modified rdf:datatype="http://www.w3.org/2001/XMLSchema#date">2012-06-14</dcterms:modified>
        <dcterms:hasVersion rdf:resource="http://dublincore.org/usage/terms/history/#DCMIType-005"/>
        <rdfs:comment xml:lang="en">The set of classes specified by the DCMI Type Vocabulary, used to categorize the nature or genre of the resource.</rdfs:comment>
        <rdfs:isDefinedBy rdf:resource="http://purl.org/dc/terms/"/>
        <rdfs:label xml:lang="en">DCMI Type Vocabulary</rdfs:label>
        <rdfs:seeAlso rdf:resource="http://purl.org/dc/dcmitype/"/>
    </owl:NamedIndividual>
    


    <!-- http://purl.org/dc/terms/DDC -->

    <owl:NamedIndividual rdf:about="http://purl.org/dc/terms/DDC">
        <rdf:type rdf:resource="http://purl.org/dc/dcam/VocabularyEncodingScheme"/>
        <dcterms:issued rdf:datatype="http://www.w3.org/2001/XMLSchema#date">2000-07-11</dcterms:issued>
        <dcterms:modified rdf:datatype="http://www.w3.org/2001/XMLSchema#date">2008-01-14</dcterms:modified>
        <dcterms:hasVersion rdf:resource="http://dublincore.org/usage/terms/history/#DDC-003"/>
        <rdfs:comment xml:lang="en">The set of conceptual resources specified by the Dewey Decimal Classification.</rdfs:comment>
        <rdfs:isDefinedBy rdf:resource="http://purl.org/dc/terms/"/>
        <rdfs:label xml:lang="en">DDC</rdfs:label>
        <rdfs:seeAlso rdf:resource="http://www.oclc.org/dewey/"/>
    </owl:NamedIndividual>
    


    <!-- http://purl.org/dc/terms/FileFormat -->

    <owl:NamedIndividual rdf:about="http://purl.org/dc/terms/FileFormat">
        <dcterms:issued rdf:datatype="http://www.w3.org/2001/XMLSchema#date">2008-01-14</dcterms:issued>
    </owl:NamedIndividual>
    


    <!-- http://purl.org/dc/terms/Frequency -->

    <owl:NamedIndividual rdf:about="http://purl.org/dc/terms/Frequency">
        <dcterms:issued rdf:datatype="http://www.w3.org/2001/XMLSchema#date">2008-01-14</dcterms:issued>
    </owl:NamedIndividual>
    


    <!-- http://purl.org/dc/terms/IMT -->

    <owl:NamedIndividual rdf:about="http://purl.org/dc/terms/IMT">
        <rdf:type rdf:resource="http://purl.org/dc/dcam/VocabularyEncodingScheme"/>
        <dcterms:issued rdf:datatype="http://www.w3.org/2001/XMLSchema#date">2000-07-11</dcterms:issued>
        <dcterms:modified rdf:datatype="http://www.w3.org/2001/XMLSchema#date">2008-01-14</dcterms:modified>
        <dcterms:hasVersion rdf:resource="http://dublincore.org/usage/terms/history/#IMT-004"/>
        <rdfs:comment xml:lang="en">The set of media types specified by the Internet Assigned Numbers Authority.</rdfs:comment>
        <rdfs:isDefinedBy rdf:resource="http://purl.org/dc/terms/"/>
        <rdfs:label xml:lang="en">IMT</rdfs:label>
        <rdfs:seeAlso rdf:resource="http://www.iana.org/assignments/media-types/"/>
    </owl:NamedIndividual>
    


    <!-- http://purl.org/dc/terms/ISO3166 -->

    <owl:NamedIndividual rdf:about="http://purl.org/dc/terms/ISO3166">
        <dcterms:issued rdf:datatype="http://www.w3.org/2001/XMLSchema#date">2000-07-11</dcterms:issued>
        <dcterms:modified rdf:datatype="http://www.w3.org/2001/XMLSchema#date">2008-01-14</dcterms:modified>
    </owl:NamedIndividual>
    


    <!-- http://purl.org/dc/terms/ISO639-2 -->

    <owl:NamedIndividual rdf:about="http://purl.org/dc/terms/ISO639-2">
        <dcterms:issued rdf:datatype="http://www.w3.org/2001/XMLSchema#date">2000-07-11</dcterms:issued>
        <dcterms:modified rdf:datatype="http://www.w3.org/2001/XMLSchema#date">2008-01-14</dcterms:modified>
    </owl:NamedIndividual>
    


    <!-- http://purl.org/dc/terms/ISO639-3 -->

    <owl:NamedIndividual rdf:about="http://purl.org/dc/terms/ISO639-3">
        <dcterms:issued rdf:datatype="http://www.w3.org/2001/XMLSchema#date">2008-01-14</dcterms:issued>
    </owl:NamedIndividual>
    


    <!-- http://purl.org/dc/terms/Jurisdiction -->

    <owl:NamedIndividual rdf:about="http://purl.org/dc/terms/Jurisdiction">
        <dcterms:issued rdf:datatype="http://www.w3.org/2001/XMLSchema#date">2008-01-14</dcterms:issued>
    </owl:NamedIndividual>
    


    <!-- http://purl.org/dc/terms/LCC -->

    <owl:NamedIndividual rdf:about="http://purl.org/dc/terms/LCC">
        <rdf:type rdf:resource="http://purl.org/dc/dcam/VocabularyEncodingScheme"/>
        <dcterms:issued rdf:datatype="http://www.w3.org/2001/XMLSchema#date">2000-07-11</dcterms:issued>
        <dcterms:modified rdf:datatype="http://www.w3.org/2001/XMLSchema#date">2008-01-14</dcterms:modified>
        <dcterms:hasVersion rdf:resource="http://dublincore.org/usage/terms/history/#LCC-003"/>
        <rdfs:comment xml:lang="en">The set of conceptual resources specified by the Library of Congress Classification.</rdfs:comment>
        <rdfs:isDefinedBy rdf:resource="http://purl.org/dc/terms/"/>
        <rdfs:label xml:lang="en">LCC</rdfs:label>
        <rdfs:seeAlso rdf:resource="http://lcweb.loc.gov/catdir/cpso/lcco/lcco.html"/>
    </owl:NamedIndividual>
    


    <!-- http://purl.org/dc/terms/LCSH -->

    <owl:NamedIndividual rdf:about="http://purl.org/dc/terms/LCSH">
        <rdf:type rdf:resource="http://purl.org/dc/dcam/VocabularyEncodingScheme"/>
        <dcterms:issued rdf:datatype="http://www.w3.org/2001/XMLSchema#date">2000-07-11</dcterms:issued>
        <dcterms:modified rdf:datatype="http://www.w3.org/2001/XMLSchema#date">2008-01-14</dcterms:modified>
        <dcterms:hasVersion rdf:resource="http://dublincore.org/usage/terms/history/#LCSH-003"/>
        <rdfs:comment xml:lang="en">The set of labeled concepts specified by the Library of Congress Subject Headings.</rdfs:comment>
        <rdfs:isDefinedBy rdf:resource="http://purl.org/dc/terms/"/>
        <rdfs:label xml:lang="en">LCSH</rdfs:label>
    </owl:NamedIndividual>
    


    <!-- http://purl.org/dc/terms/LicenseDocument -->

    <owl:NamedIndividual rdf:about="http://purl.org/dc/terms/LicenseDocument">
        <dcterms:issued rdf:datatype="http://www.w3.org/2001/XMLSchema#date">2008-01-14</dcterms:issued>
    </owl:NamedIndividual>
    


    <!-- http://purl.org/dc/terms/LinguisticSystem -->

    <owl:NamedIndividual rdf:about="http://purl.org/dc/terms/LinguisticSystem">
        <dcterms:issued rdf:datatype="http://www.w3.org/2001/XMLSchema#date">2008-01-14</dcterms:issued>
    </owl:NamedIndividual>
    


    <!-- http://purl.org/dc/terms/Location -->

    <owl:NamedIndividual rdf:about="http://purl.org/dc/terms/Location">
        <dcterms:issued rdf:datatype="http://www.w3.org/2001/XMLSchema#date">2008-01-14</dcterms:issued>
    </owl:NamedIndividual>
    


    <!-- http://purl.org/dc/terms/LocationPeriodOrJurisdiction -->

    <owl:NamedIndividual rdf:about="http://purl.org/dc/terms/LocationPeriodOrJurisdiction">
        <dcterms:issued rdf:datatype="http://www.w3.org/2001/XMLSchema#date">2008-01-14</dcterms:issued>
    </owl:NamedIndividual>
    


    <!-- http://purl.org/dc/terms/MESH -->

    <owl:NamedIndividual rdf:about="http://purl.org/dc/terms/MESH">
        <rdf:type rdf:resource="http://purl.org/dc/dcam/VocabularyEncodingScheme"/>
        <dcterms:issued rdf:datatype="http://www.w3.org/2001/XMLSchema#date">2000-07-11</dcterms:issued>
        <dcterms:modified rdf:datatype="http://www.w3.org/2001/XMLSchema#date">2008-01-14</dcterms:modified>
        <dcterms:hasVersion rdf:resource="http://dublincore.org/usage/terms/history/#MESH-003"/>
        <rdfs:comment xml:lang="en">The set of labeled concepts specified by the Medical Subject Headings.</rdfs:comment>
        <rdfs:isDefinedBy rdf:resource="http://purl.org/dc/terms/"/>
        <rdfs:label xml:lang="en">MeSH</rdfs:label>
        <rdfs:seeAlso rdf:resource="http://www.nlm.nih.gov/mesh/meshhome.html"/>
    </owl:NamedIndividual>
    


    <!-- http://purl.org/dc/terms/MediaType -->

    <owl:NamedIndividual rdf:about="http://purl.org/dc/terms/MediaType">
        <dcterms:issued rdf:datatype="http://www.w3.org/2001/XMLSchema#date">2008-01-14</dcterms:issued>
    </owl:NamedIndividual>
    


    <!-- http://purl.org/dc/terms/MediaTypeOrExtent -->

    <owl:NamedIndividual rdf:about="http://purl.org/dc/terms/MediaTypeOrExtent">
        <dcterms:issued rdf:datatype="http://www.w3.org/2001/XMLSchema#date">2008-01-14</dcterms:issued>
    </owl:NamedIndividual>
    


    <!-- http://purl.org/dc/terms/MethodOfAccrual -->

    <owl:NamedIndividual rdf:about="http://purl.org/dc/terms/MethodOfAccrual">
        <dcterms:issued rdf:datatype="http://www.w3.org/2001/XMLSchema#date">2008-01-14</dcterms:issued>
    </owl:NamedIndividual>
    


    <!-- http://purl.org/dc/terms/MethodOfInstruction -->

    <owl:NamedIndividual rdf:about="http://purl.org/dc/terms/MethodOfInstruction">
        <dcterms:issued rdf:datatype="http://www.w3.org/2001/XMLSchema#date">2008-01-14</dcterms:issued>
    </owl:NamedIndividual>
    


    <!-- http://purl.org/dc/terms/NLM -->

    <owl:NamedIndividual rdf:about="http://purl.org/dc/terms/NLM">
        <rdf:type rdf:resource="http://purl.org/dc/dcam/VocabularyEncodingScheme"/>
        <dcterms:issued rdf:datatype="http://www.w3.org/2001/XMLSchema#date">2005-06-13</dcterms:issued>
        <dcterms:modified rdf:datatype="http://www.w3.org/2001/XMLSchema#date">2008-01-14</dcterms:modified>
        <dcterms:hasVersion rdf:resource="http://dublincore.org/usage/terms/history/#NLM-002"/>
        <rdfs:comment xml:lang="en">The set of conceptual resources specified by the National Library of Medicine Classification.</rdfs:comment>
        <rdfs:isDefinedBy rdf:resource="http://purl.org/dc/terms/"/>
        <rdfs:label xml:lang="en">NLM</rdfs:label>
        <rdfs:seeAlso rdf:resource="http://wwwcf.nlm.nih.gov/class/"/>
    </owl:NamedIndividual>
    


    <!-- http://purl.org/dc/terms/Period -->

    <owl:NamedIndividual rdf:about="http://purl.org/dc/terms/Period">
        <dcterms:issued rdf:datatype="http://www.w3.org/2001/XMLSchema#date">2000-07-11</dcterms:issued>
        <dcterms:modified rdf:datatype="http://www.w3.org/2001/XMLSchema#date">2008-01-14</dcterms:modified>
    </owl:NamedIndividual>
    


    <!-- http://purl.org/dc/terms/PeriodOfTime -->

    <owl:NamedIndividual rdf:about="http://purl.org/dc/terms/PeriodOfTime">
        <dcterms:issued rdf:datatype="http://www.w3.org/2001/XMLSchema#date">2008-01-14</dcterms:issued>
    </owl:NamedIndividual>
    


    <!-- http://purl.org/dc/terms/PhysicalMedium -->

    <owl:NamedIndividual rdf:about="http://purl.org/dc/terms/PhysicalMedium">
        <dcterms:issued rdf:datatype="http://www.w3.org/2001/XMLSchema#date">2008-01-14</dcterms:issued>
    </owl:NamedIndividual>
    


    <!-- http://purl.org/dc/terms/PhysicalResource -->

    <owl:NamedIndividual rdf:about="http://purl.org/dc/terms/PhysicalResource">
        <dcterms:issued rdf:datatype="http://www.w3.org/2001/XMLSchema#date">2008-01-14</dcterms:issued>
    </owl:NamedIndividual>
    


    <!-- http://purl.org/dc/terms/Point -->

    <owl:NamedIndividual rdf:about="http://purl.org/dc/terms/Point">
        <dcterms:issued rdf:datatype="http://www.w3.org/2001/XMLSchema#date">2000-07-11</dcterms:issued>
        <dcterms:modified rdf:datatype="http://www.w3.org/2001/XMLSchema#date">2008-01-14</dcterms:modified>
    </owl:NamedIndividual>
    


    <!-- http://purl.org/dc/terms/Policy -->

    <owl:NamedIndividual rdf:about="http://purl.org/dc/terms/Policy">
        <dcterms:issued rdf:datatype="http://www.w3.org/2001/XMLSchema#date">2008-01-14</dcterms:issued>
    </owl:NamedIndividual>
    


    <!-- http://purl.org/dc/terms/ProvenanceStatement -->

    <owl:NamedIndividual rdf:about="http://purl.org/dc/terms/ProvenanceStatement">
        <dcterms:issued rdf:datatype="http://www.w3.org/2001/XMLSchema#date">2008-01-14</dcterms:issued>
    </owl:NamedIndividual>
    


    <!-- http://purl.org/dc/terms/RFC1766 -->

    <owl:NamedIndividual rdf:about="http://purl.org/dc/terms/RFC1766">
        <dcterms:issued rdf:datatype="http://www.w3.org/2001/XMLSchema#date">2000-07-11</dcterms:issued>
        <dcterms:modified rdf:datatype="http://www.w3.org/2001/XMLSchema#date">2008-01-14</dcterms:modified>
    </owl:NamedIndividual>
    


    <!-- http://purl.org/dc/terms/RFC3066 -->

    <owl:NamedIndividual rdf:about="http://purl.org/dc/terms/RFC3066">
        <dcterms:issued rdf:datatype="http://www.w3.org/2001/XMLSchema#date">2002-07-13</dcterms:issued>
        <dcterms:modified rdf:datatype="http://www.w3.org/2001/XMLSchema#date">2008-01-14</dcterms:modified>
    </owl:NamedIndividual>
    


    <!-- http://purl.org/dc/terms/RFC4646 -->

    <owl:NamedIndividual rdf:about="http://purl.org/dc/terms/RFC4646">
        <dcterms:issued rdf:datatype="http://www.w3.org/2001/XMLSchema#date">2008-01-14</dcterms:issued>
    </owl:NamedIndividual>
    


    <!-- http://purl.org/dc/terms/RFC5646 -->

    <owl:NamedIndividual rdf:about="http://purl.org/dc/terms/RFC5646">
        <dcterms:issued rdf:datatype="http://www.w3.org/2001/XMLSchema#date">2010-10-11</dcterms:issued>
    </owl:NamedIndividual>
    


    <!-- http://purl.org/dc/terms/RightsStatement -->

    <owl:NamedIndividual rdf:about="http://purl.org/dc/terms/RightsStatement">
        <dcterms:issued rdf:datatype="http://www.w3.org/2001/XMLSchema#date">2008-01-14</dcterms:issued>
    </owl:NamedIndividual>
    


    <!-- http://purl.org/dc/terms/SizeOrDuration -->

    <owl:NamedIndividual rdf:about="http://purl.org/dc/terms/SizeOrDuration">
        <dcterms:issued rdf:datatype="http://www.w3.org/2001/XMLSchema#date">2008-01-14</dcterms:issued>
    </owl:NamedIndividual>
    


    <!-- http://purl.org/dc/terms/Standard -->

    <owl:NamedIndividual rdf:about="http://purl.org/dc/terms/Standard">
        <dcterms:issued rdf:datatype="http://www.w3.org/2001/XMLSchema#date">2008-01-14</dcterms:issued>
    </owl:NamedIndividual>
    


    <!-- http://purl.org/dc/terms/TGN -->

    <owl:NamedIndividual rdf:about="http://purl.org/dc/terms/TGN">
        <rdf:type rdf:resource="http://purl.org/dc/dcam/VocabularyEncodingScheme"/>
        <dcterms:issued rdf:datatype="http://www.w3.org/2001/XMLSchema#date">2000-07-11</dcterms:issued>
        <dcterms:modified rdf:datatype="http://www.w3.org/2001/XMLSchema#date">2008-01-14</dcterms:modified>
        <dcterms:hasVersion rdf:resource="http://dublincore.org/usage/terms/history/#TGN-003"/>
        <rdfs:comment xml:lang="en">The set of places specified by the Getty Thesaurus of Geographic Names.</rdfs:comment>
        <rdfs:isDefinedBy rdf:resource="http://purl.org/dc/terms/"/>
        <rdfs:label xml:lang="en">TGN</rdfs:label>
        <rdfs:seeAlso rdf:resource="http://www.getty.edu/research/tools/vocabulary/tgn/index.html"/>
    </owl:NamedIndividual>
    


    <!-- http://purl.org/dc/terms/UDC -->

    <owl:NamedIndividual rdf:about="http://purl.org/dc/terms/UDC">
        <rdf:type rdf:resource="http://purl.org/dc/dcam/VocabularyEncodingScheme"/>
        <dcterms:issued rdf:datatype="http://www.w3.org/2001/XMLSchema#date">2000-07-11</dcterms:issued>
        <dcterms:modified rdf:datatype="http://www.w3.org/2001/XMLSchema#date">2008-01-14</dcterms:modified>
        <dcterms:hasVersion rdf:resource="http://dublincore.org/usage/terms/history/#UDC-003"/>
        <rdfs:comment xml:lang="en">The set of conceptual resources specified by the Universal Decimal Classification.</rdfs:comment>
        <rdfs:isDefinedBy rdf:resource="http://purl.org/dc/terms/"/>
        <rdfs:label xml:lang="en">UDC</rdfs:label>
        <rdfs:seeAlso rdf:resource="http://www.udcc.org/"/>
    </owl:NamedIndividual>
    


    <!-- http://purl.org/dc/terms/URI -->

    <owl:NamedIndividual rdf:about="http://purl.org/dc/terms/URI">
        <dcterms:issued rdf:datatype="http://www.w3.org/2001/XMLSchema#date">2000-07-11</dcterms:issued>
        <dcterms:modified rdf:datatype="http://www.w3.org/2001/XMLSchema#date">2008-01-14</dcterms:modified>
    </owl:NamedIndividual>
    


    <!-- http://purl.org/dc/terms/W3CDTF -->

    <owl:NamedIndividual rdf:about="http://purl.org/dc/terms/W3CDTF">
        <dcterms:issued rdf:datatype="http://www.w3.org/2001/XMLSchema#date">2000-07-11</dcterms:issued>
        <dcterms:modified rdf:datatype="http://www.w3.org/2001/XMLSchema#date">2008-01-14</dcterms:modified>
    </owl:NamedIndividual>
    


    <!-- http://purl.org/dc/terms/abstract -->

    <owl:NamedIndividual rdf:about="http://purl.org/dc/terms/abstract">
        <dcterms:issued rdf:datatype="http://www.w3.org/2001/XMLSchema#date">2000-07-11</dcterms:issued>
        <dcterms:modified rdf:datatype="http://www.w3.org/2001/XMLSchema#date">2008-01-14</dcterms:modified>
    </owl:NamedIndividual>
    


    <!-- http://purl.org/dc/terms/accessRights -->

    <owl:NamedIndividual rdf:about="http://purl.org/dc/terms/accessRights">
        <dcterms:issued rdf:datatype="http://www.w3.org/2001/XMLSchema#date">2003-02-15</dcterms:issued>
        <dcterms:modified rdf:datatype="http://www.w3.org/2001/XMLSchema#date">2008-01-14</dcterms:modified>
    </owl:NamedIndividual>
    


    <!-- http://purl.org/dc/terms/accrualMethod -->

    <owl:NamedIndividual rdf:about="http://purl.org/dc/terms/accrualMethod">
        <dcterms:issued rdf:datatype="http://www.w3.org/2001/XMLSchema#date">2005-06-13</dcterms:issued>
        <dcterms:modified rdf:datatype="http://www.w3.org/2001/XMLSchema#date">2010-10-11</dcterms:modified>
    </owl:NamedIndividual>
    


    <!-- http://purl.org/dc/terms/accrualPeriodicity -->

    <owl:NamedIndividual rdf:about="http://purl.org/dc/terms/accrualPeriodicity">
        <dcterms:issued rdf:datatype="http://www.w3.org/2001/XMLSchema#date">2005-06-13</dcterms:issued>
        <dcterms:modified rdf:datatype="http://www.w3.org/2001/XMLSchema#date">2010-10-11</dcterms:modified>
    </owl:NamedIndividual>
    


    <!-- http://purl.org/dc/terms/accrualPolicy -->

    <owl:NamedIndividual rdf:about="http://purl.org/dc/terms/accrualPolicy">
        <dcterms:issued rdf:datatype="http://www.w3.org/2001/XMLSchema#date">2005-06-13</dcterms:issued>
        <dcterms:modified rdf:datatype="http://www.w3.org/2001/XMLSchema#date">2010-10-11</dcterms:modified>
    </owl:NamedIndividual>
    


    <!-- http://purl.org/dc/terms/alternative -->

    <owl:NamedIndividual rdf:about="http://purl.org/dc/terms/alternative">
        <dcterms:issued rdf:datatype="http://www.w3.org/2001/XMLSchema#date">2000-07-11</dcterms:issued>
        <dcterms:modified rdf:datatype="http://www.w3.org/2001/XMLSchema#date">2010-10-11</dcterms:modified>
    </owl:NamedIndividual>
    


    <!-- http://purl.org/dc/terms/audience -->

    <owl:NamedIndividual rdf:about="http://purl.org/dc/terms/audience">
        <dcterms:issued rdf:datatype="http://www.w3.org/2001/XMLSchema#date">2001-05-21</dcterms:issued>
        <dcterms:modified rdf:datatype="http://www.w3.org/2001/XMLSchema#date">2008-01-14</dcterms:modified>
    </owl:NamedIndividual>
    


    <!-- http://purl.org/dc/terms/available -->

    <owl:NamedIndividual rdf:about="http://purl.org/dc/terms/available">
        <dcterms:issued rdf:datatype="http://www.w3.org/2001/XMLSchema#date">2000-07-11</dcterms:issued>
        <dcterms:modified rdf:datatype="http://www.w3.org/2001/XMLSchema#date">2008-01-14</dcterms:modified>
    </owl:NamedIndividual>
    


    <!-- http://purl.org/dc/terms/bibliographicCitation -->

    <owl:NamedIndividual rdf:about="http://purl.org/dc/terms/bibliographicCitation">
        <dcterms:issued rdf:datatype="http://www.w3.org/2001/XMLSchema#date">2003-02-15</dcterms:issued>
        <dcterms:modified rdf:datatype="http://www.w3.org/2001/XMLSchema#date">2008-01-14</dcterms:modified>
    </owl:NamedIndividual>
    


    <!-- http://purl.org/dc/terms/conformsTo -->

    <owl:NamedIndividual rdf:about="http://purl.org/dc/terms/conformsTo">
        <dcterms:issued rdf:datatype="http://www.w3.org/2001/XMLSchema#date">2001-05-21</dcterms:issued>
        <dcterms:modified rdf:datatype="http://www.w3.org/2001/XMLSchema#date">2008-01-14</dcterms:modified>
    </owl:NamedIndividual>
    


    <!-- http://purl.org/dc/terms/contributor -->

    <owl:NamedIndividual rdf:about="http://purl.org/dc/terms/contributor">
        <dcterms:issued rdf:datatype="http://www.w3.org/2001/XMLSchema#date">2008-01-14</dcterms:issued>
        <dcterms:modified rdf:datatype="http://www.w3.org/2001/XMLSchema#date">2010-10-11</dcterms:modified>
    </owl:NamedIndividual>
    


    <!-- http://purl.org/dc/terms/coverage -->

    <owl:NamedIndividual rdf:about="http://purl.org/dc/terms/coverage">
        <dcterms:issued rdf:datatype="http://www.w3.org/2001/XMLSchema#date">2008-01-14</dcterms:issued>
        <dcterms:modified rdf:datatype="http://www.w3.org/2001/XMLSchema#date">2008-01-14</dcterms:modified>
    </owl:NamedIndividual>
    


    <!-- http://purl.org/dc/terms/created -->

    <owl:NamedIndividual rdf:about="http://purl.org/dc/terms/created">
        <dcterms:issued rdf:datatype="http://www.w3.org/2001/XMLSchema#date">2000-07-11</dcterms:issued>
        <dcterms:modified rdf:datatype="http://www.w3.org/2001/XMLSchema#date">2008-01-14</dcterms:modified>
    </owl:NamedIndividual>
    


    <!-- http://purl.org/dc/terms/creator -->

    <owl:NamedIndividual rdf:about="http://purl.org/dc/terms/creator">
        <dcterms:issued rdf:datatype="http://www.w3.org/2001/XMLSchema#date">2008-01-14</dcterms:issued>
        <dcterms:modified rdf:datatype="http://www.w3.org/2001/XMLSchema#date">2010-10-11</dcterms:modified>
    </owl:NamedIndividual>
    


    <!-- http://purl.org/dc/terms/date -->

    <owl:NamedIndividual rdf:about="http://purl.org/dc/terms/date">
        <dcterms:issued rdf:datatype="http://www.w3.org/2001/XMLSchema#date">2008-01-14</dcterms:issued>
        <dcterms:modified rdf:datatype="http://www.w3.org/2001/XMLSchema#date">2008-01-14</dcterms:modified>
    </owl:NamedIndividual>
    


    <!-- http://purl.org/dc/terms/dateAccepted -->

    <owl:NamedIndividual rdf:about="http://purl.org/dc/terms/dateAccepted">
        <dcterms:issued rdf:datatype="http://www.w3.org/2001/XMLSchema#date">2002-07-13</dcterms:issued>
        <dcterms:modified rdf:datatype="http://www.w3.org/2001/XMLSchema#date">2008-01-14</dcterms:modified>
    </owl:NamedIndividual>
    


    <!-- http://purl.org/dc/terms/dateCopyrighted -->

    <owl:NamedIndividual rdf:about="http://purl.org/dc/terms/dateCopyrighted">
        <dcterms:issued rdf:datatype="http://www.w3.org/2001/XMLSchema#date">2002-07-13</dcterms:issued>
        <dcterms:modified rdf:datatype="http://www.w3.org/2001/XMLSchema#date">2008-01-14</dcterms:modified>
    </owl:NamedIndividual>
    


    <!-- http://purl.org/dc/terms/dateSubmitted -->

    <owl:NamedIndividual rdf:about="http://purl.org/dc/terms/dateSubmitted">
        <dcterms:issued rdf:datatype="http://www.w3.org/2001/XMLSchema#date">2002-07-13</dcterms:issued>
        <dcterms:modified rdf:datatype="http://www.w3.org/2001/XMLSchema#date">2008-01-14</dcterms:modified>
    </owl:NamedIndividual>
    


    <!-- http://purl.org/dc/terms/description -->

    <owl:NamedIndividual rdf:about="http://purl.org/dc/terms/description">
        <dcterms:issued rdf:datatype="http://www.w3.org/2001/XMLSchema#date">2008-01-14</dcterms:issued>
        <dcterms:modified rdf:datatype="http://www.w3.org/2001/XMLSchema#date">2008-01-14</dcterms:modified>
    </owl:NamedIndividual>
    


    <!-- http://purl.org/dc/terms/educationLevel -->

    <owl:NamedIndividual rdf:about="http://purl.org/dc/terms/educationLevel">
        <dcterms:issued rdf:datatype="http://www.w3.org/2001/XMLSchema#date">2002-07-13</dcterms:issued>
        <dcterms:modified rdf:datatype="http://www.w3.org/2001/XMLSchema#date">2008-01-14</dcterms:modified>
    </owl:NamedIndividual>
    


    <!-- http://purl.org/dc/terms/extent -->

    <owl:NamedIndividual rdf:about="http://purl.org/dc/terms/extent">
        <dcterms:issued rdf:datatype="http://www.w3.org/2001/XMLSchema#date">2000-07-11</dcterms:issued>
        <dcterms:modified rdf:datatype="http://www.w3.org/2001/XMLSchema#date">2008-01-14</dcterms:modified>
    </owl:NamedIndividual>
    


    <!-- http://purl.org/dc/terms/format -->

    <owl:NamedIndividual rdf:about="http://purl.org/dc/terms/format">
        <dcterms:issued rdf:datatype="http://www.w3.org/2001/XMLSchema#date">2008-01-14</dcterms:issued>
        <dcterms:modified rdf:datatype="http://www.w3.org/2001/XMLSchema#date">2008-01-14</dcterms:modified>
    </owl:NamedIndividual>
    


    <!-- http://purl.org/dc/terms/hasFormat -->

    <owl:NamedIndividual rdf:about="http://purl.org/dc/terms/hasFormat">
        <dcterms:issued rdf:datatype="http://www.w3.org/2001/XMLSchema#date">2000-07-11</dcterms:issued>
        <dcterms:modified rdf:datatype="http://www.w3.org/2001/XMLSchema#date">2008-01-14</dcterms:modified>
    </owl:NamedIndividual>
    


    <!-- http://purl.org/dc/terms/hasPart -->

    <owl:NamedIndividual rdf:about="http://purl.org/dc/terms/hasPart">
        <dcterms:issued rdf:datatype="http://www.w3.org/2001/XMLSchema#date">2000-07-11</dcterms:issued>
        <dcterms:modified rdf:datatype="http://www.w3.org/2001/XMLSchema#date">2008-01-14</dcterms:modified>
    </owl:NamedIndividual>
    


    <!-- http://purl.org/dc/terms/hasVersion -->

    <owl:NamedIndividual rdf:about="http://purl.org/dc/terms/hasVersion">
        <dcterms:issued rdf:datatype="http://www.w3.org/2001/XMLSchema#date">2000-07-11</dcterms:issued>
        <dcterms:modified rdf:datatype="http://www.w3.org/2001/XMLSchema#date">2008-01-14</dcterms:modified>
    </owl:NamedIndividual>
    


    <!-- http://purl.org/dc/terms/identifier -->

    <owl:NamedIndividual rdf:about="http://purl.org/dc/terms/identifier">
        <dcterms:issued rdf:datatype="http://www.w3.org/2001/XMLSchema#date">2008-01-14</dcterms:issued>
        <dcterms:modified rdf:datatype="http://www.w3.org/2001/XMLSchema#date">2008-01-14</dcterms:modified>
    </owl:NamedIndividual>
    


    <!-- http://purl.org/dc/terms/instructionalMethod -->

    <owl:NamedIndividual rdf:about="http://purl.org/dc/terms/instructionalMethod">
        <dcterms:issued rdf:datatype="http://www.w3.org/2001/XMLSchema#date">2005-06-13</dcterms:issued>
        <dcterms:modified rdf:datatype="http://www.w3.org/2001/XMLSchema#date">2008-01-14</dcterms:modified>
    </owl:NamedIndividual>
    


    <!-- http://purl.org/dc/terms/isFormatOf -->

    <owl:NamedIndividual rdf:about="http://purl.org/dc/terms/isFormatOf">
        <dcterms:issued rdf:datatype="http://www.w3.org/2001/XMLSchema#date">2000-07-11</dcterms:issued>
        <dcterms:modified rdf:datatype="http://www.w3.org/2001/XMLSchema#date">2008-01-14</dcterms:modified>
    </owl:NamedIndividual>
    


    <!-- http://purl.org/dc/terms/isPartOf -->

    <owl:NamedIndividual rdf:about="http://purl.org/dc/terms/isPartOf">
        <dcterms:issued rdf:datatype="http://www.w3.org/2001/XMLSchema#date">2000-07-11</dcterms:issued>
        <dcterms:modified rdf:datatype="http://www.w3.org/2001/XMLSchema#date">2008-01-14</dcterms:modified>
    </owl:NamedIndividual>
    


    <!-- http://purl.org/dc/terms/isReferencedBy -->

    <owl:NamedIndividual rdf:about="http://purl.org/dc/terms/isReferencedBy">
        <dcterms:issued rdf:datatype="http://www.w3.org/2001/XMLSchema#date">2000-07-11</dcterms:issued>
        <dcterms:modified rdf:datatype="http://www.w3.org/2001/XMLSchema#date">2008-01-14</dcterms:modified>
    </owl:NamedIndividual>
    


    <!-- http://purl.org/dc/terms/isReplacedBy -->

    <owl:NamedIndividual rdf:about="http://purl.org/dc/terms/isReplacedBy">
        <dcterms:issued rdf:datatype="http://www.w3.org/2001/XMLSchema#date">2000-07-11</dcterms:issued>
        <dcterms:modified rdf:datatype="http://www.w3.org/2001/XMLSchema#date">2008-01-14</dcterms:modified>
    </owl:NamedIndividual>
    


    <!-- http://purl.org/dc/terms/isRequiredBy -->

    <owl:NamedIndividual rdf:about="http://purl.org/dc/terms/isRequiredBy">
        <dcterms:issued rdf:datatype="http://www.w3.org/2001/XMLSchema#date">2000-07-11</dcterms:issued>
        <dcterms:modified rdf:datatype="http://www.w3.org/2001/XMLSchema#date">2008-01-14</dcterms:modified>
    </owl:NamedIndividual>
    


    <!-- http://purl.org/dc/terms/isVersionOf -->

    <owl:NamedIndividual rdf:about="http://purl.org/dc/terms/isVersionOf">
        <dcterms:issued rdf:datatype="http://www.w3.org/2001/XMLSchema#date">2000-07-11</dcterms:issued>
        <dcterms:modified rdf:datatype="http://www.w3.org/2001/XMLSchema#date">2008-01-14</dcterms:modified>
    </owl:NamedIndividual>
    


    <!-- http://purl.org/dc/terms/issued -->

    <owl:DatatypeProperty rdf:about="http://purl.org/dc/terms/issued">
        <rdf:type rdf:resource="http://www.w3.org/2002/07/owl#NamedIndividual"/>
        <dcterms:issued rdf:datatype="http://www.w3.org/2001/XMLSchema#date">2000-07-11</dcterms:issued>
        <dcterms:modified rdf:datatype="http://www.w3.org/2001/XMLSchema#date">2008-01-14</dcterms:modified>
    </owl:DatatypeProperty>
    


    <!-- http://purl.org/dc/terms/language -->

    <owl:NamedIndividual rdf:about="http://purl.org/dc/terms/language">
        <dcterms:issued rdf:datatype="http://www.w3.org/2001/XMLSchema#date">2008-01-14</dcterms:issued>
        <dcterms:modified rdf:datatype="http://www.w3.org/2001/XMLSchema#date">2008-01-14</dcterms:modified>
    </owl:NamedIndividual>
    


    <!-- http://purl.org/dc/terms/license -->

    <owl:NamedIndividual rdf:about="http://purl.org/dc/terms/license">
        <dcterms:issued rdf:datatype="http://www.w3.org/2001/XMLSchema#date">2004-06-14</dcterms:issued>
        <dcterms:modified rdf:datatype="http://www.w3.org/2001/XMLSchema#date">2008-01-14</dcterms:modified>
    </owl:NamedIndividual>
    


    <!-- http://purl.org/dc/terms/mediator -->

    <owl:NamedIndividual rdf:about="http://purl.org/dc/terms/mediator">
        <dcterms:issued rdf:datatype="http://www.w3.org/2001/XMLSchema#date">2001-05-21</dcterms:issued>
        <dcterms:modified rdf:datatype="http://www.w3.org/2001/XMLSchema#date">2008-01-14</dcterms:modified>
    </owl:NamedIndividual>
    


    <!-- http://purl.org/dc/terms/medium -->

    <owl:NamedIndividual rdf:about="http://purl.org/dc/terms/medium">
        <dcterms:issued rdf:datatype="http://www.w3.org/2001/XMLSchema#date">2000-07-11</dcterms:issued>
        <dcterms:modified rdf:datatype="http://www.w3.org/2001/XMLSchema#date">2008-01-14</dcterms:modified>
    </owl:NamedIndividual>
    


    <!-- http://purl.org/dc/terms/modified -->

    <owl:DatatypeProperty rdf:about="http://purl.org/dc/terms/modified">
        <rdf:type rdf:resource="http://www.w3.org/2002/07/owl#NamedIndividual"/>
        <dcterms:issued rdf:datatype="http://www.w3.org/2001/XMLSchema#date">2000-07-11</dcterms:issued>
        <dcterms:modified rdf:datatype="http://www.w3.org/2001/XMLSchema#date">2008-01-14</dcterms:modified>
    </owl:DatatypeProperty>
    


    <!-- http://purl.org/dc/terms/provenance -->

    <owl:NamedIndividual rdf:about="http://purl.org/dc/terms/provenance">
        <dcterms:issued rdf:datatype="http://www.w3.org/2001/XMLSchema#date">2004-09-20</dcterms:issued>
        <dcterms:modified rdf:datatype="http://www.w3.org/2001/XMLSchema#date">2008-01-14</dcterms:modified>
    </owl:NamedIndividual>
    


    <!-- http://purl.org/dc/terms/publisher -->

    <owl:NamedIndividual rdf:about="http://purl.org/dc/terms/publisher">
        <dcterms:issued rdf:datatype="http://www.w3.org/2001/XMLSchema#date">2008-01-14</dcterms:issued>
        <dcterms:modified rdf:datatype="http://www.w3.org/2001/XMLSchema#date">2010-10-11</dcterms:modified>
    </owl:NamedIndividual>
    


    <!-- http://purl.org/dc/terms/references -->

    <owl:NamedIndividual rdf:about="http://purl.org/dc/terms/references">
        <dcterms:issued rdf:datatype="http://www.w3.org/2001/XMLSchema#date">2000-07-11</dcterms:issued>
        <dcterms:modified rdf:datatype="http://www.w3.org/2001/XMLSchema#date">2008-01-14</dcterms:modified>
    </owl:NamedIndividual>
    


    <!-- http://purl.org/dc/terms/relation -->

    <owl:NamedIndividual rdf:about="http://purl.org/dc/terms/relation">
        <dcterms:issued rdf:datatype="http://www.w3.org/2001/XMLSchema#date">2008-01-14</dcterms:issued>
        <dcterms:modified rdf:datatype="http://www.w3.org/2001/XMLSchema#date">2008-01-14</dcterms:modified>
    </owl:NamedIndividual>
    


    <!-- http://purl.org/dc/terms/replaces -->

    <owl:NamedIndividual rdf:about="http://purl.org/dc/terms/replaces">
        <dcterms:issued rdf:datatype="http://www.w3.org/2001/XMLSchema#date">2000-07-11</dcterms:issued>
        <dcterms:modified rdf:datatype="http://www.w3.org/2001/XMLSchema#date">2008-01-14</dcterms:modified>
    </owl:NamedIndividual>
    


    <!-- http://purl.org/dc/terms/requires -->

    <owl:NamedIndividual rdf:about="http://purl.org/dc/terms/requires">
        <dcterms:issued rdf:datatype="http://www.w3.org/2001/XMLSchema#date">2000-07-11</dcterms:issued>
        <dcterms:modified rdf:datatype="http://www.w3.org/2001/XMLSchema#date">2008-01-14</dcterms:modified>
    </owl:NamedIndividual>
    


    <!-- http://purl.org/dc/terms/rights -->

    <owl:NamedIndividual rdf:about="http://purl.org/dc/terms/rights">
        <dcterms:issued rdf:datatype="http://www.w3.org/2001/XMLSchema#date">2008-01-14</dcterms:issued>
        <dcterms:modified rdf:datatype="http://www.w3.org/2001/XMLSchema#date">2008-01-14</dcterms:modified>
    </owl:NamedIndividual>
    


    <!-- http://purl.org/dc/terms/rightsHolder -->

    <owl:NamedIndividual rdf:about="http://purl.org/dc/terms/rightsHolder">
        <dcterms:issued rdf:datatype="http://www.w3.org/2001/XMLSchema#date">2004-06-14</dcterms:issued>
        <dcterms:modified rdf:datatype="http://www.w3.org/2001/XMLSchema#date">2008-01-14</dcterms:modified>
    </owl:NamedIndividual>
    


    <!-- http://purl.org/dc/terms/source -->

    <owl:NamedIndividual rdf:about="http://purl.org/dc/terms/source">
        <dcterms:issued rdf:datatype="http://www.w3.org/2001/XMLSchema#date">2008-01-14</dcterms:issued>
        <dcterms:modified rdf:datatype="http://www.w3.org/2001/XMLSchema#date">2008-01-14</dcterms:modified>
    </owl:NamedIndividual>
    


    <!-- http://purl.org/dc/terms/spatial -->

    <owl:NamedIndividual rdf:about="http://purl.org/dc/terms/spatial">
        <dcterms:issued rdf:datatype="http://www.w3.org/2001/XMLSchema#date">2000-07-11</dcterms:issued>
        <dcterms:modified rdf:datatype="http://www.w3.org/2001/XMLSchema#date">2008-01-14</dcterms:modified>
    </owl:NamedIndividual>
    


    <!-- http://purl.org/dc/terms/subject -->

    <owl:NamedIndividual rdf:about="http://purl.org/dc/terms/subject">
        <dcterms:issued rdf:datatype="http://www.w3.org/2001/XMLSchema#date">2008-01-14</dcterms:issued>
        <dcterms:modified rdf:datatype="http://www.w3.org/2001/XMLSchema#date">2012-06-14</dcterms:modified>
    </owl:NamedIndividual>
    


    <!-- http://purl.org/dc/terms/tableOfContents -->

    <owl:NamedIndividual rdf:about="http://purl.org/dc/terms/tableOfContents">
        <dcterms:issued rdf:datatype="http://www.w3.org/2001/XMLSchema#date">2000-07-11</dcterms:issued>
        <dcterms:modified rdf:datatype="http://www.w3.org/2001/XMLSchema#date">2008-01-14</dcterms:modified>
    </owl:NamedIndividual>
    


    <!-- http://purl.org/dc/terms/temporal -->

    <owl:NamedIndividual rdf:about="http://purl.org/dc/terms/temporal">
        <dcterms:issued rdf:datatype="http://www.w3.org/2001/XMLSchema#date">2000-07-11</dcterms:issued>
        <dcterms:modified rdf:datatype="http://www.w3.org/2001/XMLSchema#date">2008-01-14</dcterms:modified>
    </owl:NamedIndividual>
    


    <!-- http://purl.org/dc/terms/title -->

    <owl:NamedIndividual rdf:about="http://purl.org/dc/terms/title">
        <dcterms:issued rdf:datatype="http://www.w3.org/2001/XMLSchema#date">2008-01-14</dcterms:issued>
        <dcterms:modified rdf:datatype="http://www.w3.org/2001/XMLSchema#date">2010-10-11</dcterms:modified>
    </owl:NamedIndividual>
    


    <!-- http://purl.org/dc/terms/type -->

    <owl:NamedIndividual rdf:about="http://purl.org/dc/terms/type">
        <dcterms:issued rdf:datatype="http://www.w3.org/2001/XMLSchema#date">2008-01-14</dcterms:issued>
        <dcterms:modified rdf:datatype="http://www.w3.org/2001/XMLSchema#date">2008-01-14</dcterms:modified>
    </owl:NamedIndividual>
    


    <!-- http://purl.org/dc/terms/valid -->

    <owl:NamedIndividual rdf:about="http://purl.org/dc/terms/valid">
        <dcterms:issued rdf:datatype="http://www.w3.org/2001/XMLSchema#date">2000-07-11</dcterms:issued>
        <dcterms:modified rdf:datatype="http://www.w3.org/2001/XMLSchema#date">2008-01-14</dcterms:modified>
    </owl:NamedIndividual>
    


    <!-- http://purl.org/ontology/po/ -->

    <owl:NamedIndividual rdf:about="http://purl.org/ontology/po/">
        <rdf:type rdf:resource="http://www.bbc.co.uk/ontologies/provenance/Ontology"/>
        <contributor rdf:resource="http://metade.org/foaf.rdf#me"/>
        <contributor rdf:resource="http://smethur.st/#me"/>
        <contributor rdf:resource="http://www.aelius.com/njh#me"/>
        <dcterms:license rdf:resource="http://creativecommons.org/licenses/by/4.0#id"/>
        <date>2009/02/20 16:00:00</date>
    </owl:NamedIndividual>
    


    <!-- http://smethur.st/#me -->

    <owl:NamedIndividual rdf:about="http://smethur.st/#me"/>
    


    <!-- http://www.aelius.com/njh#me -->

    <owl:NamedIndividual rdf:about="http://www.aelius.com/njh#me"/>
    


    <!-- 
    ///////////////////////////////////////////////////////////////////////////////////////
    //
    // Annotations
    //
    ///////////////////////////////////////////////////////////////////////////////////////
     -->

    <rdf:Description rdf:about="http://purl.org/dc/elements/1.1/">
        <dcterms:publisher rdf:resource="http://purl.org/dc/aboutdcmi#DCMI"/>
        <dcterms:title xml:lang="en">Dublin Core Metadata Element Set, Version 1.1</dcterms:title>
        <dcterms:modified rdf:datatype="http://www.w3.org/2001/XMLSchema#date">2012-06-14</dcterms:modified>
    </rdf:Description>
    <rdf:Description rdf:about="http://purl.org/dc/elements/1.1/contributor">
        <rdfs:label xml:lang="en">Contributor</rdfs:label>
        <dcterms:hasVersion rdf:resource="http://dublincore.org/usage/terms/history/#contributor-006"/>
        <skos:note xml:lang="en">A second property with the same name as this property has been declared in the dcterms: namespace (http://purl.org/dc/terms/).  See the Introduction to the document &quot;DCMI Metadata Terms&quot; (http://dublincore.org/documents/dcmi-terms/) for an explanation.</skos:note>
        <rdfs:comment xml:lang="en">An entity responsible for making contributions to the resource.</rdfs:comment>
        <dcterms:description xml:lang="en">Examples of a Contributor include a person, an organization, or a service. Typically, the name of a Contributor should be used to indicate the entity.</dcterms:description>
        <dcterms:modified rdf:datatype="http://www.w3.org/2001/XMLSchema#date">2008-01-14</dcterms:modified>
        <dcterms:issued rdf:datatype="http://www.w3.org/2001/XMLSchema#date">1999-07-02</dcterms:issued>
        <rdfs:isDefinedBy rdf:resource="http://purl.org/dc/elements/1.1/"/>
    </rdf:Description>
    <rdf:Description rdf:about="http://purl.org/dc/elements/1.1/date">
        <skos:note xml:lang="en">A second property with the same name as this property has been declared in the dcterms: namespace (http://purl.org/dc/terms/).  See the Introduction to the document &quot;DCMI Metadata Terms&quot; (http://dublincore.org/documents/dcmi-terms/) for an explanation.</skos:note>
        <dcterms:issued rdf:datatype="http://www.w3.org/2001/XMLSchema#date">1999-07-02</dcterms:issued>
        <dcterms:modified rdf:datatype="http://www.w3.org/2001/XMLSchema#date">2008-01-14</dcterms:modified>
        <rdfs:isDefinedBy rdf:resource="http://purl.org/dc/elements/1.1/"/>
        <dcterms:hasVersion rdf:resource="http://dublincore.org/usage/terms/history/#date-006"/>
        <rdfs:comment xml:lang="en">A point or period of time associated with an event in the lifecycle of the resource.</rdfs:comment>
        <dcterms:description xml:lang="en">Date may be used to express temporal information at any level of granularity.  Recommended best practice is to use an encoding scheme, such as the W3CDTF profile of ISO 8601 [W3CDTF].</dcterms:description>
        <rdfs:label xml:lang="en">Date</rdfs:label>
    </rdf:Description>
    <rdf:Description rdf:about="http://purl.org/dc/terms/Agent">
        <rdfs:label xml:lang="en">Agent</rdfs:label>
        <rdfs:comment xml:lang="en">A resource that acts or has the power to act.</rdfs:comment>
        <rdfs:isDefinedBy rdf:resource="http://purl.org/dc/terms/"/>
        <dcterms:description xml:lang="en">Examples of Agent include person, organization, and software agent.</dcterms:description>
        <dcterms:hasVersion rdf:resource="http://dublincore.org/usage/terms/history/#Agent-001"/>
    </rdf:Description>
    <rdf:Description rdf:about="http://purl.org/dc/terms/AgentClass">
        <rdfs:isDefinedBy rdf:resource="http://purl.org/dc/terms/"/>
        <rdfs:label xml:lang="en">Agent Class</rdfs:label>
        <rdfs:comment xml:lang="en">A group of agents.</rdfs:comment>
        <dcterms:description xml:lang="en">Examples of Agent Class include groups seen as classes, such as students, women, charities, lecturers.</dcterms:description>
        <dcterms:hasVersion rdf:resource="http://dublincore.org/usage/terms/history/#AgentClass-003"/>
    </rdf:Description>
    <rdf:Description rdf:about="http://purl.org/dc/terms/BibliographicResource">
        <rdfs:isDefinedBy rdf:resource="http://purl.org/dc/terms/"/>
        <dcterms:hasVersion rdf:resource="http://dublincore.org/usage/terms/history/#BibliographicResource-001"/>
        <rdfs:comment xml:lang="en">A book, article, or other documentary resource.</rdfs:comment>
        <rdfs:label xml:lang="en">Bibliographic Resource</rdfs:label>
    </rdf:Description>
    <rdf:Description rdf:about="http://purl.org/dc/terms/Box">
        <rdfs:comment xml:lang="en">The set of regions in space defined by their geographic coordinates according to the DCMI Box Encoding Scheme.</rdfs:comment>
        <rdfs:isDefinedBy rdf:resource="http://purl.org/dc/terms/"/>
        <rdfs:label xml:lang="en">DCMI Box</rdfs:label>
        <rdfs:seeAlso rdf:resource="http://dublincore.org/documents/dcmi-box/"/>
        <dcterms:hasVersion rdf:resource="http://dublincore.org/usage/terms/history/#Box-003"/>
    </rdf:Description>
    <rdf:Description rdf:about="http://purl.org/dc/terms/FileFormat">
        <dcterms:description xml:lang="en">Examples include the formats defined by the list of Internet Media Types.</dcterms:description>
        <dcterms:hasVersion rdf:resource="http://dublincore.org/usage/terms/history/#FileFormat-001"/>
        <rdfs:label xml:lang="en">File Format</rdfs:label>
        <rdfs:comment xml:lang="en">A digital resource format.</rdfs:comment>
        <rdfs:isDefinedBy rdf:resource="http://purl.org/dc/terms/"/>
    </rdf:Description>
    <rdf:Description rdf:about="http://purl.org/dc/terms/Frequency">
        <rdfs:label xml:lang="en">Frequency</rdfs:label>
        <dcterms:hasVersion rdf:resource="http://dublincore.org/usage/terms/history/#Frequency-001"/>
        <rdfs:isDefinedBy rdf:resource="http://purl.org/dc/terms/"/>
        <rdfs:comment xml:lang="en">A rate at which something recurs.</rdfs:comment>
    </rdf:Description>
    <rdf:Description rdf:about="http://purl.org/dc/terms/ISO3166">
        <rdfs:comment xml:lang="en">The set of codes listed in ISO 3166-1 for the representation of names of countries.</rdfs:comment>
        <dcterms:hasVersion rdf:resource="http://dublincore.org/usage/terms/history/#ISO3166-004"/>
        <rdfs:isDefinedBy rdf:resource="http://purl.org/dc/terms/"/>
        <rdfs:label xml:lang="en">ISO 3166</rdfs:label>
        <rdfs:seeAlso rdf:resource="http://www.iso.org/iso/en/prods-services/iso3166ma/02iso-3166-code-lists/list-en1.html"/>
    </rdf:Description>
    <rdf:Description rdf:about="http://purl.org/dc/terms/ISO639-2">
        <rdfs:seeAlso rdf:resource="http://lcweb.loc.gov/standards/iso639-2/langhome.html"/>
        <rdfs:comment xml:lang="en">The three-letter alphabetic codes listed in ISO639-2 for the representation of names of languages.</rdfs:comment>
        <rdfs:isDefinedBy rdf:resource="http://purl.org/dc/terms/"/>
        <rdfs:label xml:lang="en">ISO 639-2</rdfs:label>
        <dcterms:hasVersion rdf:resource="http://dublincore.org/usage/terms/history/#ISO639-2-003"/>
    </rdf:Description>
    <rdf:Description rdf:about="http://purl.org/dc/terms/ISO639-3">
        <rdfs:comment xml:lang="en">The set of three-letter codes listed in ISO 639-3 for the representation of names of languages.</rdfs:comment>
        <rdfs:label xml:lang="en">ISO 639-3</rdfs:label>
        <rdfs:isDefinedBy rdf:resource="http://purl.org/dc/terms/"/>
        <dcterms:hasVersion rdf:resource="http://dublincore.org/usage/terms/history/#ISO639-3-001"/>
        <rdfs:seeAlso rdf:resource="http://www.sil.org/iso639-3/"/>
    </rdf:Description>
    <rdf:Description rdf:about="http://purl.org/dc/terms/Jurisdiction">
        <dcterms:hasVersion rdf:resource="http://dublincore.org/usage/terms/history/#Jurisdiction-001"/>
        <rdfs:label xml:lang="en">Jurisdiction</rdfs:label>
        <rdfs:isDefinedBy rdf:resource="http://purl.org/dc/terms/"/>
        <rdfs:comment xml:lang="en">The extent or range of judicial, law enforcement, or other authority.</rdfs:comment>
    </rdf:Description>
    <rdf:Description rdf:about="http://purl.org/dc/terms/LicenseDocument">
        <rdfs:label xml:lang="en">License Document</rdfs:label>
        <rdfs:isDefinedBy rdf:resource="http://purl.org/dc/terms/"/>
        <rdfs:comment xml:lang="en">A legal document giving official permission to do something with a Resource.</rdfs:comment>
        <dcterms:hasVersion rdf:resource="http://dublincore.org/usage/terms/history/#LicenseDocument-001"/>
    </rdf:Description>
    <rdf:Description rdf:about="http://purl.org/dc/terms/LinguisticSystem">
        <dcterms:hasVersion rdf:resource="http://dublincore.org/usage/terms/history/#LinguisticSystem-001"/>
        <dcterms:description xml:lang="en">Examples include written, spoken, sign, and computer languages.</dcterms:description>
        <rdfs:isDefinedBy rdf:resource="http://purl.org/dc/terms/"/>
        <rdfs:comment xml:lang="en">A system of signs, symbols, sounds, gestures, or rules used in communication.</rdfs:comment>
        <rdfs:label xml:lang="en">Linguistic System</rdfs:label>
    </rdf:Description>
    <rdf:Description rdf:about="http://purl.org/dc/terms/Location">
        <dcterms:hasVersion rdf:resource="http://dublincore.org/usage/terms/history/#Location-001"/>
        <rdfs:label xml:lang="en">Location</rdfs:label>
        <rdfs:isDefinedBy rdf:resource="http://purl.org/dc/terms/"/>
        <rdfs:comment xml:lang="en">A spatial region or named place.</rdfs:comment>
    </rdf:Description>
    <rdf:Description rdf:about="http://purl.org/dc/terms/LocationPeriodOrJurisdiction">
        <rdfs:label xml:lang="en">Location, Period, or Jurisdiction</rdfs:label>
        <rdfs:comment xml:lang="en">A location, period of time, or jurisdiction.</rdfs:comment>
        <rdfs:isDefinedBy rdf:resource="http://purl.org/dc/terms/"/>
        <dcterms:hasVersion rdf:resource="http://dublincore.org/usage/terms/history/#LocationPeriodOrJurisdiction-001"/>
    </rdf:Description>
    <rdf:Description rdf:about="http://purl.org/dc/terms/MediaType">
        <rdfs:comment xml:lang="en">A file format or physical medium.</rdfs:comment>
        <rdfs:label xml:lang="en">Media Type</rdfs:label>
        <rdfs:isDefinedBy rdf:resource="http://purl.org/dc/terms/"/>
        <dcterms:hasVersion rdf:resource="http://dublincore.org/usage/terms/history/#MediaType-001"/>
    </rdf:Description>
    <rdf:Description rdf:about="http://purl.org/dc/terms/MediaTypeOrExtent">
        <rdfs:isDefinedBy rdf:resource="http://purl.org/dc/terms/"/>
        <rdfs:comment xml:lang="en">A media type or extent.</rdfs:comment>
        <rdfs:label xml:lang="en">Media Type or Extent</rdfs:label>
        <dcterms:hasVersion rdf:resource="http://dublincore.org/usage/terms/history/#MediaTypeOrExtent-001"/>
    </rdf:Description>
    <rdf:Description rdf:about="http://purl.org/dc/terms/MethodOfAccrual">
        <rdfs:isDefinedBy rdf:resource="http://purl.org/dc/terms/"/>
        <rdfs:comment xml:lang="en">A method by which resources are added to a collection.</rdfs:comment>
        <dcterms:hasVersion rdf:resource="http://dublincore.org/usage/terms/history/#MethodOfAccrual-001"/>
        <rdfs:label xml:lang="en">Method of Accrual</rdfs:label>
    </rdf:Description>
    <rdf:Description rdf:about="http://purl.org/dc/terms/MethodOfInstruction">
        <rdfs:label xml:lang="en">Method of Instruction</rdfs:label>
        <rdfs:comment xml:lang="en">A process that is used to engender knowledge, attitudes, and skills.</rdfs:comment>
        <dcterms:hasVersion rdf:resource="http://dublincore.org/usage/terms/history/#MethodOfInstruction-001"/>
        <rdfs:isDefinedBy rdf:resource="http://purl.org/dc/terms/"/>
    </rdf:Description>
    <rdf:Description rdf:about="http://purl.org/dc/terms/Period">
        <rdfs:comment xml:lang="en">The set of time intervals defined by their limits according to the DCMI Period Encoding Scheme.</rdfs:comment>
        <rdfs:seeAlso rdf:resource="http://dublincore.org/documents/dcmi-period/"/>
        <rdfs:label xml:lang="en">DCMI Period</rdfs:label>
        <rdfs:isDefinedBy rdf:resource="http://purl.org/dc/terms/"/>
        <dcterms:hasVersion rdf:resource="http://dublincore.org/usage/terms/history/#Period-003"/>
    </rdf:Description>
    <rdf:Description rdf:about="http://purl.org/dc/terms/PeriodOfTime">
        <rdfs:comment xml:lang="en">An interval of time that is named or defined by its start and end dates.</rdfs:comment>
        <dcterms:hasVersion rdf:resource="http://dublincore.org/usage/terms/history/#PeriodOfTime-001"/>
        <rdfs:isDefinedBy rdf:resource="http://purl.org/dc/terms/"/>
        <rdfs:label xml:lang="en">Period of Time</rdfs:label>
    </rdf:Description>
    <rdf:Description rdf:about="http://purl.org/dc/terms/PhysicalMedium">
        <dcterms:hasVersion rdf:resource="http://dublincore.org/usage/terms/history/#PhysicalMedium-001"/>
        <dcterms:description xml:lang="en">Examples include paper, canvas, or DVD.</dcterms:description>
        <rdfs:label xml:lang="en">Physical Medium</rdfs:label>
        <rdfs:isDefinedBy rdf:resource="http://purl.org/dc/terms/"/>
        <rdfs:comment xml:lang="en">A physical material or carrier.</rdfs:comment>
    </rdf:Description>
    <rdf:Description rdf:about="http://purl.org/dc/terms/PhysicalResource">
        <rdfs:isDefinedBy rdf:resource="http://purl.org/dc/terms/"/>
        <rdfs:comment xml:lang="en">A material thing.</rdfs:comment>
        <dcterms:hasVersion rdf:resource="http://dublincore.org/usage/terms/history/#PhysicalResource-001"/>
        <rdfs:label xml:lang="en">Physical Resource</rdfs:label>
    </rdf:Description>
    <rdf:Description rdf:about="http://purl.org/dc/terms/Point">
        <rdfs:comment xml:lang="en">The set of points in space defined by their geographic coordinates according to the DCMI Point Encoding Scheme.</rdfs:comment>
        <rdfs:label xml:lang="en">DCMI Point</rdfs:label>
        <dcterms:hasVersion rdf:resource="http://dublincore.org/usage/terms/history/#Point-003"/>
        <rdfs:seeAlso rdf:resource="http://dublincore.org/documents/dcmi-point/"/>
        <rdfs:isDefinedBy rdf:resource="http://purl.org/dc/terms/"/>
    </rdf:Description>
    <rdf:Description rdf:about="http://purl.org/dc/terms/Policy">
        <rdfs:label xml:lang="en">Policy</rdfs:label>
        <rdfs:isDefinedBy rdf:resource="http://purl.org/dc/terms/"/>
        <rdfs:comment xml:lang="en">A plan or course of action by an authority, intended to influence and determine decisions, actions, and other matters.</rdfs:comment>
        <dcterms:hasVersion rdf:resource="http://dublincore.org/usage/terms/history/#Policy-001"/>
    </rdf:Description>
    <rdf:Description rdf:about="http://purl.org/dc/terms/ProvenanceStatement">
        <rdfs:label xml:lang="en">Provenance Statement</rdfs:label>
        <rdfs:isDefinedBy rdf:resource="http://purl.org/dc/terms/"/>
        <dcterms:hasVersion rdf:resource="http://dublincore.org/usage/terms/history/#ProvenanceStatement-001"/>
        <rdfs:comment xml:lang="en">A statement of any changes in ownership and custody of a resource since its creation that are significant for its authenticity, integrity, and interpretation.</rdfs:comment>
    </rdf:Description>
    <rdf:Description rdf:about="http://purl.org/dc/terms/RFC1766">
        <rdfs:isDefinedBy rdf:resource="http://purl.org/dc/terms/"/>
        <rdfs:seeAlso rdf:resource="http://www.ietf.org/rfc/rfc1766.txt"/>
        <rdfs:comment xml:lang="en">The set of tags, constructed according to RFC 1766, for the identification of languages.</rdfs:comment>
        <dcterms:hasVersion rdf:resource="http://dublincore.org/usage/terms/history/#RFC1766-003"/>
        <rdfs:label xml:lang="en">RFC 1766</rdfs:label>
    </rdf:Description>
    <rdf:Description rdf:about="http://purl.org/dc/terms/RFC3066">
        <rdfs:label xml:lang="en">RFC 3066</rdfs:label>
        <rdfs:isDefinedBy rdf:resource="http://purl.org/dc/terms/"/>
        <dcterms:description xml:lang="en">RFC 3066 has been obsoleted by RFC 4646.</dcterms:description>
        <rdfs:comment xml:lang="en">The set of tags constructed according to RFC 3066 for the identification of languages.</rdfs:comment>
        <rdfs:seeAlso rdf:resource="http://www.ietf.org/rfc/rfc3066.txt"/>
        <dcterms:hasVersion rdf:resource="http://dublincore.org/usage/terms/history/#RFC3066-002"/>
    </rdf:Description>
    <rdf:Description rdf:about="http://purl.org/dc/terms/RFC4646">
        <dcterms:description xml:lang="en">RFC 4646 obsoletes RFC 3066.</dcterms:description>
        <dcterms:hasVersion rdf:resource="http://dublincore.org/usage/terms/history/#RFC4646-001"/>
        <rdfs:seeAlso rdf:resource="http://www.ietf.org/rfc/rfc4646.txt"/>
        <rdfs:isDefinedBy rdf:resource="http://purl.org/dc/terms/"/>
        <rdfs:comment xml:lang="en">The set of tags constructed according to RFC 4646 for the identification of languages.</rdfs:comment>
        <rdfs:label xml:lang="en">RFC 4646</rdfs:label>
    </rdf:Description>
    <rdf:Description rdf:about="http://purl.org/dc/terms/RFC5646">
        <rdfs:seeAlso rdf:resource="http://www.ietf.org/rfc/rfc5646.txt"/>
        <dcterms:hasVersion rdf:resource="http://dublincore.org/usage/terms/history/#RFC5646-001"/>
        <rdfs:comment xml:lang="en">The set of tags constructed according to RFC 5646 for the identification of languages.</rdfs:comment>
        <rdfs:label xml:lang="en">RFC 5646</rdfs:label>
        <dcterms:description xml:lang="en">RFC 5646 obsoletes RFC 4646.</dcterms:description>
        <rdfs:isDefinedBy rdf:resource="http://purl.org/dc/terms/"/>
    </rdf:Description>
    <rdf:Description rdf:about="http://purl.org/dc/terms/RightsStatement">
        <rdfs:label xml:lang="en">Rights Statement</rdfs:label>
        <rdfs:isDefinedBy rdf:resource="http://purl.org/dc/terms/"/>
        <rdfs:comment xml:lang="en">A statement about the intellectual property rights (IPR) held in or over a Resource, a legal document giving official permission to do something with a resource, or a statement about access rights.</rdfs:comment>
        <dcterms:hasVersion rdf:resource="http://dublincore.org/usage/terms/history/#RightsStatement-001"/>
    </rdf:Description>
    <rdf:Description rdf:about="http://purl.org/dc/terms/SizeOrDuration">
        <rdfs:label xml:lang="en">Size or Duration</rdfs:label>
        <dcterms:hasVersion rdf:resource="http://dublincore.org/usage/terms/history/#SizeOrDuration-001"/>
        <dcterms:description xml:lang="en">Examples include a number of pages, a specification of length, width, and breadth, or a period in hours, minutes, and seconds.</dcterms:description>
        <rdfs:comment xml:lang="en">A dimension or extent, or a time taken to play or execute.</rdfs:comment>
        <rdfs:isDefinedBy rdf:resource="http://purl.org/dc/terms/"/>
    </rdf:Description>
    <rdf:Description rdf:about="http://purl.org/dc/terms/Standard">
        <rdfs:comment xml:lang="en">A basis for comparison; a reference point against which other things can be evaluated.</rdfs:comment>
        <rdfs:label xml:lang="en">Standard</rdfs:label>
        <rdfs:isDefinedBy rdf:resource="http://purl.org/dc/terms/"/>
        <dcterms:hasVersion rdf:resource="http://dublincore.org/usage/terms/history/#Standard-001"/>
    </rdf:Description>
    <rdf:Description rdf:about="http://purl.org/dc/terms/URI">
        <rdfs:isDefinedBy rdf:resource="http://purl.org/dc/terms/"/>
        <rdfs:comment xml:lang="en">The set of identifiers constructed according to the generic syntax for Uniform Resource Identifiers as specified by the Internet Engineering Task Force.</rdfs:comment>
        <rdfs:seeAlso rdf:resource="http://www.ietf.org/rfc/rfc3986.txt"/>
        <dcterms:hasVersion rdf:resource="http://dublincore.org/usage/terms/history/#URI-003"/>
        <rdfs:label xml:lang="en">URI</rdfs:label>
    </rdf:Description>
    <rdf:Description rdf:about="http://purl.org/dc/terms/W3CDTF">
        <rdfs:label xml:lang="en">W3C-DTF</rdfs:label>
        <rdfs:comment xml:lang="en">The set of dates and times constructed according to the W3C Date and Time Formats Specification.</rdfs:comment>
        <rdfs:isDefinedBy rdf:resource="http://purl.org/dc/terms/"/>
        <dcterms:hasVersion rdf:resource="http://dublincore.org/usage/terms/history/#W3CDTF-003"/>
        <rdfs:seeAlso rdf:resource="http://www.w3.org/TR/NOTE-datetime"/>
    </rdf:Description>
    <rdf:Description rdf:about="http://purl.org/dc/terms/abstract">
        <rdfs:label xml:lang="en">Abstract</rdfs:label>
        <dcterms:hasVersion rdf:resource="http://dublincore.org/usage/terms/history/#abstract-003"/>
        <rdfs:isDefinedBy rdf:resource="http://purl.org/dc/terms/"/>
        <rdfs:comment xml:lang="en">A summary of the resource.</rdfs:comment>
    </rdf:Description>
    <rdf:Description rdf:about="http://purl.org/dc/terms/accessRights">
        <dcterms:description xml:lang="en">Access Rights may include information regarding access or restrictions based on privacy, security, or other policies.</dcterms:description>
        <rdfs:comment xml:lang="en">Information about who can access the resource or an indication of its security status.</rdfs:comment>
        <rdfs:label xml:lang="en">Access Rights</rdfs:label>
        <dcterms:hasVersion rdf:resource="http://dublincore.org/usage/terms/history/#accessRights-002"/>
        <rdfs:isDefinedBy rdf:resource="http://purl.org/dc/terms/"/>
    </rdf:Description>
    <rdf:Description rdf:about="http://purl.org/dc/terms/accrualMethod">
        <rdfs:label xml:lang="en">Accrual Method</rdfs:label>
        <dcterms:hasVersion rdf:resource="http://dublincore.org/usage/terms/history/#accrualMethod-003"/>
        <rdfs:comment xml:lang="en">The method by which items are added to a collection.</rdfs:comment>
        <rdfs:isDefinedBy rdf:resource="http://purl.org/dc/terms/"/>
    </rdf:Description>
    <rdf:Description rdf:about="http://purl.org/dc/terms/accrualPeriodicity">
        <dcterms:hasVersion rdf:resource="http://dublincore.org/usage/terms/history/#accrualPeriodicity-003"/>
        <rdfs:label xml:lang="en">Accrual Periodicity</rdfs:label>
        <rdfs:comment xml:lang="en">The frequency with which items are added to a collection.</rdfs:comment>
        <rdfs:isDefinedBy rdf:resource="http://purl.org/dc/terms/"/>
    </rdf:Description>
    <rdf:Description rdf:about="http://purl.org/dc/terms/accrualPolicy">
        <rdfs:isDefinedBy rdf:resource="http://purl.org/dc/terms/"/>
        <rdfs:comment xml:lang="en">The policy governing the addition of items to a collection.</rdfs:comment>
        <dcterms:hasVersion rdf:resource="http://dublincore.org/usage/terms/history/#accrualPolicy-003"/>
        <rdfs:label xml:lang="en">Accrual Policy</rdfs:label>
    </rdf:Description>
    <rdf:Description rdf:about="http://purl.org/dc/terms/alternative">
        <rdfs:comment xml:lang="en">An alternative name for the resource.</rdfs:comment>
        <rdfs:isDefinedBy rdf:resource="http://purl.org/dc/terms/"/>
        <dcterms:hasVersion rdf:resource="http://dublincore.org/usage/terms/history/#alternative-003"/>
        <dcterms:description xml:lang="en">The distinction between titles and alternative titles is application-specific.</dcterms:description>
        <rdfs:label xml:lang="en">Alternative Title</rdfs:label>
    </rdf:Description>
    <rdf:Description rdf:about="http://purl.org/dc/terms/audience">
        <rdfs:comment xml:lang="en">A class of entity for whom the resource is intended or useful.</rdfs:comment>
        <dcterms:hasVersion rdf:resource="http://dublincore.org/usage/terms/history/#audience-003"/>
        <rdfs:label xml:lang="en">Audience</rdfs:label>
        <rdfs:isDefinedBy rdf:resource="http://purl.org/dc/terms/"/>
    </rdf:Description>
    <rdf:Description rdf:about="http://purl.org/dc/terms/available">
        <rdfs:isDefinedBy rdf:resource="http://purl.org/dc/terms/"/>
        <rdfs:label xml:lang="en">Date Available</rdfs:label>
        <rdfs:comment xml:lang="en">Date (often a range) that the resource became or will become available.</rdfs:comment>
        <dcterms:hasVersion rdf:resource="http://dublincore.org/usage/terms/history/#available-003"/>
    </rdf:Description>
    <rdf:Description rdf:about="http://purl.org/dc/terms/bibliographicCitation">
        <dcterms:description xml:lang="en">Recommended practice is to include sufficient bibliographic detail to identify the resource as unambiguously as possible.</dcterms:description>
        <rdfs:label xml:lang="en">Bibliographic Citation</rdfs:label>
        <dcterms:hasVersion rdf:resource="http://dublincore.org/usage/terms/history/#bibliographicCitation-002"/>
        <rdfs:comment xml:lang="en">A bibliographic reference for the resource.</rdfs:comment>
        <rdfs:isDefinedBy rdf:resource="http://purl.org/dc/terms/"/>
    </rdf:Description>
    <rdf:Description rdf:about="http://purl.org/dc/terms/conformsTo">
        <rdfs:isDefinedBy rdf:resource="http://purl.org/dc/terms/"/>
        <rdfs:label xml:lang="en">Conforms To</rdfs:label>
        <rdfs:comment xml:lang="en">An established standard to which the described resource conforms.</rdfs:comment>
        <dcterms:hasVersion rdf:resource="http://dublincore.org/usage/terms/history/#conformsTo-003"/>
    </rdf:Description>
    <rdf:Description rdf:about="http://purl.org/dc/terms/contributor">
        <rdfs:comment xml:lang="en">An entity responsible for making contributions to the resource.</rdfs:comment>
        <rdfs:isDefinedBy rdf:resource="http://purl.org/dc/terms/"/>
        <dcterms:description xml:lang="en">Examples of a Contributor include a person, an organization, or a service.</dcterms:description>
        <dcterms:hasVersion rdf:resource="http://dublincore.org/usage/terms/history/#contributorT-001"/>
        <rdfs:label xml:lang="en">Contributor</rdfs:label>
    </rdf:Description>
    <rdf:Description rdf:about="http://purl.org/dc/terms/coverage">
        <rdfs:isDefinedBy rdf:resource="http://purl.org/dc/terms/"/>
        <dcterms:hasVersion rdf:resource="http://dublincore.org/usage/terms/history/#coverageT-001"/>
        <rdfs:label xml:lang="en">Coverage</rdfs:label>
        <dcterms:description xml:lang="en">Spatial topic and spatial applicability may be a named place or a location specified by its geographic coordinates. Temporal topic may be a named period, date, or date range. A jurisdiction may be a named administrative entity or a geographic place to which the resource applies. Recommended best practice is to use a controlled vocabulary such as the Thesaurus of Geographic Names [TGN]. Where appropriate, named places or time periods can be used in preference to numeric identifiers such as sets of coordinates or date ranges.</dcterms:description>
        <rdfs:comment xml:lang="en">The spatial or temporal topic of the resource, the spatial applicability of the resource, or the jurisdiction under which the resource is relevant.</rdfs:comment>
    </rdf:Description>
    <rdf:Description rdf:about="http://purl.org/dc/terms/created">
        <rdfs:isDefinedBy rdf:resource="http://purl.org/dc/terms/"/>
        <rdfs:comment xml:lang="en">Date of creation of the resource.</rdfs:comment>
        <dcterms:hasVersion rdf:resource="http://dublincore.org/usage/terms/history/#created-003"/>
        <rdfs:label xml:lang="en">Date Created</rdfs:label>
    </rdf:Description>
    <rdf:Description rdf:about="http://purl.org/dc/terms/creator">
        <rdfs:comment xml:lang="en">An entity primarily responsible for making the resource.</rdfs:comment>
        <dcterms:hasVersion rdf:resource="http://dublincore.org/usage/terms/history/#creatorT-002"/>
        <rdfs:isDefinedBy rdf:resource="http://purl.org/dc/terms/"/>
        <rdfs:label xml:lang="en">Creator</rdfs:label>
        <dcterms:description xml:lang="en">Examples of a Creator include a person, an organization, or a service.</dcterms:description>
    </rdf:Description>
    <rdf:Description rdf:about="http://purl.org/dc/terms/date">
        <rdfs:isDefinedBy rdf:resource="http://purl.org/dc/terms/"/>
        <dcterms:hasVersion rdf:resource="http://dublincore.org/usage/terms/history/#dateT-001"/>
        <rdfs:comment xml:lang="en">A point or period of time associated with an event in the lifecycle of the resource.</rdfs:comment>
        <dcterms:description xml:lang="en">Date may be used to express temporal information at any level of granularity.  Recommended best practice is to use an encoding scheme, such as the W3CDTF profile of ISO 8601 [W3CDTF].</dcterms:description>
        <rdfs:label xml:lang="en">Date</rdfs:label>
    </rdf:Description>
    <rdf:Description rdf:about="http://purl.org/dc/terms/dateAccepted">
        <dcterms:hasVersion rdf:resource="http://dublincore.org/usage/terms/history/#dateAccepted-002"/>
        <dcterms:description xml:lang="en">Examples of resources to which a Date Accepted may be relevant are a thesis (accepted by a university department) or an article (accepted by a journal).</dcterms:description>
        <rdfs:comment xml:lang="en">Date of acceptance of the resource.</rdfs:comment>
        <rdfs:label xml:lang="en">Date Accepted</rdfs:label>
        <rdfs:isDefinedBy rdf:resource="http://purl.org/dc/terms/"/>
    </rdf:Description>
    <rdf:Description rdf:about="http://purl.org/dc/terms/dateCopyrighted">
        <rdfs:isDefinedBy rdf:resource="http://purl.org/dc/terms/"/>
        <rdfs:label xml:lang="en">Date Copyrighted</rdfs:label>
        <rdfs:comment xml:lang="en">Date of copyright.</rdfs:comment>
        <dcterms:hasVersion rdf:resource="http://dublincore.org/usage/terms/history/#dateCopyrighted-002"/>
    </rdf:Description>
    <rdf:Description rdf:about="http://purl.org/dc/terms/dateSubmitted">
        <rdfs:comment xml:lang="en">Date of submission of the resource.</rdfs:comment>
        <dcterms:description xml:lang="en">Examples of resources to which a Date Submitted may be relevant are a thesis (submitted to a university department) or an article (submitted to a journal).</dcterms:description>
        <rdfs:label xml:lang="en">Date Submitted</rdfs:label>
        <dcterms:hasVersion rdf:resource="http://dublincore.org/usage/terms/history/#dateSubmitted-002"/>
        <rdfs:isDefinedBy rdf:resource="http://purl.org/dc/terms/"/>
    </rdf:Description>
    <owl:AnnotationProperty rdf:about="http://purl.org/dc/terms/description">
        <rdfs:label xml:lang="en">Description</rdfs:label>
        <rdfs:isDefinedBy rdf:resource="http://purl.org/dc/terms/"/>
        <rdfs:comment xml:lang="en">An account of the resource.</rdfs:comment>
        <dcterms:hasVersion rdf:resource="http://dublincore.org/usage/terms/history/#descriptionT-001"/>
        <dcterms:description xml:lang="en">Description may include but is not limited to: an abstract, a table of contents, a graphical representation, or a free-text account of the resource.</dcterms:description>
    </owl:AnnotationProperty>
    <rdf:Description rdf:about="http://purl.org/dc/terms/educationLevel">
        <rdfs:isDefinedBy rdf:resource="http://purl.org/dc/terms/"/>
        <rdfs:label xml:lang="en">Audience Education Level</rdfs:label>
        <rdfs:comment xml:lang="en">A class of entity, defined in terms of progression through an educational or training context, for which the described resource is intended.</rdfs:comment>
        <dcterms:hasVersion rdf:resource="http://dublincore.org/usage/terms/history/#educationLevel-002"/>
    </rdf:Description>
    <rdf:Description rdf:about="http://purl.org/dc/terms/extent">
        <rdfs:isDefinedBy rdf:resource="http://purl.org/dc/terms/"/>
        <rdfs:comment xml:lang="en">The size or duration of the resource.</rdfs:comment>
        <rdfs:label xml:lang="en">Extent</rdfs:label>
        <dcterms:hasVersion rdf:resource="http://dublincore.org/usage/terms/history/#extent-003"/>
    </rdf:Description>
    <rdf:Description rdf:about="http://purl.org/dc/terms/format">
        <dcterms:hasVersion rdf:resource="http://dublincore.org/usage/terms/history/#formatT-001"/>
        <rdfs:comment xml:lang="en">The file format, physical medium, or dimensions of the resource.</rdfs:comment>
        <dcterms:description xml:lang="en">Examples of dimensions include size and duration. Recommended best practice is to use a controlled vocabulary such as the list of Internet Media Types [MIME].</dcterms:description>
        <rdfs:isDefinedBy rdf:resource="http://purl.org/dc/terms/"/>
        <rdfs:label xml:lang="en">Format</rdfs:label>
    </rdf:Description>
    <rdf:Description rdf:about="http://purl.org/dc/terms/hasFormat">
        <skos:note xml:lang="en">This term is intended to be used with non-literal values as defined in the DCMI Abstract Model (http://dublincore.org/documents/abstract-model/).  As of December 2007, the DCMI Usage Board is seeking a way to express this intention with a formal range declaration.</skos:note>
        <rdfs:isDefinedBy rdf:resource="http://purl.org/dc/terms/"/>
        <dcterms:hasVersion rdf:resource="http://dublincore.org/usage/terms/history/#hasFormat-003"/>
        <rdfs:label xml:lang="en">Has Format</rdfs:label>
        <rdfs:comment xml:lang="en">A related resource that is substantially the same as the pre-existing described resource, but in another format.</rdfs:comment>
    </rdf:Description>
    <rdf:Description rdf:about="http://purl.org/dc/terms/hasPart">
        <rdfs:isDefinedBy rdf:resource="http://purl.org/dc/terms/"/>
        <skos:note xml:lang="en">This term is intended to be used with non-literal values as defined in the DCMI Abstract Model (http://dublincore.org/documents/abstract-model/).  As of December 2007, the DCMI Usage Board is seeking a way to express this intention with a formal range declaration.</skos:note>
        <rdfs:label xml:lang="en">Has Part</rdfs:label>
        <rdfs:comment xml:lang="en">A related resource that is included either physically or logically in the described resource.</rdfs:comment>
        <dcterms:hasVersion rdf:resource="http://dublincore.org/usage/terms/history/#hasPart-003"/>
    </rdf:Description>
    <owl:AnnotationProperty rdf:about="http://purl.org/dc/terms/hasVersion">
        <dcterms:hasVersion rdf:resource="http://dublincore.org/usage/terms/history/#hasVersion-003"/>
        <rdfs:isDefinedBy rdf:resource="http://purl.org/dc/terms/"/>
        <rdfs:comment xml:lang="en">A related resource that is a version, edition, or adaptation of the described resource.</rdfs:comment>
        <skos:note xml:lang="en">This term is intended to be used with non-literal values as defined in the DCMI Abstract Model (http://dublincore.org/documents/abstract-model/).  As of December 2007, the DCMI Usage Board is seeking a way to express this intention with a formal range declaration.</skos:note>
        <rdfs:label xml:lang="en">Has Version</rdfs:label>
    </owl:AnnotationProperty>
    <rdf:Description rdf:about="http://purl.org/dc/terms/identifier">
        <dcterms:hasVersion rdf:resource="http://dublincore.org/usage/terms/history/#identifierT-001"/>
        <rdfs:isDefinedBy rdf:resource="http://purl.org/dc/terms/"/>
        <dcterms:description xml:lang="en">Recommended best practice is to identify the resource by means of a string conforming to a formal identification system. </dcterms:description>
        <rdfs:comment xml:lang="en">An unambiguous reference to the resource within a given context.</rdfs:comment>
        <rdfs:label xml:lang="en">Identifier</rdfs:label>
    </rdf:Description>
    <rdf:Description rdf:about="http://purl.org/dc/terms/instructionalMethod">
        <dcterms:description xml:lang="en">Instructional Method will typically include ways of presenting instructional materials or conducting instructional activities, patterns of learner-to-learner and learner-to-instructor interactions, and mechanisms by which group and individual levels of learning are measured.  Instructional methods include all aspects of the instruction and learning processes from planning and implementation through evaluation and feedback.</dcterms:description>
        <rdfs:label xml:lang="en">Instructional Method</rdfs:label>
        <rdfs:comment xml:lang="en">A process, used to engender knowledge, attitudes and skills, that the described resource is designed to support.</rdfs:comment>
        <dcterms:hasVersion rdf:resource="http://dublincore.org/usage/terms/history/#instructionalMethod-002"/>
        <rdfs:isDefinedBy rdf:resource="http://purl.org/dc/terms/"/>
    </rdf:Description>
    <rdf:Description rdf:about="http://purl.org/dc/terms/isFormatOf">
        <dcterms:hasVersion rdf:resource="http://dublincore.org/usage/terms/history/#isFormatOf-003"/>
        <rdfs:comment xml:lang="en">A related resource that is substantially the same as the described resource, but in another format.</rdfs:comment>
        <skos:note xml:lang="en">This term is intended to be used with non-literal values as defined in the DCMI Abstract Model (http://dublincore.org/documents/abstract-model/).  As of December 2007, the DCMI Usage Board is seeking a way to express this intention with a formal range declaration.</skos:note>
        <rdfs:isDefinedBy rdf:resource="http://purl.org/dc/terms/"/>
        <rdfs:label xml:lang="en">Is Format Of</rdfs:label>
    </rdf:Description>
    <rdf:Description rdf:about="http://purl.org/dc/terms/isPartOf">
        <rdfs:label xml:lang="en">Is Part Of</rdfs:label>
        <dcterms:hasVersion rdf:resource="http://dublincore.org/usage/terms/history/#isPartOf-003"/>
        <skos:note xml:lang="en">This term is intended to be used with non-literal values as defined in the DCMI Abstract Model (http://dublincore.org/documents/abstract-model/).  As of December 2007, the DCMI Usage Board is seeking a way to express this intention with a formal range declaration.</skos:note>
        <rdfs:isDefinedBy rdf:resource="http://purl.org/dc/terms/"/>
        <rdfs:comment xml:lang="en">A related resource in which the described resource is physically or logically included.</rdfs:comment>
    </rdf:Description>
    <rdf:Description rdf:about="http://purl.org/dc/terms/isReferencedBy">
        <rdfs:label xml:lang="en">Is Referenced By</rdfs:label>
        <rdfs:comment xml:lang="en">A related resource that references, cites, or otherwise points to the described resource.</rdfs:comment>
        <skos:note xml:lang="en">This term is intended to be used with non-literal values as defined in the DCMI Abstract Model (http://dublincore.org/documents/abstract-model/).  As of December 2007, the DCMI Usage Board is seeking a way to express this intention with a formal range declaration.</skos:note>
        <rdfs:isDefinedBy rdf:resource="http://purl.org/dc/terms/"/>
        <dcterms:hasVersion rdf:resource="http://dublincore.org/usage/terms/history/#isReferencedBy-003"/>
    </rdf:Description>
    <rdf:Description rdf:about="http://purl.org/dc/terms/isReplacedBy">
        <rdfs:isDefinedBy rdf:resource="http://purl.org/dc/terms/"/>
        <rdfs:label xml:lang="en">Is Replaced By</rdfs:label>
        <rdfs:comment xml:lang="en">A related resource that supplants, displaces, or supersedes the described resource.</rdfs:comment>
        <skos:note xml:lang="en">This term is intended to be used with non-literal values as defined in the DCMI Abstract Model (http://dublincore.org/documents/abstract-model/).  As of December 2007, the DCMI Usage Board is seeking a way to express this intention with a formal range declaration.</skos:note>
        <dcterms:hasVersion rdf:resource="http://dublincore.org/usage/terms/history/#isReplacedBy-003"/>
    </rdf:Description>
    <rdf:Description rdf:about="http://purl.org/dc/terms/isRequiredBy">
        <skos:note xml:lang="en">This term is intended to be used with non-literal values as defined in the DCMI Abstract Model (http://dublincore.org/documents/abstract-model/).  As of December 2007, the DCMI Usage Board is seeking a way to express this intention with a formal range declaration.</skos:note>
        <rdfs:isDefinedBy rdf:resource="http://purl.org/dc/terms/"/>
        <rdfs:label xml:lang="en">Is Required By</rdfs:label>
        <dcterms:hasVersion rdf:resource="http://dublincore.org/usage/terms/history/#isRequiredBy-003"/>
        <rdfs:comment xml:lang="en">A related resource that requires the described resource to support its function, delivery, or coherence.</rdfs:comment>
    </rdf:Description>
    <rdf:Description rdf:about="http://purl.org/dc/terms/isVersionOf">
        <rdfs:label xml:lang="en">Is Version Of</rdfs:label>
        <rdfs:comment xml:lang="en">A related resource of which the described resource is a version, edition, or adaptation.</rdfs:comment>
        <rdfs:isDefinedBy rdf:resource="http://purl.org/dc/terms/"/>
        <skos:note xml:lang="en">This term is intended to be used with non-literal values as defined in the DCMI Abstract Model (http://dublincore.org/documents/abstract-model/).  As of December 2007, the DCMI Usage Board is seeking a way to express this intention with a formal range declaration.</skos:note>
        <dcterms:hasVersion rdf:resource="http://dublincore.org/usage/terms/history/#isVersionOf-003"/>
        <dcterms:description xml:lang="en">Changes in version imply substantive changes in content rather than differences in format.</dcterms:description>
    </rdf:Description>
    <rdf:Description rdf:about="http://purl.org/dc/terms/issued">
        <rdfs:comment xml:lang="en">Date of formal issuance (e.g., publication) of the resource.</rdfs:comment>
        <rdfs:isDefinedBy rdf:resource="http://purl.org/dc/terms/"/>
        <dcterms:hasVersion rdf:resource="http://dublincore.org/usage/terms/history/#issued-003"/>
        <rdfs:label xml:lang="en">Date Issued</rdfs:label>
    </rdf:Description>
    <rdf:Description rdf:about="http://purl.org/dc/terms/language">
        <rdfs:label xml:lang="en">Language</rdfs:label>
        <dcterms:hasVersion rdf:resource="http://dublincore.org/usage/terms/history/#languageT-001"/>
        <dcterms:description xml:lang="en">Recommended best practice is to use a controlled vocabulary such as RFC 4646 [RFC4646].</dcterms:description>
        <rdfs:isDefinedBy rdf:resource="http://purl.org/dc/terms/"/>
        <rdfs:comment xml:lang="en">A language of the resource.</rdfs:comment>
    </rdf:Description>
    <rdf:Description rdf:about="http://purl.org/dc/terms/license">
        <rdfs:label xml:lang="en">License</rdfs:label>
        <rdfs:comment xml:lang="en">A legal document giving official permission to do something with the resource.</rdfs:comment>
        <dcterms:hasVersion rdf:resource="http://dublincore.org/usage/terms/history/#license-002"/>
        <rdfs:isDefinedBy rdf:resource="http://purl.org/dc/terms/"/>
    </rdf:Description>
    <rdf:Description rdf:about="http://purl.org/dc/terms/mediator">
        <dcterms:description xml:lang="en">In an educational context, a mediator might be a parent, teacher, teaching assistant, or care-giver.</dcterms:description>
        <rdfs:comment xml:lang="en">An entity that mediates access to the resource and for whom the resource is intended or useful.</rdfs:comment>
        <dcterms:hasVersion rdf:resource="http://dublincore.org/usage/terms/history/#mediator-003"/>
        <rdfs:isDefinedBy rdf:resource="http://purl.org/dc/terms/"/>
        <rdfs:label xml:lang="en">Mediator</rdfs:label>
    </rdf:Description>
    <rdf:Description rdf:about="http://purl.org/dc/terms/medium">
        <rdfs:isDefinedBy rdf:resource="http://purl.org/dc/terms/"/>
        <rdfs:label xml:lang="en">Medium</rdfs:label>
        <rdfs:comment xml:lang="en">The material or physical carrier of the resource.</rdfs:comment>
        <dcterms:hasVersion rdf:resource="http://dublincore.org/usage/terms/history/#medium-003"/>
    </rdf:Description>
    <rdf:Description rdf:about="http://purl.org/dc/terms/modified">
        <rdfs:isDefinedBy rdf:resource="http://purl.org/dc/terms/"/>
        <rdfs:label xml:lang="en">Date Modified</rdfs:label>
        <dcterms:hasVersion rdf:resource="http://dublincore.org/usage/terms/history/#modified-003"/>
        <rdfs:comment xml:lang="en">Date on which the resource was changed.</rdfs:comment>
    </rdf:Description>
    <rdf:Description rdf:about="http://purl.org/dc/terms/provenance">
        <rdfs:comment xml:lang="en">A statement of any changes in ownership and custody of the resource since its creation that are significant for its authenticity, integrity, and interpretation.</rdfs:comment>
        <rdfs:isDefinedBy rdf:resource="http://purl.org/dc/terms/"/>
        <dcterms:description xml:lang="en">The statement may include a description of any changes successive custodians made to the resource.</dcterms:description>
        <dcterms:hasVersion rdf:resource="http://dublincore.org/usage/terms/history/#provenance-002"/>
        <rdfs:label xml:lang="en">Provenance</rdfs:label>
    </rdf:Description>
    <rdf:Description rdf:about="http://purl.org/dc/terms/publisher">
        <rdfs:label xml:lang="en">Publisher</rdfs:label>
        <dcterms:description xml:lang="en">Examples of a Publisher include a person, an organization, or a service.</dcterms:description>
        <dcterms:hasVersion rdf:resource="http://dublincore.org/usage/terms/history/#publisherT-001"/>
        <rdfs:isDefinedBy rdf:resource="http://purl.org/dc/terms/"/>
        <rdfs:comment xml:lang="en">An entity responsible for making the resource available.</rdfs:comment>
    </rdf:Description>
    <rdf:Description rdf:about="http://purl.org/dc/terms/references">
        <rdfs:comment xml:lang="en">A related resource that is referenced, cited, or otherwise pointed to by the described resource.</rdfs:comment>
        <rdfs:label xml:lang="en">References</rdfs:label>
        <dcterms:hasVersion rdf:resource="http://dublincore.org/usage/terms/history/#references-003"/>
        <skos:note xml:lang="en">This term is intended to be used with non-literal values as defined in the DCMI Abstract Model (http://dublincore.org/documents/abstract-model/).  As of December 2007, the DCMI Usage Board is seeking a way to express this intention with a formal range declaration.</skos:note>
        <rdfs:isDefinedBy rdf:resource="http://purl.org/dc/terms/"/>
    </rdf:Description>
    <rdf:Description rdf:about="http://purl.org/dc/terms/relation">
        <skos:note xml:lang="en">This term is intended to be used with non-literal values as defined in the DCMI Abstract Model (http://dublincore.org/documents/abstract-model/).  As of December 2007, the DCMI Usage Board is seeking a way to express this intention with a formal range declaration.</skos:note>
        <rdfs:isDefinedBy rdf:resource="http://purl.org/dc/terms/"/>
        <dcterms:hasVersion rdf:resource="http://dublincore.org/usage/terms/history/#relationT-001"/>
        <dcterms:description xml:lang="en">Recommended best practice is to identify the related resource by means of a string conforming to a formal identification system. </dcterms:description>
        <rdfs:label xml:lang="en">Relation</rdfs:label>
        <rdfs:comment xml:lang="en">A related resource.</rdfs:comment>
    </rdf:Description>
    <rdf:Description rdf:about="http://purl.org/dc/terms/replaces">
        <skos:note xml:lang="en">This term is intended to be used with non-literal values as defined in the DCMI Abstract Model (http://dublincore.org/documents/abstract-model/).  As of December 2007, the DCMI Usage Board is seeking a way to express this intention with a formal range declaration.</skos:note>
        <rdfs:label xml:lang="en">Replaces</rdfs:label>
        <dcterms:hasVersion rdf:resource="http://dublincore.org/usage/terms/history/#replaces-003"/>
        <rdfs:comment xml:lang="en">A related resource that is supplanted, displaced, or superseded by the described resource.</rdfs:comment>
        <rdfs:isDefinedBy rdf:resource="http://purl.org/dc/terms/"/>
    </rdf:Description>
    <rdf:Description rdf:about="http://purl.org/dc/terms/requires">
        <dcterms:hasVersion rdf:resource="http://dublincore.org/usage/terms/history/#requires-003"/>
        <rdfs:label xml:lang="en">Requires</rdfs:label>
        <rdfs:comment xml:lang="en">A related resource that is required by the described resource to support its function, delivery, or coherence.</rdfs:comment>
        <rdfs:isDefinedBy rdf:resource="http://purl.org/dc/terms/"/>
        <skos:note xml:lang="en">This term is intended to be used with non-literal values as defined in the DCMI Abstract Model (http://dublincore.org/documents/abstract-model/).  As of December 2007, the DCMI Usage Board is seeking a way to express this intention with a formal range declaration.</skos:note>
    </rdf:Description>
    <rdf:Description rdf:about="http://purl.org/dc/terms/rights">
        <rdfs:isDefinedBy rdf:resource="http://purl.org/dc/terms/"/>
        <rdfs:label xml:lang="en">Rights</rdfs:label>
        <rdfs:comment xml:lang="en">Information about rights held in and over the resource.</rdfs:comment>
        <dcterms:hasVersion rdf:resource="http://dublincore.org/usage/terms/history/#rightsT-001"/>
        <dcterms:description xml:lang="en">Typically, rights information includes a statement about various property rights associated with the resource, including intellectual property rights.</dcterms:description>
    </rdf:Description>
    <rdf:Description rdf:about="http://purl.org/dc/terms/rightsHolder">
        <dcterms:hasVersion rdf:resource="http://dublincore.org/usage/terms/history/#rightsHolder-002"/>
        <rdfs:isDefinedBy rdf:resource="http://purl.org/dc/terms/"/>
        <rdfs:comment xml:lang="en">A person or organization owning or managing rights over the resource.</rdfs:comment>
        <rdfs:label xml:lang="en">Rights Holder</rdfs:label>
    </rdf:Description>
    <rdf:Description rdf:about="http://purl.org/dc/terms/source">
        <rdfs:label xml:lang="en">Source</rdfs:label>
        <skos:note xml:lang="en">This term is intended to be used with non-literal values as defined in the DCMI Abstract Model (http://dublincore.org/documents/abstract-model/).  As of December 2007, the DCMI Usage Board is seeking a way to express this intention with a formal range declaration.</skos:note>
        <rdfs:isDefinedBy rdf:resource="http://purl.org/dc/terms/"/>
        <dcterms:hasVersion rdf:resource="http://dublincore.org/usage/terms/history/#sourceT-001"/>
        <rdfs:comment xml:lang="en">A related resource from which the described resource is derived.</rdfs:comment>
        <dcterms:description xml:lang="en">The described resource may be derived from the related resource in whole or in part. Recommended best practice is to identify the related resource by means of a string conforming to a formal identification system.</dcterms:description>
    </rdf:Description>
    <rdf:Description rdf:about="http://purl.org/dc/terms/spatial">
        <rdfs:label xml:lang="en">Spatial Coverage</rdfs:label>
        <rdfs:isDefinedBy rdf:resource="http://purl.org/dc/terms/"/>
        <rdfs:comment xml:lang="en">Spatial characteristics of the resource.</rdfs:comment>
        <dcterms:hasVersion rdf:resource="http://dublincore.org/usage/terms/history/#spatial-003"/>
    </rdf:Description>
    <rdf:Description rdf:about="http://purl.org/dc/terms/subject">
        <dcterms:hasVersion rdf:resource="http://dublincore.org/usage/terms/history/#subjectT-002"/>
        <skos:note xml:lang="en">This term is intended to be used with non-literal values as defined in the DCMI Abstract Model (http://dublincore.org/documents/abstract-model/).  As of December 2007, the DCMI Usage Board is seeking a way to express this intention with a formal range declaration.</skos:note>
        <rdfs:label xml:lang="en">Subject</rdfs:label>
        <rdfs:comment xml:lang="en">The topic of the resource.</rdfs:comment>
        <dcterms:description xml:lang="en">Typically, the subject will be represented using keywords, key phrases, or classification codes. Recommended best practice is to use a controlled vocabulary.</dcterms:description>
        <rdfs:isDefinedBy rdf:resource="http://purl.org/dc/terms/"/>
    </rdf:Description>
    <rdf:Description rdf:about="http://purl.org/dc/terms/tableOfContents">
        <rdfs:comment xml:lang="en">A list of subunits of the resource.</rdfs:comment>
        <rdfs:isDefinedBy rdf:resource="http://purl.org/dc/terms/"/>
        <rdfs:label xml:lang="en">Table Of Contents</rdfs:label>
        <dcterms:hasVersion rdf:resource="http://dublincore.org/usage/terms/history/#tableOfContents-003"/>
    </rdf:Description>
    <rdf:Description rdf:about="http://purl.org/dc/terms/temporal">
        <rdfs:label xml:lang="en">Temporal Coverage</rdfs:label>
        <dcterms:hasVersion rdf:resource="http://dublincore.org/usage/terms/history/#temporal-003"/>
        <rdfs:comment xml:lang="en">Temporal characteristics of the resource.</rdfs:comment>
        <rdfs:isDefinedBy rdf:resource="http://purl.org/dc/terms/"/>
    </rdf:Description>
    <rdf:Description rdf:about="http://purl.org/dc/terms/title">
        <rdfs:label xml:lang="en">Title</rdfs:label>
        <rdfs:comment xml:lang="en">A name given to the resource.</rdfs:comment>
        <dcterms:hasVersion rdf:resource="http://dublincore.org/usage/terms/history/#titleT-002"/>
        <rdfs:isDefinedBy rdf:resource="http://purl.org/dc/terms/"/>
    </rdf:Description>
    <rdf:Description rdf:about="http://purl.org/dc/terms/type">
        <rdfs:isDefinedBy rdf:resource="http://purl.org/dc/terms/"/>
        <dcterms:description xml:lang="en">Recommended best practice is to use a controlled vocabulary such as the DCMI Type Vocabulary [DCMITYPE]. To describe the file format, physical medium, or dimensions of the resource, use the Format element.</dcterms:description>
        <rdfs:comment xml:lang="en">The nature or genre of the resource.</rdfs:comment>
        <rdfs:label xml:lang="en">Type</rdfs:label>
        <dcterms:hasVersion rdf:resource="http://dublincore.org/usage/terms/history/#typeT-001"/>
    </rdf:Description>
    <rdf:Description rdf:about="http://purl.org/dc/terms/valid">
        <rdfs:comment xml:lang="en">Date (often a range) of validity of a resource.</rdfs:comment>
        <rdfs:label xml:lang="en">Date Valid</rdfs:label>
        <rdfs:isDefinedBy rdf:resource="http://purl.org/dc/terms/"/>
        <dcterms:hasVersion rdf:resource="http://dublincore.org/usage/terms/history/#valid-003"/>
    </rdf:Description>
</rdf:RDF>



<!-- Generated by the OWL API (version 4.5.6.2018-09-06T00:27:41Z) https://github.com/owlcs/owlapi -->

